@prefix dcterms: <http://purl.org/dc/terms/> .
@prefix linkml: <https://w3id.org/linkml/> .
@prefix owl: <http://www.w3.org/2002/07/owl#> .
@prefix rdfs: <http://www.w3.org/2000/01/rdf-schema#> .
@prefix skos: <http://www.w3.org/2004/02/skos/core#> .
@prefix xsd: <http://www.w3.org/2001/XMLSchema#> .

<https://example.org/crdch_model> a owl:Ontology ;
    rdfs:label "CRDC-H" ;
    dcterms:license "https://creativecommons.org/publicdomain/zero/1.0/" ;
    skos:editorialNote "Derived from [CDM_Dictionary_v1 (Active)](https://docs.google.com/spreadsheets/d/1oWS7cao-fgz2MKWtyr8h2dEL9unX__0bJrWKv6mQmM4)" ;
    linkml:generation_date "2021-08-23 08:43" ;
    linkml:metamodel_version "1.7.0" ;
    linkml:source_file "crdch_model.yaml" ;
    linkml:source_file_date "Thu Aug 19 12:22:13 2021" ;
    linkml:source_file_size 1079148 .

<https://example.org/crdch_model/CcdhBoolean> a owl:Class,
        linkml:TypeDefinition ;
    rdfs:label "ccdh_boolean" ;
    rdfs:subClassOf linkml:Boolean ;
    skos:definition "Value representing either “true” or “false”.  Permissible values (case-sensitive) = “true”, “false”, “1”, “0”." ;
    skos:editorialNote "Derived from [ccdh_boolean in sheet Primitives](https://docs.google.com/spreadsheets/d/1oWS7cao-fgz2MKWtyr8h2dEL9unX__0bJrWKv6mQmM4/edit#gid=497370447)" .

<https://example.org/crdch_model/CcdhCode> a owl:Class,
        linkml:TypeDefinition ;
    rdfs:label "ccdh_code" ;
    rdfs:subClassOf linkml:String ;
    skos:definition "" ;
    skos:editorialNote "Derived from [ccdh_code in sheet Primitives](https://docs.google.com/spreadsheets/d/1oWS7cao-fgz2MKWtyr8h2dEL9unX__0bJrWKv6mQmM4/edit#gid=497370447)" .

<https://example.org/crdch_model/CcdhCurie> a owl:Class,
        linkml:TypeDefinition ;
    rdfs:label "ccdh_curie" ;
    rdfs:subClassOf linkml:Uriorcurie ;
    skos:definition "A compact URI (CURIE), which is a bipartite identifier of the form prefix:reference, in which the prefix is a convenient abbreviation of a URI.  It is expressed in the format “prefix:reference”. When a mapping of prefix to base URI is provided (external to this data type), a CURIE may be mapped to a URI." ;
    skos:editorialNote "Derived from [ccdh_curie in sheet Primitives](https://docs.google.com/spreadsheets/d/1oWS7cao-fgz2MKWtyr8h2dEL9unX__0bJrWKv6mQmM4/edit#gid=497370447)" .

<https://example.org/crdch_model/CcdhDateTime> a owl:Class,
        linkml:TypeDefinition ;
    rdfs:label "ccdh_dateTime" ;
    rdfs:subClassOf linkml:Datetime ;
    skos:definition "A date and time string specified using a specialized concatenation of the date and time data types, in the general format YYYY-MM-DDThh:mm:ss+zz:zz." ;
    skos:editorialNote "Derived from [ccdh_dateTime in sheet Primitives](https://docs.google.com/spreadsheets/d/1oWS7cao-fgz2MKWtyr8h2dEL9unX__0bJrWKv6mQmM4/edit#gid=497370447)" .

<https://example.org/crdch_model/CcdhDecimal> a owl:Class,
        linkml:TypeDefinition ;
    rdfs:label "ccdh_decimal" ;
    rdfs:subClassOf linkml:Decimal ;
    skos:definition "A rational number that has a decimal representation.  This data type does not restrict the size or precision of the number." ;
    skos:editorialNote "Derived from [ccdh_decimal in sheet Primitives](https://docs.google.com/spreadsheets/d/1oWS7cao-fgz2MKWtyr8h2dEL9unX__0bJrWKv6mQmM4/edit#gid=497370447)" .

<https://example.org/crdch_model/CcdhInteger> a owl:Class,
        linkml:TypeDefinition ;
    rdfs:label "ccdh_integer" ;
    rdfs:subClassOf linkml:Integer ;
    skos:definition "An integer number.  This data type is based on the decimal type, but the fractional component is not allowed.  There are no restrictions on the size of the integer." ;
    skos:editorialNote "Derived from [ccdh_integer in sheet Primitives](https://docs.google.com/spreadsheets/d/1oWS7cao-fgz2MKWtyr8h2dEL9unX__0bJrWKv6mQmM4/edit#gid=497370447)" .

<https://example.org/crdch_model/CcdhString> a owl:Class,
        linkml:TypeDefinition ;
    rdfs:label "ccdh_string" ;
    rdfs:subClassOf linkml:String ;
    skos:definition "A sequence of Unicode characters.  There are no limits on the number of characters in the string." ;
    skos:editorialNote "Derived from [ccdh_string in sheet Primitives](https://docs.google.com/spreadsheets/d/1oWS7cao-fgz2MKWtyr8h2dEL9unX__0bJrWKv6mQmM4/edit#gid=497370447)" .

linkml:Date a owl:Class,
        linkml:TypeDefinition ;
    rdfs:label "date" ;
    rdfs:subClassOf [ a owl:Restriction ;
            owl:onDataRange xsd:date ;
            owl:onProperty linkml:topValue ;
            owl:qualifiedCardinality 1 ] ;
    skos:definition "a date (year, month and day) in an idealized calendar" ;
    skos:editorialNote "URI is dateTime because OWL reasoners don't work with straight date or time" .

linkml:Double a owl:Class,
        linkml:TypeDefinition ;
    rdfs:label "double" ;
    rdfs:subClassOf [ a owl:Restriction ;
            owl:onDataRange xsd:double ;
            owl:onProperty linkml:topValue ;
            owl:qualifiedCardinality 1 ] ;
    skos:definition "A real number that conforms to the xsd:double specification" .

linkml:Float a owl:Class,
        linkml:TypeDefinition ;
    rdfs:label "float" ;
    rdfs:subClassOf [ a owl:Restriction ;
            owl:onDataRange xsd:float ;
            owl:onProperty linkml:topValue ;
            owl:qualifiedCardinality 1 ] ;
    skos:definition "A real number that conforms to the xsd:float specification" .

linkml:Ncname a owl:Class,
        linkml:TypeDefinition ;
    rdfs:label "ncname" ;
    rdfs:subClassOf [ a owl:Restriction ;
            owl:onDataRange xsd:string ;
            owl:onProperty linkml:topValue ;
            owl:qualifiedCardinality 1 ] ;
    skos:definition "Prefix part of CURIE" .

linkml:Nodeidentifier a owl:Class,
        linkml:TypeDefinition ;
    rdfs:label "nodeidentifier" ;
    rdfs:subClassOf [ a owl:Restriction ;
            owl:onDataRange <http://www.w3.org/ns/shex#nonLiteral> ;
            owl:onProperty linkml:topValue ;
            owl:qualifiedCardinality 1 ] ;
    skos:definition "A URI, CURIE or BNODE that represents a node in a model." .

linkml:Objectidentifier a owl:Class,
        linkml:TypeDefinition ;
    rdfs:label "objectidentifier" ;
    rdfs:subClassOf [ a owl:Restriction ;
            owl:onDataRange <http://www.w3.org/ns/shex#iri> ;
            owl:onProperty linkml:topValue ;
            owl:qualifiedCardinality 1 ] ;
    skos:definition "A URI or CURIE that represents an object in the model." ;
    skos:note "Used for inheritence and type checking" .

linkml:SubsetDefinition a owl:Class ;
    rdfs:label "subset_definition" ;
    skos:definition "the name and description of a subset" .

linkml:Time a owl:Class,
        linkml:TypeDefinition ;
    rdfs:label "time" ;
    rdfs:subClassOf [ a owl:Restriction ;
            owl:onDataRange xsd:dateTime ;
            owl:onProperty linkml:topValue ;
            owl:qualifiedCardinality 1 ] ;
    skos:definition "A time object represents a (local) time of day, independent of any particular day" ;
    skos:editorialNote "URI is dateTime because OWL reasoners don't work with straight date or time" .

linkml:Uri a owl:Class,
        linkml:TypeDefinition ;
    rdfs:label "uri" ;
    rdfs:subClassOf [ a owl:Restriction ;
            owl:onDataRange xsd:anyURI ;
            owl:onProperty linkml:topValue ;
            owl:qualifiedCardinality 1 ] ;
    skos:definition "a complete URI" .

linkml:alcoholExposureObservation__category a owl:ObjectProperty,
        linkml:SlotDefinition ;
    rdfs:label "alcoholExposureObservation__category" ;
    rdfs:domain <https://example.org/crdch_model/AlcoholExposureObservation> ;
    rdfs:range <http://UNKNOWN.org/enum_CRDCH_AlcoholExposureObservation_category> ;
    skos:definition "The general category of observation described" ;
    skos:editorialNote "Cardinality: 0..0" ;
    linkml:examples "Example(value='', description=None)" .

linkml:alcoholExposureObservation__focus a owl:ObjectProperty,
        linkml:SlotDefinition ;
    rdfs:label "alcoholExposureObservation__focus" ;
    rdfs:domain <https://example.org/crdch_model/AlcoholExposureObservation> ;
    rdfs:range <https://example.org/crdch_model/Entity> ;
    skos:definition "The entity or entities directly observed/measured in generating an observation result." ;
    skos:editorialNote "Cardinality: 0..0" ;
    skos:note "The 'focus', 'subject', and 'specimen' fields are useful when data creators want an Observation object to stand on its own, so it can point back to the entities it is about.  These fields are not needed when an Observation is embedded in a Specimen or other entity, where focus, subject, and specimen can be determined from context. " ;
    linkml:examples "Example(value='', description=None)" .

linkml:alcoholExposureObservation__id a owl:ObjectProperty,
        linkml:SlotDefinition ;
    rdfs:label "alcoholExposureObservation__id" ;
    rdfs:domain <https://example.org/crdch_model/AlcoholExposureObservation> ;
    rdfs:range <https://example.org/crdch_model/Entity> ;
    skos:definition "The 'logical' identifier of the entity within the system of record.  The simple value of this attribute stands for an identifier of this data object within the system, it can be used as a reference from other objects within the same system (i.e. primary and foreign keys), and it should be unique per type of object. The same data object copied to a different system will likely have a different \"id\" in the new system since \"id\" values are system specific and do not represent persistent business identifiers. Business identifiers are assigned outside the information system and are captured in the \"identifier\" field. The \"id\" field is more likely to be a serially or randomly generated value that is assigned to the data object as it is created in a system." ;
    skos:editorialNote "Cardinality: 0..0" ;
    skos:note "FHIR naming conventions are followed here, where 'id' is used for logical identifiers, and 'identifier' for business identifiers.   The identified entity may have a different 'id' in a different system, and have many external business 'identifiers' associated with it. If an \"id\" value can also be considered to be a business identifier, and should be transmissible to other systems, it should be duplicated in the \"identifier\" attribute along with the additional metadata needed to give context to the value of \"id\". An entity in this model that does not have an \"id\" field is considered to be an embeddable entity that can not stand on its own. " ;
    linkml:examples "Example(value='', description=None)" .

linkml:alcoholExposureObservation__method_type a owl:ObjectProperty,
        linkml:SlotDefinition ;
    rdfs:label "alcoholExposureObservation__method_type" ;
    rdfs:domain <https://example.org/crdch_model/AlcoholExposureObservation> ;
    rdfs:range <http://UNKNOWN.org/enum_CRDCH_AlcoholExposureObservation_method_type> ;
    skos:definition "A type of method used in generating the Observation result." ;
    skos:editorialNote "Cardinality: 0..0" ;
    skos:note "This may be a type of observational, measurement, experimental, or computational method specifying how to generate data (e.g. 'manual counting', 'bright field microscopy',). Or a Guideline or SOP specifying how to interpret data and/or encode the result of an  Observation (e.g. a Cancer Staging system such as that defined by the AJCC, or variant interpretation guideline such as that provided by the ACMG)." ;
    linkml:examples "Example(value='', description=None)" .

linkml:alcoholExposureObservation__observation_type a owl:ObjectProperty,
        linkml:SlotDefinition ;
    rdfs:label "alcoholExposureObservation__observation_type" ;
    rdfs:domain <https://example.org/crdch_model/AlcoholExposureObservation> ;
    rdfs:range <http://UNKNOWN.org/enum_CRDCH_AlcoholExposureObservation_observation_type> ;
    skos:definition "The specific type of alcohol exposure observation made - i.e. the feature or characteristic that was observed, measured, estimated, etc.." ;
    skos:editorialNote "Cardinality: 1..1" ;
    skos:note "This field holds the 'key' in the core key-value pair comprised of the observation_type field and the relevant value(s) field." ;
    linkml:examples "Example(value='alcohol_days_per_week', description=None)",
        "Example(value='alcohol_drinks_per_day', description=None)",
        "Example(value='alcohol_history', description=None)",
        "Example(value='alcohol_intensity', description=None)" .

linkml:alcoholExposureObservation__performed_by a owl:ObjectProperty,
        linkml:SlotDefinition ;
    rdfs:label "alcoholExposureObservation__performed_by" ;
    rdfs:domain <https://example.org/crdch_model/AlcoholExposureObservation> ;
    rdfs:range <https://example.org/crdch_model/Organization> ;
    skos:definition "The organization or group that performed the observation activity." ;
    skos:editorialNote "Cardinality: 0..0" ;
    linkml:examples "Example(value='', description=None)" .

linkml:alcoholExposureObservation__subject a owl:ObjectProperty,
        linkml:SlotDefinition ;
    rdfs:label "alcoholExposureObservation__subject" ;
    rdfs:domain <https://example.org/crdch_model/AlcoholExposureObservation> ;
    rdfs:range <https://example.org/crdch_model/Subject> ;
    skos:definition "The patient that the observation is about (if not the direct focus).  e.g. observations are often made on specimens derived from a patient, or other entities related to a patient, that ultimately tell us something about the patient of interest." ;
    skos:editorialNote "Cardinality: 0..0" ;
    linkml:examples "Example(value='', description=None)" .

linkml:alcoholExposureObservation__valueCodeableConcept a owl:ObjectProperty,
        linkml:SlotDefinition ;
    rdfs:label "alcoholExposureObservation__valueCodeableConcept" ;
    rdfs:domain <https://example.org/crdch_model/AlcoholExposureObservation> ;
    rdfs:range <http://UNKNOWN.org/enum_CRDCH_AlcoholExposureObservation_valueCodeableConcept> ;
    skos:definition "The result of the observation, encoded as a CodeableConcept." ;
    skos:editorialNote "Cardinality: 0..1" ;
    skos:note "One and only one of the value(x) fields must be populated." ;
    linkml:examples "Example(value='', description=None)" .

linkml:alcoholExposureObservation__valueInteger a owl:ObjectProperty,
        linkml:SlotDefinition ;
    rdfs:label "alcoholExposureObservation__valueInteger" ;
    rdfs:domain <https://example.org/crdch_model/AlcoholExposureObservation> ;
    rdfs:range <https://example.org/crdch_model/Entity> ;
    skos:definition "The result of the observation, encoded as an integer." ;
    skos:editorialNote "Cardinality: 0..1" ;
    skos:note "One and only one of the value(x) fields must be populated." ;
    linkml:examples "Example(value='', description=None)" .

linkml:biologicProduct__description a owl:ObjectProperty,
        linkml:SlotDefinition ;
    rdfs:label "biologicProduct__description" ;
    rdfs:domain <https://example.org/crdch_model/BiologicProduct> ;
    rdfs:range <https://example.org/crdch_model/Entity> ;
    skos:definition "A free text field to capture additional info/explanation about the model system" ;
    skos:editorialNote "Cardinality: 0..1" ;
    linkml:examples "Example(value='', description=None)" .

linkml:biologicProduct__growth_rate a owl:ObjectProperty,
        linkml:SlotDefinition ;
    rdfs:label "biologicProduct__growth_rate" ;
    rdfs:domain <https://example.org/crdch_model/BiologicProduct> ;
    rdfs:range <https://example.org/crdch_model/Entity> ;
    skos:definition "When the specimen an actively growing model system, such as a cell or tissue culture, this property captures its rate of growth." ;
    linkml:examples "Example(value='', description=None)" .

linkml:biologicProduct__id a owl:ObjectProperty,
        linkml:SlotDefinition ;
    rdfs:label "biologicProduct__id" ;
    rdfs:domain <https://example.org/crdch_model/BiologicProduct> ;
    rdfs:range <https://example.org/crdch_model/Entity> ;
    skos:definition "The 'logical' identifier of the entity within the system of record.  The simple value of this attribute stands for an identifier of this data object within the system, it can be used as a reference from other objects within the same system (i.e. primary and foreign keys), and it should be unique per type of object. The same data object copied to a different system will likely have a different \"id\" in the new system since \"id\" values are system specific and do not represent persistent business identifiers. Business identifiers are assigned outside the information system and are captured in the \"identifier\" field. The \"id\" field is more likely to be a serially or randomly generated value that is assigned to the data object as it is created in a system." ;
    skos:editorialNote "Cardinality: 0..1" ;
    skos:note "FHIR naming conventions are followed here, where 'id' is used for logical identifiers, and 'identifier' for business identifiers.   The identified entity may have a different 'id' in a different system, and have many external business 'identifiers' associated with it. If an \"id\" value can also be considered to be a business identifier, and should be transmissible to other systems, it should be duplicated in the \"identifier\" attribute along with the additional metadata needed to give context to the value of \"id\". An entity in this model that does not have an \"id\" field is considered to be an embeddable entity that can not stand on its own. " ;
    linkml:examples "Example(value='', description=None)" .

linkml:biologicProduct__identifier a owl:ObjectProperty,
        linkml:SlotDefinition ;
    rdfs:label "biologicProduct__identifier" ;
    rdfs:domain <https://example.org/crdch_model/BiologicProduct> ;
    rdfs:range <https://example.org/crdch_model/Identifier> ;
    skos:definition "A 'business' identifier or accession number for the entity, typically as provided by an external system or authority, that are globally unique and persist across implementing systems. Also, since these identifiers are created outside the information system through a specific business process, the Identifier type has additional attributes to capture this additional metadata so the actual identifier values are qualified by the context that created those values. This additional context allows \"identifier\" instances to be transmitted as business data across systems while still being able to trace them back to the system of origin." ;
    skos:editorialNote "Cardinality: 0..m" ;
    skos:note "FHIR naming conventions are followed here, where 'id' is used for logical identifiers which are unique only within a given system, and 'identifier' for business identifiers, which are used to connect entities or share content across systems.  The complex 'Identifier' data type is used  to capture the identifier itself, along with metadata about its source." ;
    linkml:examples "Example(value='', description=None)" .

linkml:biologicProduct__passage_number a owl:ObjectProperty,
        linkml:SlotDefinition ;
    rdfs:label "biologicProduct__passage_number" ;
    rdfs:domain <https://example.org/crdch_model/BiologicProduct> ;
    rdfs:range <https://example.org/crdch_model/Entity> ;
    skos:definition "When the specimen an actively growing model system, such as a cell or tissue culture, this property captures its passage number." ;
    linkml:examples "Example(value='', description=None)" .

linkml:biologicProduct__product_type a owl:ObjectProperty,
        linkml:SlotDefinition ;
    rdfs:label "biologicProduct__product_type" ;
    rdfs:domain <https://example.org/crdch_model/BiologicProduct> ;
    rdfs:range <http://UNKNOWN.org/enum_CRDCH_BiologicProduct_product_type> ;
    skos:definition "The high level type of model system (e.g. cell line, cell culture, tissue culture, organoid)" ;
    skos:editorialNote "Cardinality: 0..1" ;
    linkml:examples "Example(value='cell culture', description=None)",
        "Example(value='cell line', description=None)",
        "Example(value='organoid', description=None)",
        "Example(value='tissue culture', description=None)" .

linkml:bodySite__qualifier a owl:ObjectProperty,
        linkml:SlotDefinition ;
    rdfs:label "bodySite__qualifier" ;
    rdfs:domain <https://example.org/crdch_model/BodySite> ;
    rdfs:range <http://UNKNOWN.org/enum_CRDCH_BodySite_qualifier> ;
    skos:definition "A qualifier that further refines or specifies the location of the body site (e.g. to indicate laterality, upper v. lower, containment, etc)." ;
    skos:editorialNote "Cardinality: 0..m" ;
    linkml:examples "Example(value='bilateral', description=None)",
        "Example(value='left', description=None)",
        "Example(value='right', description=None)" .

linkml:bodySite__site a owl:ObjectProperty,
        linkml:SlotDefinition ;
    rdfs:label "bodySite__site" ;
    rdfs:domain <https://example.org/crdch_model/BodySite> ;
    rdfs:range <http://UNKNOWN.org/enum_CRDCH_BodySite_site> ;
    skos:definition "A term describing any site in the body." ;
    skos:editorialNote "Cardinality: 1..1" ;
    linkml:examples "Example(value='Adenoid', description=None)",
        "Example(value='Adipose', description=None)",
        "Example(value='Adrenal', description=None)" .

linkml:cancerGradeObservationSet__category a owl:ObjectProperty,
        linkml:SlotDefinition ;
    rdfs:label "cancerGradeObservationSet__category" ;
    rdfs:domain <https://example.org/crdch_model/CancerGradeObservationSet> ;
    rdfs:range <http://UNKNOWN.org/enum_CRDCH_CancerGradeObservationSet_category> ;
    skos:definition "The general category of observation set described" ;
    skos:editorialNote "Cardinality: 0..0" ;
    skos:note "FHIR naming conventions are followed here, where 'id' is used for logical identifiers which are unique only within a given system, and 'identifier' for business identifiers, which are used to connect entities or share content across systems.  The complex 'Identifier' data type is used  to capture the identifier itself, along with metadata about its source." ;
    linkml:examples "Example(value='', description=None)" .

linkml:cancerGradeObservationSet__focus a owl:ObjectProperty,
        linkml:SlotDefinition ;
    rdfs:label "cancerGradeObservationSet__focus" ;
    rdfs:domain <https://example.org/crdch_model/CancerGradeObservationSet> ;
    rdfs:range <https://example.org/crdch_model/Entity> ;
    skos:definition "The entity or entities directly observed/measured in generating an observation result." ;
    skos:editorialNote "Cardinality: 0..m" ;
    skos:note "The 'focus', 'subject', and 'specimen' fields are useful when data creators want an Observation object to stand on its own, so it can point back to the entities it is about.  These fields are not needed when an Observation is embedded in a Specimen or other entity, where focus, subject, and specimen can be determined from context. " ;
    linkml:examples "Example(value='', description=None)" .

linkml:cancerGradeObservationSet__id a owl:ObjectProperty,
        linkml:SlotDefinition ;
    rdfs:label "cancerGradeObservationSet__id" ;
    rdfs:domain <https://example.org/crdch_model/CancerGradeObservationSet> ;
    rdfs:range <https://example.org/crdch_model/Entity> ;
    skos:definition "The 'logical' identifier of the entity within the system of record.  The simple value of this attribute stands for an identifier of this data object within the system, it can be used as a reference from other objects within the same system (i.e. primary and foreign keys), and it should be unique per type of object. The same data object copied to a different system will likely have a different \"id\" in the new system since \"id\" values are system specific and do not represent persistent business identifiers. Business identifiers are assigned outside the information system and are captured in the \"identifier\" field. The \"id\" field is more likely to be a serially or randomly generated value that is assigned to the data object as it is created in a system." ;
    skos:editorialNote "Cardinality: 0..0" ;
    skos:note "FHIR naming conventions are followed here, where 'id' is used for logical identifiers, and 'identifier' for business identifiers.   The identified entity may have a different 'id' in a different system, and have many external business 'identifiers' associated with it. If an \"id\" value can also be considered to be a business identifier, and should be transmissible to other systems, it should be duplicated in the \"identifier\" attribute along with the additional metadata needed to give context to the value of \"id\". An entity in this model that does not have an \"id\" field is considered to be an embeddable entity that can not stand on its own. " ;
    linkml:examples "Example(value='', description=None)" .

linkml:cancerGradeObservationSet__method_type a owl:ObjectProperty,
        linkml:SlotDefinition ;
    rdfs:label "cancerGradeObservationSet__method_type" ;
    rdfs:domain <https://example.org/crdch_model/CancerGradeObservationSet> ;
    rdfs:range <http://UNKNOWN.org/enum_CRDCH_CancerGradeObservationSet_method_type> ;
    skos:definition "The cancer grade classification system being used to classify the cancer (e.g. INPC, Gleason, etc.)" ;
    skos:editorialNote "Cardinality: 0..m" ;
    skos:note "This may be a type of observational, measurement, experimental, or computational method specifying how to generate data (e.g. 'manual counting', 'bright field microscopy'). Or a Guideline or SOP specifying how to interpret data and/or encode the result of an  Observation (e.g. a Cancer Staging system such as that defined by the AJCC, or variant interpretation guideline such as that provided by the ACMG)." ;
    linkml:examples "Example(value='Gleason', description=None)",
        "Example(value='INPC', description=None)",
        "Example(value='Unspecified grading system', description=None)" .

linkml:cancerGradeObservationSet__observations a owl:ObjectProperty,
        linkml:SlotDefinition ;
    rdfs:label "cancerGradeObservationSet__observations" ;
    rdfs:domain <https://example.org/crdch_model/CancerGradeObservationSet> ;
    rdfs:range <https://example.org/crdch_model/CancerGradeObservation> ;
    skos:definition "A set of one or more more atomic observations about the cancer grade that classifies the cancer (e.g. Poorly differentiated, differentiated, etc.)" ;
    skos:editorialNote "Cardinality: 0..m" ;
    linkml:examples "Example(value='', description=None)" .

linkml:cancerGradeObservationSet__performed_by a owl:ObjectProperty,
        linkml:SlotDefinition ;
    rdfs:label "cancerGradeObservationSet__performed_by" ;
    rdfs:domain <https://example.org/crdch_model/CancerGradeObservationSet> ;
    rdfs:range <https://example.org/crdch_model/Organization> ;
    skos:definition "The organization or group that performed the observation activity." ;
    skos:editorialNote "Cardinality: 0..1" ;
    linkml:examples "Example(value='', description=None)" .

linkml:cancerGradeObservationSet__subject a owl:ObjectProperty,
        linkml:SlotDefinition ;
    rdfs:label "cancerGradeObservationSet__subject" ;
    rdfs:domain <https://example.org/crdch_model/CancerGradeObservationSet> ;
    rdfs:range <https://example.org/crdch_model/Subject> ;
    skos:definition "The patient that the observation is about (if not the direct focus).  e.g. observations are often made on specimens derived from a patient, or other entities related to a patient, that ultimately tell us something about the patient of interest." ;
    skos:editorialNote "Cardinality: 0..1" ;
    linkml:examples "Example(value='', description=None)" .

linkml:cancerGradeObservation__category a owl:ObjectProperty,
        linkml:SlotDefinition ;
    rdfs:label "cancerGradeObservation__category" ;
    rdfs:domain <https://example.org/crdch_model/CancerGradeObservation> ;
    rdfs:range <http://UNKNOWN.org/enum_CRDCH_CancerGradeObservation_category> ;
    skos:definition "The general category of observation described" ;
    skos:editorialNote "Cardinality: 0..0" ;
    linkml:examples "Example(value='', description=None)" .

linkml:cancerGradeObservation__focus a owl:ObjectProperty,
        linkml:SlotDefinition ;
    rdfs:label "cancerGradeObservation__focus" ;
    rdfs:domain <https://example.org/crdch_model/CancerGradeObservation> ;
    rdfs:range <https://example.org/crdch_model/Entity> ;
    skos:definition "The entity or entities directly observed/measured in generating an observation result." ;
    skos:editorialNote "Cardinality: 0..0" ;
    skos:note "The 'focus', 'subject', and 'specimen' fields are useful when data creators want an Observation object to stand on its own, so it can point back to the entities it is about.  These fields are not needed when an Observation is embedded in a Specimen or other entity, where focus, subject, and specimen can be determined from context. " ;
    linkml:examples "Example(value='', description=None)" .

linkml:cancerGradeObservation__id a owl:ObjectProperty,
        linkml:SlotDefinition ;
    rdfs:label "cancerGradeObservation__id" ;
    rdfs:domain <https://example.org/crdch_model/CancerGradeObservation> ;
    rdfs:range <https://example.org/crdch_model/Entity> ;
    skos:definition "The 'logical' identifier of the entity within the system of record.  The simple value of this attribute stands for an identifier of this data object within the system, it can be used as a reference from other objects within the same system (i.e. primary and foreign keys), and it should be unique per type of object. The same data object copied to a different system will likely have a different \"id\" in the new system since \"id\" values are system specific and do not represent persistent business identifiers. Business identifiers are assigned outside the information system and are captured in the \"identifier\" field. The \"id\" field is more likely to be a serially or randomly generated value that is assigned to the data object as it is created in a system." ;
    skos:editorialNote "Cardinality: 0..0" ;
    skos:note "FHIR naming conventions are followed here, where 'id' is used for logical identifiers, and 'identifier' for business identifiers.   The identified entity may have a different 'id' in a different system, and have many external business 'identifiers' associated with it. If an \"id\" value can also be considered to be a business identifier, and should be transmissible to other systems, it should be duplicated in the \"identifier\" attribute along with the additional metadata needed to give context to the value of \"id\". An entity in this model that does not have an \"id\" field is considered to be an embeddable entity that can not stand on its own. " ;
    linkml:examples "Example(value='', description=None)" .

linkml:cancerGradeObservation__method_type a owl:ObjectProperty,
        linkml:SlotDefinition ;
    rdfs:label "cancerGradeObservation__method_type" ;
    rdfs:domain <https://example.org/crdch_model/CancerGradeObservation> ;
    rdfs:range <http://UNKNOWN.org/enum_CRDCH_CancerGradeObservation_method_type> ;
    skos:definition "A type of method used in generating the Observation result." ;
    skos:editorialNote "Cardinality: 0..0" ;
    skos:note "This may be a type of observational, measurement, experimental, or computational method specifying how to generate data (e.g. 'manual counting', 'bright field microscopy',). Or a Guideline or SOP specifying how to interpret data and/or encode the result of an  Observation (e.g. a Cancer Staging system such as that defined by the AJCC, or variant interpretation guideline such as that provided by the ACMG)." ;
    linkml:examples "Example(value='', description=None)" .

linkml:cancerGradeObservation__observation_type a owl:ObjectProperty,
        linkml:SlotDefinition ;
    rdfs:label "cancerGradeObservation__observation_type" ;
    rdfs:domain <https://example.org/crdch_model/CancerGradeObservation> ;
    rdfs:range <http://UNKNOWN.org/enum_CRDCH_CancerGradeObservation_observation_type> ;
    skos:definition "The cancer grade classification system being used to classify the cancer (e.g. INPC, Gleason, etc.)" ;
    skos:editorialNote "Cardinality: 1..1" ;
    skos:note "This field holds the 'key' in the core key-value pair comprised of the observation_type field and the relevant value(s) field.  " ;
    linkml:examples "Example(value='enneking_msts_grade', description=None)",
        "Example(value='esophageal_columnar_dysplasia_degree', description=None)",
        "Example(value='gleason_grade_group', description=None)",
        "Example(value='inpc_grade', description=None)",
        "Example(value='primary_gleason_grade', description=None)",
        "Example(value='secondary_gleason_grade', description=None)",
        "Example(value='tumor_grade', description=None)" .

linkml:cancerGradeObservation__subject a owl:ObjectProperty,
        linkml:SlotDefinition ;
    rdfs:label "cancerGradeObservation__subject" ;
    rdfs:domain <https://example.org/crdch_model/CancerGradeObservation> ;
    rdfs:range <https://example.org/crdch_model/Subject> ;
    skos:definition "The patient that the observation is about (if not the direct focus).  e.g. observations are often made on specimens derived from a patient, or other entities related to a patient, that ultimately tell us something about the patient of interest." ;
    skos:editorialNote "Cardinality: 0..0" ;
    linkml:examples "Example(value='', description=None)" .

linkml:cancerGradeObservation__valueCodeableConcept a owl:ObjectProperty,
        linkml:SlotDefinition ;
    rdfs:label "cancerGradeObservation__valueCodeableConcept" ;
    rdfs:domain <https://example.org/crdch_model/CancerGradeObservation> ;
    rdfs:range <http://UNKNOWN.org/enum_CRDCH_CancerGradeObservation_valueCodeableConcept> ;
    skos:definition "The value from the grade classification system that classifies the cancer (e.g. Poorly differentiated, differentiated, etc.)" ;
    skos:editorialNote "Cardinality: 1..1" ;
    skos:note "One and only one of the value(x) fields must be populated." ;
    linkml:examples "Example(value='', description=None)" .

linkml:cancerStageObservationSet__category a owl:ObjectProperty,
        linkml:SlotDefinition ;
    rdfs:label "cancerStageObservationSet__category" ;
    rdfs:domain <https://example.org/crdch_model/CancerStageObservationSet> ;
    rdfs:range <http://UNKNOWN.org/enum_CRDCH_CancerStageObservationSet_category> ;
    skos:definition "The general category of observation set described" ;
    skos:editorialNote "Cardinality: 0..0" ;
    skos:note "FHIR naming conventions are followed here, where 'id' is used for logical identifiers which are unique only within a given system, and 'identifier' for business identifiers, which are used to connect entities or share content across systems.  The complex 'Identifier' data type is used  to capture the identifier itself, along with metadata about its source." ;
    linkml:examples "Example(value='', description=None)" .

linkml:cancerStageObservationSet__focus a owl:ObjectProperty,
        linkml:SlotDefinition ;
    rdfs:label "cancerStageObservationSet__focus" ;
    rdfs:domain <https://example.org/crdch_model/CancerStageObservationSet> ;
    rdfs:range <https://example.org/crdch_model/Entity> ;
    skos:definition "The entity or entities directly observed/measured in generating an observation result." ;
    skos:editorialNote "Cardinality: 0..m" ;
    skos:note "The 'focus', 'subject', and 'specimen' fields are useful when data creators want an Observation object to stand on its own, so it can point back to the entities it is about.  These fields are not needed when an Observation is embedded in a Specimen or other entity, where focus, subject, and specimen can be determined from context. " ;
    linkml:examples "Example(value='', description=None)" .

linkml:cancerStageObservationSet__id a owl:ObjectProperty,
        linkml:SlotDefinition ;
    rdfs:label "cancerStageObservationSet__id" ;
    rdfs:domain <https://example.org/crdch_model/CancerStageObservationSet> ;
    rdfs:range <https://example.org/crdch_model/Entity> ;
    skos:definition "The 'logical' identifier of the entity within the system of record.  The simple value of this attribute stands for an identifier of this data object within the system, it can be used as a reference from other objects within the same system (i.e. primary and foreign keys), and it should be unique per type of object. The same data object copied to a different system will likely have a different \"id\" in the new system since \"id\" values are system specific and do not represent persistent business identifiers. Business identifiers are assigned outside the information system and are captured in the \"identifier\" field. The \"id\" field is more likely to be a serially or randomly generated value that is assigned to the data object as it is created in a system." ;
    skos:editorialNote "Cardinality: 0..0" ;
    skos:note "FHIR naming conventions are followed here, where 'id' is used for logical identifiers, and 'identifier' for business identifiers.   The identified entity may have a different 'id' in a different system, and have many external business 'identifiers' associated with it. If an \"id\" value can also be considered to be a business identifier, and should be transmissible to other systems, it should be duplicated in the \"identifier\" attribute along with the additional metadata needed to give context to the value of \"id\". An entity in this model that does not have an \"id\" field is considered to be an embeddable entity that can not stand on its own. " ;
    linkml:examples "Example(value='', description=None)" .

linkml:cancerStageObservationSet__method_type a owl:ObjectProperty,
        linkml:SlotDefinition ;
    rdfs:label "cancerStageObservationSet__method_type" ;
    rdfs:domain <https://example.org/crdch_model/CancerStageObservationSet> ;
    rdfs:range <http://UNKNOWN.org/enum_CRDCH_CancerStageObservationSet_method_type> ;
    skos:definition "A type of method used in generating each of the Observations bundled in the set, in this case, the particular staging system being used to classify the cancer." ;
    skos:editorialNote "Cardinality: 0..m" ;
    skos:note "This may be a type of observational, measurement, experimental, or computational method specifying how to generate data (e.g. 'manual counting', 'bright field microscopy'). Or a Guideline or SOP specifying how to interpret data and/or encode the result of an  Observation (e.g. a Cancer Staging system such as that defined by the AJCC, or variant interpretation guideline such as that provided by the ACMG)." ;
    linkml:examples "Example(value='AJCC staging system 1st edition', description=None)",
        "Example(value='AJCC staging system 2nd edition', description=None)",
        "Example(value='AJCC staging system 3rd edition', description=None)",
        "Example(value='AJCC staging system 4th edition', description=None)",
        "Example(value='AJCC staging system 5th edition', description=None)",
        "Example(value='AJCC staging system 6th edition', description=None)",
        "Example(value='AJCC staging system 7th edition', description=None)",
        "Example(value='AJCC staging system 8th edition', description=None)",
        "Example(value='Ann Arbor staging system', description=None)",
        "Example(value='COG Liver staging system', description=None)",
        "Example(value='COG Renal staging system', description=None)",
        "Example(value='Enneking MSTS staging system', description=None)",
        "Example(value='FIGO staging system', description=None)",
        "Example(value='IGCCCG staging system', description=None)",
        "Example(value='INRG staging system', description=None)",
        "Example(value='INSS staging system', description=None)",
        "Example(value='IRS staging system', description=None)",
        "Example(value='ISS staging system', description=None)",
        "Example(value='Masaoka staging system', description=None)",
        "Example(value='Unspecified staging system', description=None)" .

linkml:cancerStageObservationSet__observations a owl:ObjectProperty,
        linkml:SlotDefinition ;
    rdfs:label "cancerStageObservationSet__observations" ;
    rdfs:domain <https://example.org/crdch_model/CancerStageObservationSet> ;
    rdfs:range <https://example.org/crdch_model/CancerStageObservation> ;
    skos:definition "A set of one or more more atomic observations about the cancer stage" ;
    skos:editorialNote "Cardinality: 0..m" ;
    linkml:examples "Example(value='', description=None)" .

linkml:cancerStageObservationSet__performed_by a owl:ObjectProperty,
        linkml:SlotDefinition ;
    rdfs:label "cancerStageObservationSet__performed_by" ;
    rdfs:domain <https://example.org/crdch_model/CancerStageObservationSet> ;
    rdfs:range <https://example.org/crdch_model/Organization> ;
    skos:definition "The organization or group that performed the observation activity." ;
    skos:editorialNote "Cardinality: 0..1" ;
    linkml:examples "Example(value='', description=None)" .

linkml:cancerStageObservationSet__subject a owl:ObjectProperty,
        linkml:SlotDefinition ;
    rdfs:label "cancerStageObservationSet__subject" ;
    rdfs:domain <https://example.org/crdch_model/CancerStageObservationSet> ;
    rdfs:range <https://example.org/crdch_model/Subject> ;
    skos:definition "The patient that the observation is about (if not the direct focus).  e.g. observations are often made on specimens derived from a patient, or other entities related to a patient, that ultimately tell us something about the patient of interest." ;
    skos:editorialNote "Cardinality: 0..1" ;
    linkml:examples "Example(value='', description=None)" .

linkml:cancerStageObservation__category a owl:ObjectProperty,
        linkml:SlotDefinition ;
    rdfs:label "cancerStageObservation__category" ;
    rdfs:domain <https://example.org/crdch_model/CancerStageObservation> ;
    rdfs:range <http://UNKNOWN.org/enum_CRDCH_CancerStageObservation_category> ;
    skos:definition "The general category of observation described" ;
    skos:editorialNote "Cardinality: 0..0" ;
    linkml:examples "Example(value='', description=None)" .

linkml:cancerStageObservation__focus a owl:ObjectProperty,
        linkml:SlotDefinition ;
    rdfs:label "cancerStageObservation__focus" ;
    rdfs:domain <https://example.org/crdch_model/CancerStageObservation> ;
    rdfs:range <https://example.org/crdch_model/Entity> ;
    skos:definition "The entity or entities directly observed/measured in generating an observation result." ;
    skos:editorialNote "Cardinality: 0..0" ;
    skos:note "The 'focus', 'subject', and 'specimen' fields are useful when data creators want an Observation object to stand on its own, so it can point back to the entities it is about.  These fields are not needed when an Observation is embedded in a Specimen or other entity, where focus, subject, and specimen can be determined from context. " ;
    linkml:examples "Example(value='', description=None)" .

linkml:cancerStageObservation__id a owl:ObjectProperty,
        linkml:SlotDefinition ;
    rdfs:label "cancerStageObservation__id" ;
    rdfs:domain <https://example.org/crdch_model/CancerStageObservation> ;
    rdfs:range <https://example.org/crdch_model/Entity> ;
    skos:definition "The 'logical' identifier of the entity within the system of record.  The simple value of this attribute stands for an identifier of this data object within the system, it can be used as a reference from other objects within the same system (i.e. primary and foreign keys), and it should be unique per type of object. The same data object copied to a different system will likely have a different \"id\" in the new system since \"id\" values are system specific and do not represent persistent business identifiers. Business identifiers are assigned outside the information system and are captured in the \"identifier\" field. The \"id\" field is more likely to be a serially or randomly generated value that is assigned to the data object as it is created in a system." ;
    skos:editorialNote "Cardinality: 0..0" ;
    skos:note "FHIR naming conventions are followed here, where 'id' is used for logical identifiers, and 'identifier' for business identifiers.   The identified entity may have a different 'id' in a different system, and have many external business 'identifiers' associated with it. If an \"id\" value can also be considered to be a business identifier, and should be transmissible to other systems, it should be duplicated in the \"identifier\" attribute along with the additional metadata needed to give context to the value of \"id\". An entity in this model that does not have an \"id\" field is considered to be an embeddable entity that can not stand on its own. " ;
    linkml:examples "Example(value='', description=None)" .

linkml:cancerStageObservation__method_type a owl:ObjectProperty,
        linkml:SlotDefinition ;
    rdfs:label "cancerStageObservation__method_type" ;
    rdfs:domain <https://example.org/crdch_model/CancerStageObservation> ;
    rdfs:range <http://UNKNOWN.org/enum_CRDCH_CancerStageObservation_method_type> ;
    skos:definition "A type of method used in generating the Observation result." ;
    skos:editorialNote "Cardinality: 0..0" ;
    skos:note "This may be a type of observational, measurement, experimental, or computational method specifying how to generate data (e.g. 'manual counting', 'bright field microscopy',). Or a Guideline or SOP specifying how to interpret data and/or encode the result of an  Observation (e.g. a Cancer Staging system such as that defined by the AJCC, or variant interpretation guideline such as that provided by the ACMG)." ;
    linkml:examples "Example(value='', description=None)" .

linkml:cancerStageObservation__observation_type a owl:ObjectProperty,
        linkml:SlotDefinition ;
    rdfs:label "cancerStageObservation__observation_type" ;
    rdfs:domain <https://example.org/crdch_model/CancerStageObservation> ;
    rdfs:range <http://UNKNOWN.org/enum_CRDCH_CancerStageObservation_observation_type> ;
    skos:definition "The type of cancer staging component being represented (e.g. 'Clinical Metastasis (M)')" ;
    skos:editorialNote "Cardinality: 1..1" ;
    skos:note "This field holds the 'key' in the core key-value pair comprised of the observation_type field and the relevant value(s) field.  'Overall' should be used when: the source staging value is not definitively 'Clinical' or 'Pathological' (e.g. a TNM staged cancer without a clear indication of clinical vs pathological), or the source staging system does not use T, N, or M components and only has a single overall staging value (e.g. FIGO staging)" ;
    linkml:examples "Example(value='Ann Arbor Modifier', description=None)",
        "Example(value='Clinical Metastasis (M)', description=None)",
        "Example(value='Clinical Node (N)', description=None)",
        "Example(value='Clinical Overall', description=None)",
        "Example(value='Clinical Tumor (T)', description=None)",
        "Example(value='Metastasis (M)', description=None)",
        "Example(value='Node (N)', description=None)",
        "Example(value='Overall', description=None)",
        "Example(value='Pathological Metastasis (M)', description=None)",
        "Example(value='Pathological Node (N)', description=None)",
        "Example(value='Pathological Overall', description=None)",
        "Example(value='Pathological Tumor (T)', description=None)",
        "Example(value='Tumor (T)', description=None)" .

linkml:cancerStageObservation__performed_by a owl:ObjectProperty,
        linkml:SlotDefinition ;
    rdfs:label "cancerStageObservation__performed_by" ;
    rdfs:domain <https://example.org/crdch_model/CancerStageObservation> ;
    rdfs:range <https://example.org/crdch_model/Organization> ;
    skos:definition "The organization or group that performed the observation activity." ;
    skos:editorialNote "Cardinality: 0..0" ;
    linkml:examples "Example(value='', description=None)" .

linkml:cancerStageObservation__subject a owl:ObjectProperty,
        linkml:SlotDefinition ;
    rdfs:label "cancerStageObservation__subject" ;
    rdfs:domain <https://example.org/crdch_model/CancerStageObservation> ;
    rdfs:range <https://example.org/crdch_model/Subject> ;
    skos:definition "The patient that the observation is about (if not the direct focus).  e.g. observations are often made on specimens derived from a patient, or other entities related to a patient, that ultimately tell us something about the patient of interest." ;
    skos:editorialNote "Cardinality: 0..0" ;
    linkml:examples "Example(value='', description=None)" .

linkml:cancerStageObservation__valueCodeableConcept a owl:ObjectProperty,
        linkml:SlotDefinition ;
    rdfs:label "cancerStageObservation__valueCodeableConcept" ;
    rdfs:domain <https://example.org/crdch_model/CancerStageObservation> ;
    rdfs:range <http://UNKNOWN.org/enum_CRDCH_CancerStageObservation_valueCodeableConcept> ;
    skos:definition "The value for a cancer staging component being represented (e.g. 'M1'), encoded as a CodeableConcept." ;
    skos:editorialNote "Cardinality: 1..1" ;
    skos:note "One and only one of the value(x) fields must be populated." ;
    linkml:examples "Example(value='M0', description=None)",
        "Example(value='M1', description=None)",
        "Example(value='M1a', description=None)",
        "Example(value='N0 (i+)', description=None)",
        "Example(value='N0 (i-)', description=None)",
        "Example(value='N0', description=None)" .

linkml:cancerStageObservation__valueEntity a owl:ObjectProperty,
        linkml:SlotDefinition ;
    rdfs:label "cancerStageObservation__valueEntity" ;
    rdfs:domain <https://example.org/crdch_model/CancerStageObservation> ;
    rdfs:range <https://example.org/crdch_model/Entity> ;
    skos:definition "The value of an observation" ;
    skos:editorialNote "Cardinality: 0..0" ;
    linkml:examples "Example(value='', description=None)" .

linkml:codeableConcept__coding a owl:ObjectProperty,
        linkml:SlotDefinition ;
    rdfs:label "codeableConcept__coding" ;
    rdfs:domain <https://example.org/crdch_model/CodeableConcept> ;
    rdfs:range <https://example.org/crdch_model/Coding> ;
    skos:definition "A reference to a code defined by a terminology system" ;
    skos:editorialNote "Cardinality: 0..m" ;
    linkml:examples "Example(value='', description=None)" .

linkml:codeableConcept__text a owl:ObjectProperty,
        linkml:SlotDefinition ;
    rdfs:label "codeableConcept__text" ;
    rdfs:domain <https://example.org/crdch_model/CodeableConcept> ;
    rdfs:range <https://example.org/crdch_model/Entity> ;
    skos:definition "A human language representation of the concept represented by the Coding." ;
    skos:editorialNote "Cardinality: 0..1" ;
    skos:note "The text attribute represents the concept as entered or chosen by the user; often the value of text is the same as a display of one of the codings.  A concept that does not have an appropriate or known coding can be represented using free-text in the text attribute. " ;
    linkml:examples "Example(value='', description=None)" .

linkml:coding__code a owl:ObjectProperty,
        linkml:SlotDefinition ;
    rdfs:label "coding__code" ;
    rdfs:domain <https://example.org/crdch_model/Coding> ;
    rdfs:range <https://example.org/crdch_model/Entity> ;
    skos:definition "The symbol/value of the code, as defined by the code system." ;
    skos:editorialNote "Cardinality: 1..1" ;
    linkml:examples "Example(value='', description=None)" .

linkml:coding__label a owl:ObjectProperty,
        linkml:SlotDefinition ;
    rdfs:label "coding__label" ;
    rdfs:domain <https://example.org/crdch_model/Coding> ;
    rdfs:range <https://example.org/crdch_model/Entity> ;
    skos:definition "A human-readable name for the code, as defined by the code system." ;
    skos:editorialNote "Cardinality: 0..1" ;
    linkml:examples "Example(value='', description=None)" .

linkml:coding__system a owl:ObjectProperty,
        linkml:SlotDefinition ;
    rdfs:label "coding__system" ;
    rdfs:domain <https://example.org/crdch_model/Coding> ;
    rdfs:range <https://example.org/crdch_model/Entity> ;
    skos:definition "The code system where the code is defined." ;
    skos:editorialNote "Cardinality: 1..1" ;
    linkml:examples "Example(value='', description=None)" .

linkml:coding__systemURL a owl:ObjectProperty,
        linkml:SlotDefinition ;
    rdfs:label "coding__systemURL" ;
    rdfs:domain <https://example.org/crdch_model/Coding> ;
    rdfs:range <https://example.org/crdch_model/Entity> ;
    skos:definition "A URL where the code system can be found." ;
    skos:editorialNote "Cardinality: 0..1" ;
    linkml:examples "Example(value='', description=None)" .

linkml:coding__systemVersion a owl:ObjectProperty,
        linkml:SlotDefinition ;
    rdfs:label "coding__systemVersion" ;
    rdfs:domain <https://example.org/crdch_model/Coding> ;
    rdfs:range <https://example.org/crdch_model/Entity> ;
    skos:definition "The version of the code system." ;
    skos:editorialNote "Cardinality: 0..1" ;
    linkml:examples "Example(value='', description=None)" .

linkml:diagnosis__age_at_diagnosis a owl:ObjectProperty,
        linkml:SlotDefinition ;
    rdfs:label "diagnosis__age_at_diagnosis" ;
    rdfs:domain <https://example.org/crdch_model/Diagnosis> ;
    rdfs:range <https://example.org/crdch_model/Quantity> ;
    skos:definition "The age in days of the individual at the time of diagnosis" ;
    skos:editorialNote "Cardinality: 0..1" ;
    linkml:examples "Example(value='', description=None)" .

linkml:diagnosis__condition a owl:ObjectProperty,
        linkml:SlotDefinition ;
    rdfs:label "diagnosis__condition" ;
    rdfs:domain <https://example.org/crdch_model/Diagnosis> ;
    rdfs:range <http://UNKNOWN.org/enum_CRDCH_Diagnosis_condition> ;
    skos:definition "Code that captures the condition being diagnosed (e.g. ICD-O, ICD-10, SNOMED, etc.)" ;
    skos:editorialNote "Cardinality: 0..1" ;
    skos:note "This attribute will subsume source attributes that are bound to ICD-O and ICD-10 classification systems." ;
    linkml:examples "Example(value='', description=None)" .

linkml:diagnosis__disease_status a owl:ObjectProperty,
        linkml:SlotDefinition ;
    rdfs:label "diagnosis__disease_status" ;
    rdfs:domain <https://example.org/crdch_model/Diagnosis> ;
    rdfs:range <http://UNKNOWN.org/enum_CRDCH_Diagnosis_disease_status> ;
    skos:definition "A term that refers to the nature and/or clinical outcome of a disease (e.g., primary disease, metastatic disease, recurrent disease, etc.)" ;
    skos:editorialNote "Cardinality: 0..1" ;
    linkml:examples "Example(value='Initial Diagnosis', description=None)",
        "Example(value='Not Reported', description=None)",
        "Example(value='Progressive Disease', description=None)",
        "Example(value='Recurrent Disease', description=None)",
        "Example(value='Residual Disease', description=None)",
        "Example(value='Unknown', description=None)" .

linkml:diagnosis__grade a owl:ObjectProperty,
        linkml:SlotDefinition ;
    rdfs:label "diagnosis__grade" ;
    rdfs:domain <https://example.org/crdch_model/Diagnosis> ;
    rdfs:range <https://example.org/crdch_model/CancerGradeObservationSet> ;
    skos:definition "The degree of abnormality of cancer cells, a measure of differentiation, the extent to which cancer cells are similar in appearance and function to healthy cells of the same tissue type. The degree of differentiation often relates to the clinical behavior of the particular tumor. Based on the microscopic findings, tumor grade is commonly described by one of four degrees of severity. Histopathologic grade of a tumor may be used to plan treatment and estimate the future course, outcome, and overall prognosis of disease. Certain types of cancers, such as soft tissue sarcoma, primary brain tumors, lymphomas, and breast have special grading systems." ;
    skos:editorialNote "Cardinality: 0..m" ;
    linkml:examples "Example(value='', description=None)" .

linkml:diagnosis__id a owl:ObjectProperty,
        linkml:SlotDefinition ;
    rdfs:label "diagnosis__id" ;
    rdfs:domain <https://example.org/crdch_model/Diagnosis> ;
    rdfs:range <https://example.org/crdch_model/Entity> ;
    skos:definition "The 'logical' identifier of the entity within the system of record.  The simple value of this attribute stands for an identifier of this data object within the system, it can be used as a reference from other objects within the same system (i.e. primary and foreign keys), and it should be unique per type of object. The same data object copied to a different system will likely have a different \"id\" in the new system since \"id\" values are system specific and do not represent persistent business identifiers. Business identifiers are assigned outside the information system and are captured in the \"identifier\" field. The \"id\" field is more likely to be a serially or randomly generated value that is assigned to the data object as it is created in a system." ;
    skos:editorialNote "Cardinality: 0..1" ;
    skos:note "FHIR naming conventions are followed here, where 'id' is used for logical identifiers, and 'identifier' for business identifiers.   The identified entity may have a different 'id' in a different system, and have many external business 'identifiers' associated with it. If an \"id\" value can also be considered to be a business identifier, and should be transmissible to other systems, it should be duplicated in the \"identifier\" attribute along with the additional metadata needed to give context to the value of \"id\". An entity in this model that does not have an \"id\" field is considered to be an embeddable entity that can not stand on its own. " ;
    linkml:examples "Example(value='', description=None)" .

linkml:diagnosis__identifier a owl:ObjectProperty,
        linkml:SlotDefinition ;
    rdfs:label "diagnosis__identifier" ;
    rdfs:domain <https://example.org/crdch_model/Diagnosis> ;
    rdfs:range <https://example.org/crdch_model/Identifier> ;
    skos:definition "A 'business' identifier or accession number for the entity, typically as provided by an external system or authority, that are globally unique and persist across implementing systems. Also, since these identifiers are created outside the information system through a specific business process, the Identifier type has additional attributes to capture this additional metadata so the actual identifier values are qualified by the context that created those values. This additional context allows \"identifier\" instances to be transmitted as business data across systems while still being able to trace them back to the system of origin." ;
    skos:editorialNote "Cardinality: 0..m" ;
    skos:note "FHIR naming conventions are followed here, where 'id' is used for logical identifiers which are unique only within a given system, and 'identifier' for business identifiers, which are used to connect entities or share content across systems.  The complex 'Identifier' data type is used  to capture the identifier itself, along with metadata about its source." ;
    linkml:examples "Example(value='', description=None)" .

linkml:diagnosis__metastatic_site a owl:ObjectProperty,
        linkml:SlotDefinition ;
    rdfs:label "diagnosis__metastatic_site" ;
    rdfs:domain <https://example.org/crdch_model/Diagnosis> ;
    rdfs:range <https://example.org/crdch_model/BodySite> ;
    skos:definition "The anatomical location(s) of metastatic disease" ;
    skos:editorialNote "Cardinality: 0..m" ;
    linkml:examples "Example(value='', description=None)" .

linkml:diagnosis__method_of_diagnosis a owl:ObjectProperty,
        linkml:SlotDefinition ;
    rdfs:label "diagnosis__method_of_diagnosis" ;
    rdfs:domain <https://example.org/crdch_model/Diagnosis> ;
    rdfs:range <http://UNKNOWN.org/enum_CRDCH_Diagnosis_method_of_diagnosis> ;
    skos:definition "The method used to confirm the patients malignant diagnosis" ;
    skos:editorialNote "Cardinality: 0..1" ;
    linkml:examples "Example(value='..', description=None)",
        "Example(value='Autopsy', description=None)",
        "Example(value='Biopsy', description=None)",
        "Example(value='Blood Draw', description=None)",
        "Example(value='Bone Marrow Aspirate', description=None)",
        "Example(value='Core Biopsy', description=None)" .

linkml:diagnosis__morphology a owl:ObjectProperty,
        linkml:SlotDefinition ;
    rdfs:label "diagnosis__morphology" ;
    rdfs:domain <https://example.org/crdch_model/Diagnosis> ;
    rdfs:range <http://UNKNOWN.org/enum_CRDCH_Diagnosis_morphology> ;
    skos:definition "Code that represents the histology of the disease using the third edition of the International Classification of Diseases for Oncology, published in 2000, used principally in tumor and cancer registries for coding the site (topography) and the histology (morphology) of neoplasms." ;
    skos:editorialNote "Cardinality: 0..1" ;
    linkml:examples "Example(value='8001/3', description=None)",
        "Example(value='8002/3', description=None)",
        "Example(value='8003/3', description=None)",
        "Example(value='8004/3', description=None)",
        "Example(value='8005/3', description=None)" .

linkml:diagnosis__primary_site a owl:ObjectProperty,
        linkml:SlotDefinition ;
    rdfs:label "diagnosis__primary_site" ;
    rdfs:domain <https://example.org/crdch_model/Diagnosis> ;
    rdfs:range <https://example.org/crdch_model/BodySite> ;
    skos:definition "The anatomical location of the primary condition" ;
    skos:editorialNote "Cardinality: 0..m" ;
    linkml:examples "Example(value='', description=None)" .

linkml:diagnosis__primary_tumor_dimensional_measures a owl:ObjectProperty,
        linkml:SlotDefinition ;
    rdfs:label "diagnosis__primary_tumor_dimensional_measures" ;
    rdfs:domain <https://example.org/crdch_model/Diagnosis> ;
    rdfs:range <https://example.org/crdch_model/DimensionalObservationSet> ;
    skos:definition "Observations about the current physical dimensions of the primary tumor." ;
    skos:editorialNote "Cardinality: 0..1" ;
    linkml:examples "Example(value='', description=None)" .

linkml:diagnosis__prior_diagnosis a owl:ObjectProperty,
        linkml:SlotDefinition ;
    rdfs:label "diagnosis__prior_diagnosis" ;
    rdfs:domain <https://example.org/crdch_model/Diagnosis> ;
    rdfs:range <https://example.org/crdch_model/Diagnosis> ;
    skos:definition "A reference to a prior cancer diagnosis.  In the case of relapse/recurrent disease, this attribute may be populated with a reference to the initial diagnosis." ;
    skos:editorialNote "Cardinality: 0..1" ;
    linkml:examples "Example(value='', description=None)" .

linkml:diagnosis__related_specimen a owl:ObjectProperty,
        linkml:SlotDefinition ;
    rdfs:label "diagnosis__related_specimen" ;
    rdfs:domain <https://example.org/crdch_model/Diagnosis> ;
    rdfs:range <https://example.org/crdch_model/Specimen> ;
    skos:definition "The specimen from which this diagnosis is made" ;
    skos:editorialNote "Cardinality: 0..m" ;
    linkml:examples "Example(value='', description=None)" .

linkml:diagnosis__stage a owl:ObjectProperty,
        linkml:SlotDefinition ;
    rdfs:label "diagnosis__stage" ;
    rdfs:domain <https://example.org/crdch_model/Diagnosis> ;
    rdfs:range <https://example.org/crdch_model/CancerStageObservationSet> ;
    skos:definition "The extent of a cancer in the body. Staging is usually based on the size of the tumor, whether lymph nodes contain cancer, and whether the cancer has spread from the original site to other parts of the body." ;
    skos:editorialNote "Cardinality: 0..m" ;
    linkml:examples "Example(value='', description=None)" .

linkml:diagnosis__subject a owl:ObjectProperty,
        linkml:SlotDefinition ;
    rdfs:label "diagnosis__subject" ;
    rdfs:domain <https://example.org/crdch_model/Diagnosis> ;
    rdfs:range <https://example.org/crdch_model/Subject> ;
    skos:definition "The subject of this diagnosis." ;
    skos:editorialNote "Cardinality: 0..1" ;
    linkml:examples "Example(value='', description=None)" .

linkml:diagnosis__supporting_observation a owl:ObjectProperty,
        linkml:SlotDefinition ;
    rdfs:label "diagnosis__supporting_observation" ;
    rdfs:domain <https://example.org/crdch_model/Diagnosis> ;
    rdfs:range <https://example.org/crdch_model/Observation> ;
    skos:definition "One or more observations that capture information relevant to this condition or diagnosis." ;
    skos:editorialNote "Cardinality: 0..m" ;
    linkml:examples "Example(value='', description=None)" .

linkml:diagnosis__year_at_diagnosis a owl:ObjectProperty,
        linkml:SlotDefinition ;
    rdfs:label "diagnosis__year_at_diagnosis" ;
    rdfs:domain <https://example.org/crdch_model/Diagnosis> ;
    rdfs:range <https://example.org/crdch_model/Entity> ;
    skos:definition "Numeric value to represent the year of an individual's diagnosis." ;
    skos:editorialNote "Cardinality: 0..1" ;
    linkml:examples "Example(value='', description=None)" .

linkml:dimensionalObservationSet__category a owl:ObjectProperty,
        linkml:SlotDefinition ;
    rdfs:label "dimensionalObservationSet__category" ;
    rdfs:domain <https://example.org/crdch_model/DimensionalObservationSet> ;
    rdfs:range <http://UNKNOWN.org/enum_CRDCH_DimensionalObservationSet_category> ;
    skos:definition "The general category of observation set described" ;
    skos:editorialNote "Cardinality: 0..0" ;
    skos:note "FHIR naming conventions are followed here, where 'id' is used for logical identifiers which are unique only within a given system, and 'identifier' for business identifiers, which are used to connect entities or share content across systems.  The complex 'Identifier' data type is used  to capture the identifier itself, along with metadata about its source." ;
    linkml:examples "Example(value='', description=None)" .

linkml:dimensionalObservationSet__focus a owl:ObjectProperty,
        linkml:SlotDefinition ;
    rdfs:label "dimensionalObservationSet__focus" ;
    rdfs:domain <https://example.org/crdch_model/DimensionalObservationSet> ;
    rdfs:range <https://example.org/crdch_model/Entity> ;
    skos:definition "The entity or entities directly observed/measured in generating an observation result." ;
    skos:editorialNote "Cardinality: 0..m" ;
    skos:note "The 'focus', 'subject', and 'specimen' fields are useful when data creators want an Observation object to stand on its own, so it can point back to the entities it is about.  These fields are not needed when an Observation is embedded in a Specimen or other entity, where focus, subject, and specimen can be determined from context. " ;
    linkml:examples "Example(value='', description=None)" .

linkml:dimensionalObservationSet__id a owl:ObjectProperty,
        linkml:SlotDefinition ;
    rdfs:label "dimensionalObservationSet__id" ;
    rdfs:domain <https://example.org/crdch_model/DimensionalObservationSet> ;
    rdfs:range <https://example.org/crdch_model/Entity> ;
    skos:definition "The 'logical' identifier of the entity within the system of record.  The simple value of this attribute stands for an identifier of this data object within the system, it can be used as a reference from other objects within the same system (i.e. primary and foreign keys), and it should be unique per type of object. The same data object copied to a different system will likely have a different \"id\" in the new system since \"id\" values are system specific and do not represent persistent business identifiers. Business identifiers are assigned outside the information system and are captured in the \"identifier\" field. The \"id\" field is more likely to be a serially or randomly generated value that is assigned to the data object as it is created in a system." ;
    skos:editorialNote "Cardinality: 0..0" ;
    skos:note "FHIR naming conventions are followed here, where 'id' is used for logical identifiers, and 'identifier' for business identifiers.   The identified entity may have a different 'id' in a different system, and have many external business 'identifiers' associated with it. If an \"id\" value can also be considered to be a business identifier, and should be transmissible to other systems, it should be duplicated in the \"identifier\" attribute along with the additional metadata needed to give context to the value of \"id\". An entity in this model that does not have an \"id\" field is considered to be an embeddable entity that can not stand on its own. " ;
    linkml:examples "Example(value='', description=None)" .

linkml:dimensionalObservationSet__method_type a owl:ObjectProperty,
        linkml:SlotDefinition ;
    rdfs:label "dimensionalObservationSet__method_type" ;
    rdfs:domain <https://example.org/crdch_model/DimensionalObservationSet> ;
    rdfs:range <http://UNKNOWN.org/enum_CRDCH_DimensionalObservationSet_method_type> ;
    skos:definition "A type of method used in generating each of the Observations bundled in the set." ;
    skos:editorialNote "Cardinality: 0..m" ;
    skos:note "This may be a type of observational, measurement, experimental, or computational method specifying how to generate data (e.g. 'manual counting', 'bright field microscopy'). Or a Guideline or SOP specifying how to interpret data and/or encode the result of an  Observation (e.g. a Cancer Staging system such as that defined by the AJCC, or variant interpretation guideline such as that provided by the ACMG)." ;
    linkml:examples "Example(value='', description=None)" .

linkml:dimensionalObservationSet__observations a owl:ObjectProperty,
        linkml:SlotDefinition ;
    rdfs:label "dimensionalObservationSet__observations" ;
    rdfs:domain <https://example.org/crdch_model/DimensionalObservationSet> ;
    rdfs:range <https://example.org/crdch_model/DimensionalObservation> ;
    skos:definition "A set of one or more more atomic observations that are conceptually or logically related - e.g. two components of some compound measurement (e.g. the systolic and diastolic components of a blood pressure measurement), or a panel of related measurements run and interpreted together on the same subject/specimen (e.g. a blood panel, or separate dimensional measurements of a specimen)." ;
    skos:editorialNote "Cardinality: 0..m" ;
    linkml:examples "Example(value='', description=None)" .

linkml:dimensionalObservationSet__performed_by a owl:ObjectProperty,
        linkml:SlotDefinition ;
    rdfs:label "dimensionalObservationSet__performed_by" ;
    rdfs:domain <https://example.org/crdch_model/DimensionalObservationSet> ;
    rdfs:range <https://example.org/crdch_model/Organization> ;
    skos:definition "The organization or group that performed the observation activity." ;
    skos:editorialNote "Cardinality: 0..1" ;
    linkml:examples "Example(value='', description=None)" .

linkml:dimensionalObservationSet__subject a owl:ObjectProperty,
        linkml:SlotDefinition ;
    rdfs:label "dimensionalObservationSet__subject" ;
    rdfs:domain <https://example.org/crdch_model/DimensionalObservationSet> ;
    rdfs:range <https://example.org/crdch_model/Subject> ;
    skos:definition "The patient that the observation is about (if not the direct focus).  e.g. observations are often made on specimens derived from a patient, or other entities related to a patient, that ultimately tell us something about the patient of interest." ;
    skos:editorialNote "Cardinality: 0..1" ;
    linkml:examples "Example(value='', description=None)" .

linkml:dimensionalObservation__category a owl:ObjectProperty,
        linkml:SlotDefinition ;
    rdfs:label "dimensionalObservation__category" ;
    rdfs:domain <https://example.org/crdch_model/DimensionalObservation> ;
    rdfs:range <http://UNKNOWN.org/enum_CRDCH_DimensionalObservation_category> ;
    skos:definition "The general category of observation described" ;
    skos:editorialNote "Cardinality: 0..0" ;
    skos:note "Use only if we don't define named subtypes of Observation for specific categories." ;
    linkml:examples "Example(value='', description=None)" .

linkml:dimensionalObservation__focus a owl:ObjectProperty,
        linkml:SlotDefinition ;
    rdfs:label "dimensionalObservation__focus" ;
    rdfs:domain <https://example.org/crdch_model/DimensionalObservation> ;
    rdfs:range <https://example.org/crdch_model/Entity> ;
    skos:definition "The entity or entities directly observed/measured in generating an observation result." ;
    skos:editorialNote "Cardinality: 0..m" ;
    skos:note "The 'focus', 'subject', and 'specimen' fields are useful when data creators want an Observation object to stand on its own, so it can point back to the entities it is about.  These fields are not needed when an Observation is embedded in a Specimen or other entity, where focus, subject, and specimen can be determined from context. " ;
    linkml:examples "Example(value='', description=None)" .

linkml:dimensionalObservation__id a owl:ObjectProperty,
        linkml:SlotDefinition ;
    rdfs:label "dimensionalObservation__id" ;
    rdfs:domain <https://example.org/crdch_model/DimensionalObservation> ;
    rdfs:range <https://example.org/crdch_model/Entity> ;
    skos:definition "The 'logical' identifier of the entity within the system of record.  The simple value of this attribute stands for an identifier of this data object within the system, it can be used as a reference from other objects within the same system (i.e. primary and foreign keys), and it should be unique per type of object. The same data object copied to a different system will likely have a different \"id\" in the new system since \"id\" values are system specific and do not represent persistent business identifiers. Business identifiers are assigned outside the information system and are captured in the \"identifier\" field. The \"id\" field is more likely to be a serially or randomly generated value that is assigned to the data object as it is created in a system." ;
    skos:editorialNote "Cardinality: 0..0" ;
    skos:note "FHIR naming conventions are followed here, where 'id' is used for logical identifiers, and 'identifier' for business identifiers.   The identified entity may have a different 'id' in a different system, and have many external business 'identifiers' associated with it. If an \"id\" value can also be considered to be a business identifier, and should be transmissible to other systems, it should be duplicated in the \"identifier\" attribute along with the additional metadata needed to give context to the value of \"id\". An entity in this model that does not have an \"id\" field is considered to be an embeddable entity that can not stand on its own. " ;
    linkml:examples "Example(value='', description=None)" .

linkml:dimensionalObservation__method_type a owl:ObjectProperty,
        linkml:SlotDefinition ;
    rdfs:label "dimensionalObservation__method_type" ;
    rdfs:domain <https://example.org/crdch_model/DimensionalObservation> ;
    rdfs:range <http://UNKNOWN.org/enum_CRDCH_DimensionalObservation_method_type> ;
    skos:definition "A type of method used in generating the Observation result." ;
    skos:editorialNote "Cardinality: 0..m" ;
    skos:note "This may be a type of observational, measurement, experimental, or computational method specifying how to generate data (e.g. 'manual counting', 'bright field microscopy',). Or a Guideline or SOP specifying how to interpret data and/or encode the result of an  Observation (e.g. a Cancer Staging system such as that defined by the AJCC, or variant interpretation guideline such as that provided by the ACMG)." ;
    linkml:examples "Example(value='', description=None)" .

linkml:dimensionalObservation__observation_type a owl:ObjectProperty,
        linkml:SlotDefinition ;
    rdfs:label "dimensionalObservation__observation_type" ;
    rdfs:domain <https://example.org/crdch_model/DimensionalObservation> ;
    rdfs:range <http://UNKNOWN.org/enum_CRDCH_DimensionalObservation_observation_type> ;
    skos:definition "The specific type of observation made - i.e. the feature or characteristic that was observed, measured, estimated, etc." ;
    skos:editorialNote "Cardinality: 1..1" ;
    skos:note "This field holds the 'key' in the core key-value pair comprised of the observation_type field and the relevant value(s) field." ;
    linkml:examples "Example(value='', description=None)" .

linkml:dimensionalObservation__performed_by a owl:ObjectProperty,
        linkml:SlotDefinition ;
    rdfs:label "dimensionalObservation__performed_by" ;
    rdfs:domain <https://example.org/crdch_model/DimensionalObservation> ;
    rdfs:range <https://example.org/crdch_model/Organization> ;
    skos:definition "The organization or group that performed the observation activity." ;
    skos:editorialNote "Cardinality: 0..1" ;
    linkml:examples "Example(value='', description=None)" .

linkml:dimensionalObservation__subject a owl:ObjectProperty,
        linkml:SlotDefinition ;
    rdfs:label "dimensionalObservation__subject" ;
    rdfs:domain <https://example.org/crdch_model/DimensionalObservation> ;
    rdfs:range <https://example.org/crdch_model/Subject> ;
    skos:definition "The patient that the observation is about (if not the direct focus).  e.g. observations are often made on specimens derived from a patient, or other entities related to a patient, that ultimately tell us something about the patient of interest." ;
    skos:editorialNote "Cardinality: 0..1" ;
    linkml:examples "Example(value='', description=None)" .

linkml:dimensionalObservation__valueQuantity a owl:ObjectProperty,
        linkml:SlotDefinition ;
    rdfs:label "dimensionalObservation__valueQuantity" ;
    rdfs:domain <https://example.org/crdch_model/DimensionalObservation> ;
    rdfs:range <https://example.org/crdch_model/Quantity> ;
    skos:definition "The result of the observation, encoded as a free-text Quantity." ;
    skos:editorialNote "Cardinality: 1..1" ;
    linkml:examples "Example(value='', description=None)" .

linkml:document__description a owl:ObjectProperty,
        linkml:SlotDefinition ;
    rdfs:label "document__description" ;
    rdfs:domain <https://example.org/crdch_model/Document> ;
    rdfs:range <https://example.org/crdch_model/Entity> ;
    skos:definition "A free text description or summary of the report." ;
    skos:editorialNote "Cardinality: 0..1" ;
    linkml:examples "Example(value='', description=None)" .

linkml:document__document_type a owl:ObjectProperty,
        linkml:SlotDefinition ;
    rdfs:label "document__document_type" ;
    rdfs:domain <https://example.org/crdch_model/Document> ;
    rdfs:range <http://UNKNOWN.org/enum_CRDCH_Document_document_type> ;
    skos:definition "The high-level type of the document (e.g.  'publication', 'pathology report')" ;
    skos:editorialNote "Cardinality: 0..1" ;
    linkml:examples "Example(value='', description=None)" .

linkml:document__focus a owl:ObjectProperty,
        linkml:SlotDefinition ;
    rdfs:label "document__focus" ;
    rdfs:domain <https://example.org/crdch_model/Document> ;
    rdfs:range <https://example.org/crdch_model/Entity> ;
    skos:definition "The entity that the report is primarily about" ;
    skos:editorialNote "Cardinality: 0..1" ;
    linkml:examples "Example(value='', description=None)" .

linkml:document__id a owl:ObjectProperty,
        linkml:SlotDefinition ;
    rdfs:label "document__id" ;
    rdfs:domain <https://example.org/crdch_model/Document> ;
    rdfs:range <https://example.org/crdch_model/Entity> ;
    skos:definition "The 'logical' identifier of the entity within the system of record.  The simple value of this attribute stands for an identifier of this data object within the system, it can be used as a reference from other objects within the same system (i.e. primary and foreign keys), and it should be unique per type of object. The same data object copied to a different system will likely have a different \"id\" in the new system since \"id\" values are system specific and do not represent persistent business identifiers. Business identifiers are assigned outside the information system and are captured in the \"identifier\" field. The \"id\" field is more likely to be a serially or randomly generated value that is assigned to the data object as it is created in a system." ;
    skos:editorialNote "Cardinality: 0..1" ;
    skos:note "FHIR naming conventions are followed here, where 'id' is used for logical identifiers, and 'identifier' for business identifiers.   The identified entity may have a different 'id' in a different system, and have many external business 'identifiers' associated with it. If an \"id\" value can also be considered to be a business identifier, and should be transmissible to other systems, it should be duplicated in the \"identifier\" attribute along with the additional metadata needed to give context to the value of \"id\". An entity in this model that does not have an \"id\" field is considered to be an embeddable entity that can not stand on its own. " ;
    linkml:examples "Example(value='', description=None)" .

linkml:document__identifier a owl:ObjectProperty,
        linkml:SlotDefinition ;
    rdfs:label "document__identifier" ;
    rdfs:domain <https://example.org/crdch_model/Document> ;
    rdfs:range <https://example.org/crdch_model/Identifier> ;
    skos:definition "A 'business' identifier or accession number for the entity, typically as provided by an external system or authority, that are globally unique and persist across implementing systems. Also, since these identifiers are created outside the information system through a specific business process, the Identifier type has additional attributes to capture this additional metadata so the actual identifier values are qualified by the context that created those values. This additional context allows \"identifier\" instances to be transmitted as business data across systems while still being able to trace them back to the system of origin." ;
    skos:editorialNote "Cardinality: 0..m" ;
    skos:note "FHIR naming conventions are followed here, where 'id' is used for logical identifiers which are unique only within a given system, and 'identifier' for business identifiers, which are used to connect entities or share content across systems.  The complex 'Identifier' data type is used  to capture the identifier itself, along with metadata about its source." ;
    linkml:examples "Example(value='', description=None)" .

linkml:document__url a owl:ObjectProperty,
        linkml:SlotDefinition ;
    rdfs:label "document__url" ;
    rdfs:domain <https://example.org/crdch_model/Document> ;
    rdfs:range <https://example.org/crdch_model/Entity> ;
    skos:definition "A URL/web address where the document can be accessed." ;
    skos:editorialNote "Cardinality: 0..m" ;
    linkml:examples "Example(value='', description=None)" .

linkml:environmentalExposureObservation__category a owl:ObjectProperty,
        linkml:SlotDefinition ;
    rdfs:label "environmentalExposureObservation__category" ;
    rdfs:domain <https://example.org/crdch_model/EnvironmentalExposureObservation> ;
    rdfs:range <http://UNKNOWN.org/enum_CRDCH_EnvironmentalExposureObservation_category> ;
    skos:definition "The general category of observation described" ;
    skos:editorialNote "Cardinality: 0..0" ;
    linkml:examples "Example(value='', description=None)" .

linkml:environmentalExposureObservation__focus a owl:ObjectProperty,
        linkml:SlotDefinition ;
    rdfs:label "environmentalExposureObservation__focus" ;
    rdfs:domain <https://example.org/crdch_model/EnvironmentalExposureObservation> ;
    rdfs:range <https://example.org/crdch_model/Entity> ;
    skos:definition "The entity or entities directly observed/measured in generating an observation result." ;
    skos:editorialNote "Cardinality: 0..0" ;
    skos:note "The 'focus', 'subject', and 'specimen' fields are useful when data creators want an Observation object to stand on its own, so it can point back to the entities it is about.  These fields are not needed when an Observation is embedded in a Specimen or other entity, where focus, subject, and specimen can be determined from context. " ;
    linkml:examples "Example(value='', description=None)" .

linkml:environmentalExposureObservation__id a owl:ObjectProperty,
        linkml:SlotDefinition ;
    rdfs:label "environmentalExposureObservation__id" ;
    rdfs:domain <https://example.org/crdch_model/EnvironmentalExposureObservation> ;
    rdfs:range <https://example.org/crdch_model/Entity> ;
    skos:definition "The 'logical' identifier of the entity within the system of record.  The simple value of this attribute stands for an identifier of this data object within the system, it can be used as a reference from other objects within the same system (i.e. primary and foreign keys), and it should be unique per type of object. The same data object copied to a different system will likely have a different \"id\" in the new system since \"id\" values are system specific and do not represent persistent business identifiers. Business identifiers are assigned outside the information system and are captured in the \"identifier\" field. The \"id\" field is more likely to be a serially or randomly generated value that is assigned to the data object as it is created in a system." ;
    skos:editorialNote "Cardinality: 0..0" ;
    skos:note "FHIR naming conventions are followed here, where 'id' is used for logical identifiers, and 'identifier' for business identifiers.   The identified entity may have a different 'id' in a different system, and have many external business 'identifiers' associated with it. If an \"id\" value can also be considered to be a business identifier, and should be transmissible to other systems, it should be duplicated in the \"identifier\" attribute along with the additional metadata needed to give context to the value of \"id\". An entity in this model that does not have an \"id\" field is considered to be an embeddable entity that can not stand on its own. " ;
    linkml:examples "Example(value='', description=None)" .

linkml:environmentalExposureObservation__method_type a owl:ObjectProperty,
        linkml:SlotDefinition ;
    rdfs:label "environmentalExposureObservation__method_type" ;
    rdfs:domain <https://example.org/crdch_model/EnvironmentalExposureObservation> ;
    rdfs:range <http://UNKNOWN.org/enum_CRDCH_EnvironmentalExposureObservation_method_type> ;
    skos:definition "A type of method used in generating the Observation result." ;
    skos:editorialNote "Cardinality: 0..0" ;
    skos:note "This may be a type of observational, measurement, experimental, or computational method specifying how to generate data (e.g. 'manual counting', 'bright field microscopy',). Or a Guideline or SOP specifying how to interpret data and/or encode the result of an  Observation (e.g. a Cancer Staging system such as that defined by the AJCC, or variant interpretation guideline such as that provided by the ACMG)." ;
    linkml:examples "Example(value='', description=None)" .

linkml:environmentalExposureObservation__observation_type a owl:ObjectProperty,
        linkml:SlotDefinition ;
    rdfs:label "environmentalExposureObservation__observation_type" ;
    rdfs:domain <https://example.org/crdch_model/EnvironmentalExposureObservation> ;
    rdfs:range <http://UNKNOWN.org/enum_CRDCH_EnvironmentalExposureObservation_observation_type> ;
    skos:definition "The specific type of environmental exposure observation made - i.e. the feature or characteristic that was observed, measured, estimated, etc.." ;
    skos:editorialNote "Cardinality: 1..1" ;
    skos:note "This field holds the 'key' in the core key-value pair comprised of the observation_type field and the relevant value(s) field." ;
    linkml:examples "Example(value='asbestos_exposure', description=None)",
        "Example(value='coal_dust_exposure', description=None)",
        "Example(value='radon_exposure', description=None)",
        "Example(value='respirable_crystalline_silica_exposure', description=None)",
        "Example(value='type_of_smoke_exposure', description=None)" .

linkml:environmentalExposureObservation__performed_by a owl:ObjectProperty,
        linkml:SlotDefinition ;
    rdfs:label "environmentalExposureObservation__performed_by" ;
    rdfs:domain <https://example.org/crdch_model/EnvironmentalExposureObservation> ;
    rdfs:range <https://example.org/crdch_model/Organization> ;
    skos:definition "The organization or group that performed the observation activity." ;
    skos:editorialNote "Cardinality: 0..0" ;
    linkml:examples "Example(value='', description=None)" .

linkml:environmentalExposureObservation__subject a owl:ObjectProperty,
        linkml:SlotDefinition ;
    rdfs:label "environmentalExposureObservation__subject" ;
    rdfs:domain <https://example.org/crdch_model/EnvironmentalExposureObservation> ;
    rdfs:range <https://example.org/crdch_model/Subject> ;
    skos:definition "The patient that the observation is about (if not the direct focus).  e.g. observations are often made on specimens derived from a patient, or other entities related to a patient, that ultimately tell us something about the patient of interest." ;
    skos:editorialNote "Cardinality: 0..1" ;
    linkml:examples "Example(value='', description=None)" .

linkml:environmentalExposureObservation__valueCodeableConcept a owl:ObjectProperty,
        linkml:SlotDefinition ;
    rdfs:label "environmentalExposureObservation__valueCodeableConcept" ;
    rdfs:domain <https://example.org/crdch_model/EnvironmentalExposureObservation> ;
    rdfs:range <http://UNKNOWN.org/enum_CRDCH_EnvironmentalExposureObservation_valueCodeableConcept> ;
    skos:definition "The result of the observation, encoded as a CodeableConcept." ;
    skos:editorialNote "Cardinality: 1..1" ;
    skos:note "One and only one of the value(x) fields must be populated." ;
    linkml:examples "Example(value='', description=None)" .

linkml:executionConditionObservation__category a owl:ObjectProperty,
        linkml:SlotDefinition ;
    rdfs:label "executionConditionObservation__category" ;
    rdfs:domain <https://example.org/crdch_model/ExecutionConditionObservation> ;
    rdfs:range <http://UNKNOWN.org/enum_CRDCH_ExecutionConditionObservation_category> ;
    skos:definition "The general category of observation described" ;
    skos:editorialNote "Cardinality: 0..0" ;
    linkml:examples "Example(value='', description=None)" .

linkml:executionConditionObservation__focus a owl:ObjectProperty,
        linkml:SlotDefinition ;
    rdfs:label "executionConditionObservation__focus" ;
    rdfs:domain <https://example.org/crdch_model/ExecutionConditionObservation> ;
    rdfs:range <https://example.org/crdch_model/Entity> ;
    skos:definition "The entity or entities directly observed/measured in generating an observation result." ;
    skos:editorialNote "Cardinality: 0..0" ;
    skos:note "The 'focus', 'subject', and 'specimen' fields are useful when data creators want an Observation object to stand on its own, so it can point back to the entities it is about.  These fields are not needed when an Observation is embedded in a Specimen or other entity, where focus, subject, and specimen can be determined from context. " ;
    linkml:examples "Example(value='', description=None)" .

linkml:executionConditionObservation__id a owl:ObjectProperty,
        linkml:SlotDefinition ;
    rdfs:label "executionConditionObservation__id" ;
    rdfs:domain <https://example.org/crdch_model/ExecutionConditionObservation> ;
    rdfs:range <https://example.org/crdch_model/Entity> ;
    skos:definition "The 'logical' identifier of the entity within the system of record.  The simple value of this attribute stands for an identifier of this data object within the system, it can be used as a reference from other objects within the same system (i.e. primary and foreign keys), and it should be unique per type of object. The same data object copied to a different system will likely have a different \"id\" in the new system since \"id\" values are system specific and do not represent persistent business identifiers. Business identifiers are assigned outside the information system and are captured in the \"identifier\" field. The \"id\" field is more likely to be a serially or randomly generated value that is assigned to the data object as it is created in a system." ;
    skos:editorialNote "Cardinality: 0..0" ;
    skos:note "FHIR naming conventions are followed here, where 'id' is used for logical identifiers, and 'identifier' for business identifiers.   The identified entity may have a different 'id' in a different system, and have many external business 'identifiers' associated with it. If an \"id\" value can also be considered to be a business identifier, and should be transmissible to other systems, it should be duplicated in the \"identifier\" attribute along with the additional metadata needed to give context to the value of \"id\". An entity in this model that does not have an \"id\" field is considered to be an embeddable entity that can not stand on its own. " ;
    linkml:examples "Example(value='', description=None)" .

linkml:executionConditionObservation__method_type a owl:ObjectProperty,
        linkml:SlotDefinition ;
    rdfs:label "executionConditionObservation__method_type" ;
    rdfs:domain <https://example.org/crdch_model/ExecutionConditionObservation> ;
    rdfs:range <http://UNKNOWN.org/enum_CRDCH_ExecutionConditionObservation_method_type> ;
    skos:definition "A type of method used in generating the Observation result." ;
    skos:editorialNote "Cardinality: 0..0" ;
    skos:note "This may be a type of observational, measurement, experimental, or computational method specifying how to generate data (e.g. 'manual counting', 'bright field microscopy',). Or a Guideline or SOP specifying how to interpret data and/or encode the result of an  Observation (e.g. a Cancer Staging system such as that defined by the AJCC, or variant interpretation guideline such as that provided by the ACMG)." ;
    linkml:examples "Example(value='', description=None)" .

linkml:executionConditionObservation__observation_type a owl:ObjectProperty,
        linkml:SlotDefinition ;
    rdfs:label "executionConditionObservation__observation_type" ;
    rdfs:domain <https://example.org/crdch_model/ExecutionConditionObservation> ;
    rdfs:range <http://UNKNOWN.org/enum_CRDCH_ExecutionConditionObservation_observation_type> ;
    skos:definition "The specific type of environmental exposure observation made - i.e. the feature or characteristic that was observed, measured, estimated, etc.." ;
    skos:editorialNote "Cardinality: 1..1" ;
    skos:note "This field holds the 'key' in the core key-value pair comprised of the observation_type field and the relevant value(s) field." ;
    linkml:examples "Example(value='', description=None)" .

linkml:executionConditionObservation__performed_by a owl:ObjectProperty,
        linkml:SlotDefinition ;
    rdfs:label "executionConditionObservation__performed_by" ;
    rdfs:domain <https://example.org/crdch_model/ExecutionConditionObservation> ;
    rdfs:range <https://example.org/crdch_model/Organization> ;
    skos:definition "The organization or group that performed the observation activity." ;
    skos:editorialNote "Cardinality: 0..0" ;
    linkml:examples "Example(value='', description=None)" .

linkml:executionConditionObservation__subject a owl:ObjectProperty,
        linkml:SlotDefinition ;
    rdfs:label "executionConditionObservation__subject" ;
    rdfs:domain <https://example.org/crdch_model/ExecutionConditionObservation> ;
    rdfs:range <https://example.org/crdch_model/Subject> ;
    skos:definition "The patient that the observation is about (if not the direct focus).  e.g. observations are often made on specimens derived from a patient, or other entities related to a patient, that ultimately tell us something about the patient of interest." ;
    skos:editorialNote "Cardinality: 0..1" ;
    linkml:examples "Example(value='', description=None)" .

linkml:executionConditionObservation__valueCodeableConcept a owl:ObjectProperty,
        linkml:SlotDefinition ;
    rdfs:label "executionConditionObservation__valueCodeableConcept" ;
    rdfs:domain <https://example.org/crdch_model/ExecutionConditionObservation> ;
    rdfs:range <http://UNKNOWN.org/enum_CRDCH_ExecutionConditionObservation_valueCodeableConcept> ;
    skos:definition "The result of the observation, encoded as a CodeableConcept." ;
    skos:editorialNote "Cardinality: 1..1" ;
    skos:note "One and only one of the value(x) fields must be populated." ;
    linkml:examples "Example(value='', description=None)" .

linkml:executionTimeObservation__category a owl:ObjectProperty,
        linkml:SlotDefinition ;
    rdfs:label "executionTimeObservation__category" ;
    rdfs:domain <https://example.org/crdch_model/ExecutionTimeObservation> ;
    rdfs:range <http://UNKNOWN.org/enum_CRDCH_ExecutionTimeObservation_category> ;
    skos:definition "The general category of observation described" ;
    skos:editorialNote "Cardinality: 0..0" ;
    linkml:examples "Example(value='', description=None)" .

linkml:executionTimeObservation__focus a owl:ObjectProperty,
        linkml:SlotDefinition ;
    rdfs:label "executionTimeObservation__focus" ;
    rdfs:domain <https://example.org/crdch_model/ExecutionTimeObservation> ;
    rdfs:range <https://example.org/crdch_model/Entity> ;
    skos:definition "The entity or entities directly observed/measured in generating an observation result." ;
    skos:editorialNote "Cardinality: 0..0" ;
    skos:note "The 'focus', 'subject', and 'specimen' fields are useful when data creators want an Observation object to stand on its own, so it can point back to the entities it is about.  These fields are not needed when an Observation is embedded in a Specimen or other entity, where focus, subject, and specimen can be determined from context. " ;
    linkml:examples "Example(value='', description=None)" .

linkml:executionTimeObservation__id a owl:ObjectProperty,
        linkml:SlotDefinition ;
    rdfs:label "executionTimeObservation__id" ;
    rdfs:domain <https://example.org/crdch_model/ExecutionTimeObservation> ;
    rdfs:range <https://example.org/crdch_model/Entity> ;
    skos:definition "The 'logical' identifier of the entity within the system of record.  The simple value of this attribute stands for an identifier of this data object within the system, it can be used as a reference from other objects within the same system (i.e. primary and foreign keys), and it should be unique per type of object. The same data object copied to a different system will likely have a different \"id\" in the new system since \"id\" values are system specific and do not represent persistent business identifiers. Business identifiers are assigned outside the information system and are captured in the \"identifier\" field. The \"id\" field is more likely to be a serially or randomly generated value that is assigned to the data object as it is created in a system." ;
    skos:editorialNote "Cardinality: 0..0" ;
    skos:note "FHIR naming conventions are followed here, where 'id' is used for logical identifiers, and 'identifier' for business identifiers.   The identified entity may have a different 'id' in a different system, and have many external business 'identifiers' associated with it. If an \"id\" value can also be considered to be a business identifier, and should be transmissible to other systems, it should be duplicated in the \"identifier\" attribute along with the additional metadata needed to give context to the value of \"id\". An entity in this model that does not have an \"id\" field is considered to be an embeddable entity that can not stand on its own. " ;
    linkml:examples "Example(value='', description=None)" .

linkml:executionTimeObservation__method_type a owl:ObjectProperty,
        linkml:SlotDefinition ;
    rdfs:label "executionTimeObservation__method_type" ;
    rdfs:domain <https://example.org/crdch_model/ExecutionTimeObservation> ;
    rdfs:range <http://UNKNOWN.org/enum_CRDCH_ExecutionTimeObservation_method_type> ;
    skos:definition "A type of method used in generating the Observation result." ;
    skos:editorialNote "Cardinality: 0..0" ;
    skos:note "This may be a type of observational, measurement, experimental, or computational method specifying how to generate data (e.g. 'manual counting', 'bright field microscopy',). Or a Guideline or SOP specifying how to interpret data and/or encode the result of an  Observation (e.g. a Cancer Staging system such as that defined by the AJCC, or variant interpretation guideline such as that provided by the ACMG)." ;
    linkml:examples "Example(value='', description=None)" .

linkml:executionTimeObservation__observation_type a owl:ObjectProperty,
        linkml:SlotDefinition ;
    rdfs:label "executionTimeObservation__observation_type" ;
    rdfs:domain <https://example.org/crdch_model/ExecutionTimeObservation> ;
    rdfs:range <http://UNKNOWN.org/enum_CRDCH_ExecutionTimeObservation_observation_type> ;
    skos:definition "The specific type of environmental exposure observation made - i.e. the feature or characteristic that was observed, measured, estimated, etc.." ;
    skos:editorialNote "Cardinality: 1..1" ;
    skos:note "This field holds the 'key' in the core key-value pair comprised of the observation_type field and the relevant value(s) field." ;
    linkml:examples "Example(value='', description=None)" .

linkml:executionTimeObservation__performed_by a owl:ObjectProperty,
        linkml:SlotDefinition ;
    rdfs:label "executionTimeObservation__performed_by" ;
    rdfs:domain <https://example.org/crdch_model/ExecutionTimeObservation> ;
    rdfs:range <https://example.org/crdch_model/Organization> ;
    skos:definition "The organization or group that performed the observation activity." ;
    skos:editorialNote "Cardinality: 0..0" ;
    linkml:examples "Example(value='', description=None)" .

linkml:executionTimeObservation__subject a owl:ObjectProperty,
        linkml:SlotDefinition ;
    rdfs:label "executionTimeObservation__subject" ;
    rdfs:domain <https://example.org/crdch_model/ExecutionTimeObservation> ;
    rdfs:range <https://example.org/crdch_model/Subject> ;
    skos:definition "The patient that the observation is about (if not the direct focus).  e.g. observations are often made on specimens derived from a patient, or other entities related to a patient, that ultimately tell us something about the patient of interest." ;
    skos:editorialNote "Cardinality: 0..1" ;
    linkml:examples "Example(value='', description=None)" .

linkml:executionTimeObservation__valueQuantity a owl:ObjectProperty,
        linkml:SlotDefinition ;
    rdfs:label "executionTimeObservation__valueQuantity" ;
    rdfs:domain <https://example.org/crdch_model/ExecutionTimeObservation> ;
    rdfs:range <https://example.org/crdch_model/Quantity> ;
    skos:definition "The result of the observation, encoded as a free-text Quantity." ;
    skos:editorialNote "Cardinality: 1..1" ;
    skos:note "One and only one of the value(x) fields must be populated." ;
    linkml:examples "Example(value='', description=None)" .

linkml:exposure__alcohol_exposure a owl:ObjectProperty,
        linkml:SlotDefinition ;
    rdfs:label "exposure__alcohol_exposure" ;
    rdfs:domain <https://example.org/crdch_model/Exposure> ;
    rdfs:range <https://example.org/crdch_model/AlcoholExposureObservation> ;
    skos:definition "Observations about an individual's exposure to alcohol." ;
    skos:editorialNote "Cardinality: 0..m" ;
    linkml:examples "Example(value='', description=None)" .

linkml:exposure__environmental_exposure a owl:ObjectProperty,
        linkml:SlotDefinition ;
    rdfs:label "exposure__environmental_exposure" ;
    rdfs:domain <https://example.org/crdch_model/Exposure> ;
    rdfs:range <https://example.org/crdch_model/EnvironmentalExposureObservation> ;
    skos:definition "Observations about an individual's exposure to environmental substances that may impact clinical outcomes." ;
    skos:editorialNote "Cardinality: 0..m" ;
    linkml:examples "Example(value='', description=None)" .

linkml:exposure__id a owl:ObjectProperty,
        linkml:SlotDefinition ;
    rdfs:label "exposure__id" ;
    rdfs:domain <https://example.org/crdch_model/Exposure> ;
    rdfs:range <https://example.org/crdch_model/Entity> ;
    skos:definition "The 'logical' identifier of the entity within the system of record.  The simple value of this attribute stands for an identifier of this data object within the system, it can be used as a reference from other objects within the same system (i.e. primary and foreign keys), and it should be unique per type of object. The same data object copied to a different system will likely have a different \"id\" in the new system since \"id\" values are system specific and do not represent persistent business identifiers. Business identifiers are assigned outside the information system and are captured in the \"identifier\" field. The \"id\" field is more likely to be a serially or randomly generated value that is assigned to the data object as it is created in a system." ;
    skos:editorialNote "Cardinality: 1..1" ;
    skos:note "FHIR naming conventions are followed here, where 'id' is used for logical identifiers, and 'identifier' for business identifiers.   The identified entity may have a different 'id' in a different system, and have many external business 'identifiers' associated with it. If an \"id\" value can also be considered to be a business identifier, and should be transmissible to other systems, it should be duplicated in the \"identifier\" attribute along with the additional metadata needed to give context to the value of \"id\". An entity in this model that does not have an \"id\" field is considered to be an embeddable entity that can not stand on its own. " ;
    linkml:examples "Example(value='', description=None)" .

linkml:exposure__identifier a owl:ObjectProperty,
        linkml:SlotDefinition ;
    rdfs:label "exposure__identifier" ;
    rdfs:domain <https://example.org/crdch_model/Exposure> ;
    rdfs:range <https://example.org/crdch_model/Identifier> ;
    skos:definition "A 'business' identifier or accession number for the entity, typically as provided by an external system or authority, that are globally unique and persist across implementing systems. Also, since these identifiers are created outside the information system through a specific business process, the Identifier type has additional attributes to capture this additional metadata so the actual identifier values are qualified by the context that created those values. This additional context allows \"identifier\" instances to be transmitted as business data across systems while still being able to trace them back to the system of origin." ;
    skos:editorialNote "Cardinality: 0..m" ;
    skos:note "FHIR naming conventions are followed here, where 'id' is used for logical identifiers which are unique only within a given system, and 'identifier' for business identifiers, which are used to connect entities or share content across systems.  The complex 'Identifier' data type is used  to capture the identifier itself, along with metadata about its source." ;
    linkml:examples "Example(value='', description=None)" .

linkml:exposure__subject a owl:ObjectProperty,
        linkml:SlotDefinition ;
    rdfs:label "exposure__subject" ;
    rdfs:domain <https://example.org/crdch_model/Exposure> ;
    rdfs:range <https://example.org/crdch_model/Subject> ;
    skos:definition "A reference to the Subject that is the subject of this Exposure" ;
    skos:editorialNote "Cardinality: 0..1" ;
    linkml:examples "Example(value='', description=None)" .

linkml:exposure__tobacco_exposure a owl:ObjectProperty,
        linkml:SlotDefinition ;
    rdfs:label "exposure__tobacco_exposure" ;
    rdfs:domain <https://example.org/crdch_model/Exposure> ;
    rdfs:range <https://example.org/crdch_model/TobaccoExposureObservation> ;
    skos:definition "Observations about an individual's exposure to tobacco." ;
    skos:editorialNote "Cardinality: 0..m" ;
    linkml:examples "Example(value='', description=None)" .

linkml:histologicalCompositionObservationSet__category a owl:ObjectProperty,
        linkml:SlotDefinition ;
    rdfs:label "histologicalCompositionObservationSet__category" ;
    rdfs:domain <https://example.org/crdch_model/HistologicalCompositionObservationSet> ;
    rdfs:range <http://UNKNOWN.org/enum_CRDCH_HistologicalCompositionObservationSet_category> ;
    skos:definition "The general category of observation set described" ;
    skos:editorialNote "Cardinality: 1..1" ;
    linkml:examples "Example(value='', description=None)" .

linkml:histologicalCompositionObservationSet__focus a owl:ObjectProperty,
        linkml:SlotDefinition ;
    rdfs:label "histologicalCompositionObservationSet__focus" ;
    rdfs:domain <https://example.org/crdch_model/HistologicalCompositionObservationSet> ;
    rdfs:range <https://example.org/crdch_model/Entity> ;
    skos:definition "The entity or entities directly observed/measured in generating an observation result." ;
    skos:editorialNote "Cardinality: 0..m" ;
    skos:note "The 'focus', 'subject', and 'specimen' fields are useful when data creators want an Observation object to stand on its own, so it can point back to the entities it is about.  These fields are not needed when an Observation is embedded in a Specimen or other entity, where focus, subject, and specimen can be determined from context. " ;
    linkml:examples "Example(value='', description=None)" .

linkml:histologicalCompositionObservationSet__id a owl:ObjectProperty,
        linkml:SlotDefinition ;
    rdfs:label "histologicalCompositionObservationSet__id" ;
    rdfs:domain <https://example.org/crdch_model/HistologicalCompositionObservationSet> ;
    rdfs:range <https://example.org/crdch_model/Entity> ;
    skos:definition "The 'logical' identifier of the entity within the system of record.  The simple value of this attribute stands for an identifier of this data object within the system, it can be used as a reference from other objects within the same system (i.e. primary and foreign keys), and it should be unique per type of object. The same data object copied to a different system will likely have a different \"id\" in the new system since \"id\" values are system specific and do not represent persistent business identifiers. Business identifiers are assigned outside the information system and are captured in the \"identifier\" field. The \"id\" field is more likely to be a serially or randomly generated value that is assigned to the data object as it is created in a system." ;
    skos:editorialNote "Cardinality: 1..1" ;
    skos:note "FHIR naming conventions are followed here, where 'id' is used for logical identifiers, and 'identifier' for business identifiers.   The identified entity may have a different 'id' in a different system, and have many external business 'identifiers' associated with it. If an \"id\" value can also be considered to be a business identifier, and should be transmissible to other systems, it should be duplicated in the \"identifier\" attribute along with the additional metadata needed to give context to the value of \"id\". An entity in this model that does not have an \"id\" field is considered to be an embeddable entity that can not stand on its own. " ;
    linkml:examples "Example(value='', description=None)" .

linkml:histologicalCompositionObservationSet__method_type a owl:ObjectProperty,
        linkml:SlotDefinition ;
    rdfs:label "histologicalCompositionObservationSet__method_type" ;
    rdfs:domain <https://example.org/crdch_model/HistologicalCompositionObservationSet> ;
    rdfs:range <http://UNKNOWN.org/enum_CRDCH_HistologicalCompositionObservationSet_method_type> ;
    skos:definition "A type of method used in generating each of the Observations bundled in the set." ;
    skos:editorialNote "Cardinality: 0..m" ;
    skos:note "This may be a type of observational, measurement, experimental, or computational method specifying how to generate data (e.g. 'manual counting', 'bright field microscopy'). Or a Guideline or SOP specifying how to interpret data and/or encode the result of an  Observation (e.g. a Cancer Staging system such as that defined by the AJCC, or variant interpretation guideline such as that provided by the ACMG)." ;
    linkml:examples "Example(value='', description=None)" .

linkml:histologicalCompositionObservationSet__observations a owl:ObjectProperty,
        linkml:SlotDefinition ;
    rdfs:label "histologicalCompositionObservationSet__observations" ;
    rdfs:domain <https://example.org/crdch_model/HistologicalCompositionObservationSet> ;
    rdfs:range <https://example.org/crdch_model/HistologicalCompositionObservation> ;
    skos:definition "A set of one or more more atomic observations that are conceptually or logically related - e.g. two components of some compound measurement (e.g. the systolic and diastolic components of a blood pressure measurement), or a panel of related measurements run and interpreted together on the same subject/specimen (e.g. a blood panel, or separate dimensional measurements of a specimen)." ;
    skos:editorialNote "Cardinality: 0..m" ;
    linkml:examples "Example(value='', description=None)" .

linkml:histologicalCompositionObservationSet__performed_by a owl:ObjectProperty,
        linkml:SlotDefinition ;
    rdfs:label "histologicalCompositionObservationSet__performed_by" ;
    rdfs:domain <https://example.org/crdch_model/HistologicalCompositionObservationSet> ;
    rdfs:range <https://example.org/crdch_model/Organization> ;
    skos:definition "The organization or group that performed the observation activity." ;
    skos:editorialNote "Cardinality: 0..1" ;
    linkml:examples "Example(value='', description=None)" .

linkml:histologicalCompositionObservationSet__subject a owl:ObjectProperty,
        linkml:SlotDefinition ;
    rdfs:label "histologicalCompositionObservationSet__subject" ;
    rdfs:domain <https://example.org/crdch_model/HistologicalCompositionObservationSet> ;
    rdfs:range <https://example.org/crdch_model/Subject> ;
    skos:definition "The patient that the observation is about (if not the direct focus).  e.g. observations are often made on specimens derived from a patient, or other entities related to a patient, that ultimately tell us something about the patient of interest." ;
    skos:editorialNote "Cardinality: 0..1" ;
    linkml:examples "Example(value='', description=None)" .

linkml:histologicalCompositionObservation__category a owl:ObjectProperty,
        linkml:SlotDefinition ;
    rdfs:label "histologicalCompositionObservation__category" ;
    rdfs:domain <https://example.org/crdch_model/HistologicalCompositionObservation> ;
    rdfs:range <http://UNKNOWN.org/enum_CRDCH_HistologicalCompositionObservation_category> ;
    skos:definition "The general category of observation described" ;
    skos:editorialNote "Cardinality: 0..0" ;
    skos:note "Use only if we don't define named subtypes of Observation for specific categories." ;
    linkml:examples "Example(value='', description=None)" .

linkml:histologicalCompositionObservation__focus a owl:ObjectProperty,
        linkml:SlotDefinition ;
    rdfs:label "histologicalCompositionObservation__focus" ;
    rdfs:domain <https://example.org/crdch_model/HistologicalCompositionObservation> ;
    rdfs:range <https://example.org/crdch_model/Entity> ;
    skos:definition "The entity or entities directly observed/measured in generating an observation result." ;
    skos:editorialNote "Cardinality: 0..m" ;
    skos:note "The 'focus', 'subject', and 'specimen' fields are useful when data creators want an Observation object to stand on its own, so it can point back to the entities it is about.  These fields are not needed when an Observation is embedded in a Specimen or other entity, where focus, subject, and specimen can be determined from context. " ;
    linkml:examples "Example(value='', description=None)" .

linkml:histologicalCompositionObservation__id a owl:ObjectProperty,
        linkml:SlotDefinition ;
    rdfs:label "histologicalCompositionObservation__id" ;
    rdfs:domain <https://example.org/crdch_model/HistologicalCompositionObservation> ;
    rdfs:range <https://example.org/crdch_model/Entity> ;
    skos:definition "The 'logical' identifier of the entity within the system of record.  The simple value of this attribute stands for an identifier of this data object within the system, it can be used as a reference from other objects within the same system (i.e. primary and foreign keys), and it should be unique per type of object. The same data object copied to a different system will likely have a different \"id\" in the new system since \"id\" values are system specific and do not represent persistent business identifiers. Business identifiers are assigned outside the information system and are captured in the \"identifier\" field. The \"id\" field is more likely to be a serially or randomly generated value that is assigned to the data object as it is created in a system." ;
    skos:editorialNote "Cardinality: 0..0" ;
    skos:note "FHIR naming conventions are followed here, where 'id' is used for logical identifiers, and 'identifier' for business identifiers.   The identified entity may have a different 'id' in a different system, and have many external business 'identifiers' associated with it. If an \"id\" value can also be considered to be a business identifier, and should be transmissible to other systems, it should be duplicated in the \"identifier\" attribute along with the additional metadata needed to give context to the value of \"id\". An entity in this model that does not have an \"id\" field is considered to be an embeddable entity that can not stand on its own. " ;
    linkml:examples "Example(value='', description=None)" .

linkml:histologicalCompositionObservation__method_type a owl:ObjectProperty,
        linkml:SlotDefinition ;
    rdfs:label "histologicalCompositionObservation__method_type" ;
    rdfs:domain <https://example.org/crdch_model/HistologicalCompositionObservation> ;
    rdfs:range <http://UNKNOWN.org/enum_CRDCH_HistologicalCompositionObservation_method_type> ;
    skos:definition "A type of method used in generating the Observation result." ;
    skos:editorialNote "Cardinality: 0..m" ;
    skos:note "This may be a type of observational, measurement, experimental, or computational method specifying how to generate data (e.g. 'manual counting', 'bright field microscopy,). Or a Guideline or SOP specifying how to interpret data and/or encode the result of an  Observation (e.g. a Cancer Staging system such as that defined by the AJCC, or variant interpretation guideline such as that provided by the ACMG)." ;
    linkml:examples "Example(value='', description=None)" .

linkml:histologicalCompositionObservation__observation_type a owl:ObjectProperty,
        linkml:SlotDefinition ;
    rdfs:label "histologicalCompositionObservation__observation_type" ;
    rdfs:domain <https://example.org/crdch_model/HistologicalCompositionObservation> ;
    rdfs:range <http://UNKNOWN.org/enum_CRDCH_HistologicalCompositionObservation_observation_type> ;
    skos:definition "The specific type of observation made - i.e. the feature or characteristic that was observed, measured, estimated, etc.." ;
    skos:editorialNote "Cardinality: 1..1" ;
    skos:note "This field holds the 'key' in the core key-value pair comprised of the observation_type field and the relevant value(s) field." ;
    linkml:examples "Example(value='', description=None)" .

linkml:histologicalCompositionObservation__performed_by a owl:ObjectProperty,
        linkml:SlotDefinition ;
    rdfs:label "histologicalCompositionObservation__performed_by" ;
    rdfs:domain <https://example.org/crdch_model/HistologicalCompositionObservation> ;
    rdfs:range <https://example.org/crdch_model/Organization> ;
    skos:definition "The organization or group that performed the observation activity." ;
    skos:editorialNote "Cardinality: 0..1" ;
    linkml:examples "Example(value='', description=None)" .

linkml:histologicalCompositionObservation__subject a owl:ObjectProperty,
        linkml:SlotDefinition ;
    rdfs:label "histologicalCompositionObservation__subject" ;
    rdfs:domain <https://example.org/crdch_model/HistologicalCompositionObservation> ;
    rdfs:range <https://example.org/crdch_model/Subject> ;
    skos:definition "The patient that the observation is about (if not the direct focus).  e.g. observations are often made on specimens derived from a patient, or other entities related to a patient, that ultimately tell us something about the patient of interest." ;
    skos:editorialNote "Cardinality: 0..1" ;
    linkml:examples "Example(value='', description=None)" .

linkml:histologicalCompositionObservation__valueQuantity a owl:ObjectProperty,
        linkml:SlotDefinition ;
    rdfs:label "histologicalCompositionObservation__valueQuantity" ;
    rdfs:domain <https://example.org/crdch_model/HistologicalCompositionObservation> ;
    rdfs:range <https://example.org/crdch_model/Quantity> ;
    skos:definition "The result of the observation, encoded as a free-text Quantity." ;
    skos:editorialNote "Cardinality: 1..1" ;
    skos:note "One and only one of the value(x) fields must be populated." ;
    linkml:examples "Example(value='', description=None)" .

linkml:identifier__system a owl:ObjectProperty,
        linkml:SlotDefinition ;
    rdfs:label "identifier__system" ;
    rdfs:domain <https://example.org/crdch_model/Identifier> ;
    rdfs:range <https://example.org/crdch_model/Entity> ;
    skos:definition "The system or namespace that defines the identifier." ;
    skos:editorialNote "Cardinality: 0..1" ;
    linkml:examples "Example(value='', description=None)" .

linkml:identifier__type a owl:ObjectProperty,
        linkml:SlotDefinition ;
    rdfs:label "identifier__type" ;
    rdfs:domain <https://example.org/crdch_model/Identifier> ;
    rdfs:range <http://UNKNOWN.org/enum_CRDCH_Identifier_type> ;
    skos:definition "A code that defines the type of the identifier." ;
    skos:editorialNote "Cardinality: 0..1" ;
    linkml:examples "Example(value='', description=None)" .

linkml:identifier__value a owl:ObjectProperty,
        linkml:SlotDefinition ;
    rdfs:label "identifier__value" ;
    rdfs:domain <https://example.org/crdch_model/Identifier> ;
    rdfs:range <https://example.org/crdch_model/Entity> ;
    skos:definition "The value of the identifier, as defined by the system." ;
    skos:editorialNote "Cardinality: 1..1" ;
    linkml:examples "Example(value='', description=None)" .

linkml:observationSet__category a owl:ObjectProperty,
        linkml:SlotDefinition ;
    rdfs:label "observationSet__category" ;
    rdfs:domain <https://example.org/crdch_model/ObservationSet> ;
    rdfs:range <http://UNKNOWN.org/enum_CRDCH_ObservationSet_category> ;
    skos:definition "The general category of observation set described" ;
    skos:editorialNote "Cardinality: 1..1" ;
    linkml:examples "Example(value='CellularCompositionMeasureSet', description=None)",
        "Example(value='DimensionalMeasureSet', description=None)",
        "Example(value='TissueCompositionMeasureSet', description=None)" .

linkml:observationSet__focus a owl:ObjectProperty,
        linkml:SlotDefinition ;
    rdfs:label "observationSet__focus" ;
    rdfs:domain <https://example.org/crdch_model/ObservationSet> ;
    rdfs:range <https://example.org/crdch_model/Entity> ;
    skos:definition "The entity or entities directly observed/measured in generating an observation result." ;
    skos:editorialNote "Cardinality: 0..m" ;
    skos:note "The 'focus', 'subject', and 'specimen' fields are useful when data creators want an Observation object to stand on its own, so it can point back to the entities it is about.  These fields are not needed when an Observation is embedded in a Specimen or other entity, where focus, subject, and specimen can be determined from context. " ;
    linkml:examples "Example(value='', description=None)" .

linkml:observationSet__id a owl:ObjectProperty,
        linkml:SlotDefinition ;
    rdfs:label "observationSet__id" ;
    rdfs:domain <https://example.org/crdch_model/ObservationSet> ;
    rdfs:range <https://example.org/crdch_model/Entity> ;
    skos:definition "The 'logical' identifier of the entity within the system of record.  The simple value of this attribute stands for an identifier of this data object within the system, it can be used as a reference from other objects within the same system (i.e. primary and foreign keys), and it should be unique per type of object. The same data object copied to a different system will likely have a different \"id\" in the new system since \"id\" values are system specific and do not represent persistent business identifiers. Business identifiers are assigned outside the information system and are captured in the \"identifier\" field. The \"id\" field is more likely to be a serially or randomly generated value that is assigned to the data object as it is created in a system." ;
    skos:editorialNote "Cardinality: 1..1" ;
    skos:note "FHIR naming conventions are followed here, where 'id' is used for logical identifiers, and 'identifier' for business identifiers.   The identified entity may have a different 'id' in a different system, and have many external business 'identifiers' associated with it. If an \"id\" value can also be considered to be a business identifier, and should be transmissible to other systems, it should be duplicated in the \"identifier\" attribute along with the additional metadata needed to give context to the value of \"id\". An entity in this model that does not have an \"id\" field is considered to be an embeddable entity that can not stand on its own. " ;
    linkml:examples "Example(value='', description=None)" .

linkml:observationSet__method_type a owl:ObjectProperty,
        linkml:SlotDefinition ;
    rdfs:label "observationSet__method_type" ;
    rdfs:domain <https://example.org/crdch_model/ObservationSet> ;
    rdfs:range <http://UNKNOWN.org/enum_CRDCH_ObservationSet_method_type> ;
    skos:definition "A type of method used in generating each of the Observations bundled in the set." ;
    skos:editorialNote "Cardinality: 0..m" ;
    skos:note "This may be a type of observational, measurement, experimental, or computational method specifying how to generate data (e.g. 'manual counting', 'bright field microscopy'). Or a Guideline or SOP specifying how to interpret data and/or encode the result of an  Observation (e.g. a Cancer Staging system such as that defined by the AJCC, or variant interpretation guideline such as that provided by the ACMG)." ;
    linkml:examples "Example(value='', description=None)" .

linkml:observationSet__observations a owl:ObjectProperty,
        linkml:SlotDefinition ;
    rdfs:label "observationSet__observations" ;
    rdfs:domain <https://example.org/crdch_model/ObservationSet> ;
    rdfs:range <https://example.org/crdch_model/Observation> ;
    skos:definition "A set of one or more more atomic observations that are conceptually or logically related - e.g. two components of some compound measurement (e.g. the systolic and diastolic components of a blood pressure measurement), or a panel of related measurements run and interpreted together on the same subject/specimen (e.g. a blood panel, or separate dimensional measurements of a specimen)." ;
    skos:editorialNote "Cardinality: 0..m" ;
    linkml:examples "Example(value='', description=None)" .

linkml:observationSet__performed_by a owl:ObjectProperty,
        linkml:SlotDefinition ;
    rdfs:label "observationSet__performed_by" ;
    rdfs:domain <https://example.org/crdch_model/ObservationSet> ;
    rdfs:range <https://example.org/crdch_model/Organization> ;
    skos:definition "The organization or group that performed the observation activity." ;
    skos:editorialNote "Cardinality: 0..1" ;
    linkml:examples "Example(value='', description=None)" .

linkml:observationSet__subject a owl:ObjectProperty,
        linkml:SlotDefinition ;
    rdfs:label "observationSet__subject" ;
    rdfs:domain <https://example.org/crdch_model/ObservationSet> ;
    rdfs:range <https://example.org/crdch_model/Subject> ;
    skos:definition "The patient that the observation is about (if not the direct focus).  e.g. observations are often made on specimens derived from a patient, or other entities related to a patient, that ultimately tell us something about the patient of interest." ;
    skos:editorialNote "Cardinality: 0..1" ;
    linkml:examples "Example(value='', description=None)" .

linkml:observation__category a owl:ObjectProperty,
        linkml:SlotDefinition ;
    rdfs:label "observation__category" ;
    rdfs:domain <https://example.org/crdch_model/Observation> ;
    rdfs:range <http://UNKNOWN.org/enum_CRDCH_Observation_category> ;
    skos:definition "The general category of observation described" ;
    skos:editorialNote "Cardinality: 0..1" ;
    skos:note "Use only if we don't define named subtypes of Observation for specific categories." ;
    linkml:examples "Example(value='CellularCompositionMeasure', description=None)",
        "Example(value='DimensionalMeasure', description=None)",
        "Example(value='SpecimenQualityMeasure', description=None)",
        "Example(value='TissueCompositionMeasure', description=None)",
        "Example(value='TobbaccoExposureMeasure', description=None)" .

linkml:observation__focus a owl:ObjectProperty,
        linkml:SlotDefinition ;
    rdfs:label "observation__focus" ;
    rdfs:domain <https://example.org/crdch_model/Observation> ;
    rdfs:range <https://example.org/crdch_model/Entity> ;
    skos:definition "The entity or entities directly observed/measured in generating an observation result." ;
    skos:editorialNote "Cardinality: 0..m" ;
    skos:note "The 'focus', 'subject', and 'specimen' fields are useful when data creators want an Observation object to stand on its own, so it can point back to the entities it is about.  These fields are not needed when an Observation is embedded in a Specimen or other entity, where focus, subject, and specimen can be determined from context. " ;
    linkml:examples "Example(value='', description=None)" .

linkml:observation__id a owl:ObjectProperty,
        linkml:SlotDefinition ;
    rdfs:label "observation__id" ;
    rdfs:domain <https://example.org/crdch_model/Observation> ;
    rdfs:range <https://example.org/crdch_model/Entity> ;
    skos:definition "The 'logical' identifier of the entity within the system of record.  The simple value of this attribute stands for an identifier of this data object within the system, it can be used as a reference from other objects within the same system (i.e. primary and foreign keys), and it should be unique per type of object. The same data object copied to a different system will likely have a different \"id\" in the new system since \"id\" values are system specific and do not represent persistent business identifiers. Business identifiers are assigned outside the information system and are captured in the \"identifier\" field. The \"id\" field is more likely to be a serially or randomly generated value that is assigned to the data object as it is created in a system." ;
    skos:editorialNote "Cardinality: 0..1" ;
    skos:note "FHIR naming conventions are followed here, where 'id' is used for logical identifiers, and 'identifier' for business identifiers.   The identified entity may have a different 'id' in a different system, and have many external business 'identifiers' associated with it. If an \"id\" value can also be considered to be a business identifier, and should be transmissible to other systems, it should be duplicated in the \"identifier\" attribute along with the additional metadata needed to give context to the value of \"id\". An entity in this model that does not have an \"id\" field is considered to be an embeddable entity that can not stand on its own. " ;
    linkml:examples "Example(value='', description=None)" .

linkml:observation__method_type a owl:ObjectProperty,
        linkml:SlotDefinition ;
    rdfs:label "observation__method_type" ;
    rdfs:domain <https://example.org/crdch_model/Observation> ;
    rdfs:range <http://UNKNOWN.org/enum_CRDCH_Observation_method_type> ;
    skos:definition "A type of method used in generating the Observation result." ;
    skos:editorialNote "Cardinality: 0..m" ;
    skos:note "This may be a type of observational, measurement, experimental, or computational method specifying how to generate data (e.g. 'manual counting', 'bright field microscopy'). Or a Guideline or SOP specifying how to interpret data and/or encode the result of an  Observation (e.g. a Cancer Staging system such as that defined by the AJCC, or variant interpretation guideline such as that provided by the ACMG)." ;
    linkml:examples "Example(value='', description=None)" .

linkml:observation__observation_type a owl:ObjectProperty,
        linkml:SlotDefinition ;
    rdfs:label "observation__observation_type" ;
    rdfs:domain <https://example.org/crdch_model/Observation> ;
    rdfs:range <http://UNKNOWN.org/enum_CRDCH_Observation_observation_type> ;
    skos:definition "The specific type of observation made - i.e. the feature or characteristic that was observed, measured, estimated, etc.." ;
    skos:editorialNote "Cardinality: 1..1" ;
    skos:note "This field holds the 'key' in the core key-value pair comprised of the observation_type field and the relevant value(s) field." ;
    linkml:examples "Example(value='a260_a280_ratio', description=None)",
        "Example(value='percentage_stroma', description=None)",
        "Example(value='time_between_excision_and_freezing', description=None)",
        "Example(value='tumor_tissue_area', description=None)",
        "Example(value='width_of_tumor', description=None)" .

linkml:observation__performed_by a owl:ObjectProperty,
        linkml:SlotDefinition ;
    rdfs:label "observation__performed_by" ;
    rdfs:domain <https://example.org/crdch_model/Observation> ;
    rdfs:range <https://example.org/crdch_model/Organization> ;
    skos:definition "The organization or group that performed the observation activity." ;
    skos:editorialNote "Cardinality: 0..1" ;
    linkml:examples "Example(value='', description=None)" .

linkml:observation__subject a owl:ObjectProperty,
        linkml:SlotDefinition ;
    rdfs:label "observation__subject" ;
    rdfs:domain <https://example.org/crdch_model/Observation> ;
    rdfs:range <https://example.org/crdch_model/Subject> ;
    skos:definition "The patient that the observation is about (if not the direct focus).  e.g. observations are often made on specimens derived from a patient, or other entities related to a patient, that ultimately tell us something about the patient of interest." ;
    skos:editorialNote "Cardinality: 0..1" ;
    linkml:examples "Example(value='', description=None)" .

linkml:observation__valueBoolean a owl:ObjectProperty,
        linkml:SlotDefinition ;
    rdfs:label "observation__valueBoolean" ;
    rdfs:domain <https://example.org/crdch_model/Observation> ;
    rdfs:range <https://example.org/crdch_model/Entity> ;
    skos:definition "The result of the observation, encoded as a boolean." ;
    skos:editorialNote "Cardinality: 0..1" ;
    skos:note "One and only one of the value(x) fields must be populated." ;
    linkml:examples "Example(value='', description=None)" .

linkml:observation__valueCodeableConcept a owl:ObjectProperty,
        linkml:SlotDefinition ;
    rdfs:label "observation__valueCodeableConcept" ;
    rdfs:domain <https://example.org/crdch_model/Observation> ;
    rdfs:range <http://UNKNOWN.org/enum_CRDCH_Observation_valueCodeableConcept> ;
    skos:definition "The result of the observation, encoded as a CodeableConcept." ;
    skos:editorialNote "Cardinality: 0..1" ;
    skos:note "One and only one of the value(x) fields must be populated." ;
    linkml:examples "Example(value='', description=None)" .

linkml:observation__valueDateTime a owl:ObjectProperty,
        linkml:SlotDefinition ;
    rdfs:label "observation__valueDateTime" ;
    rdfs:domain <https://example.org/crdch_model/Observation> ;
    rdfs:range <https://example.org/crdch_model/Entity> ;
    skos:definition "The result of the observation, encoded as a dateTime." ;
    skos:editorialNote "Cardinality: 0..1" ;
    skos:note "One and only one of the value(x) fields must be populated." ;
    linkml:examples "Example(value='', description=None)" .

linkml:observation__valueDecimal a owl:ObjectProperty,
        linkml:SlotDefinition ;
    rdfs:label "observation__valueDecimal" ;
    rdfs:domain <https://example.org/crdch_model/Observation> ;
    rdfs:range <https://example.org/crdch_model/Entity> ;
    skos:definition "The result of the observation, encoded as a decimal." ;
    skos:editorialNote "Cardinality: 0..1" ;
    skos:note "One and only one of the value(x) fields must be populated." ;
    linkml:examples "Example(value='', description=None)" .

linkml:observation__valueEntity a owl:ObjectProperty,
        linkml:SlotDefinition ;
    rdfs:label "observation__valueEntity" ;
    rdfs:domain <https://example.org/crdch_model/Observation> ;
    rdfs:range <https://example.org/crdch_model/Entity> ;
    skos:definition "The value of an observation" ;
    skos:editorialNote "Cardinality: 0..1" ;
    linkml:examples "Example(value='', description=None)" .

linkml:observation__valueInteger a owl:ObjectProperty,
        linkml:SlotDefinition ;
    rdfs:label "observation__valueInteger" ;
    rdfs:domain <https://example.org/crdch_model/Observation> ;
    rdfs:range <https://example.org/crdch_model/Entity> ;
    skos:definition "The result of the observation, encoded as a decimal." ;
    skos:editorialNote "Cardinality: 0..1" ;
    skos:note "One and only one of the value(x) fields must be populated." ;
    linkml:examples "Example(value='', description=None)" .

linkml:observation__valueQuantity a owl:ObjectProperty,
        linkml:SlotDefinition ;
    rdfs:label "observation__valueQuantity" ;
    rdfs:domain <https://example.org/crdch_model/Observation> ;
    rdfs:range <https://example.org/crdch_model/Quantity> ;
    skos:definition "The result of the observation, encoded as a free-text Quantity." ;
    skos:editorialNote "Cardinality: 0..1" ;
    skos:note "One and only one of the value(x) fields must be populated." ;
    linkml:examples "Example(value='', description=None)" .

linkml:observation__valueString a owl:ObjectProperty,
        linkml:SlotDefinition ;
    rdfs:label "observation__valueString" ;
    rdfs:domain <https://example.org/crdch_model/Observation> ;
    rdfs:range <https://example.org/crdch_model/Entity> ;
    skos:definition "The result of the observation, encoded as a free-text string." ;
    skos:editorialNote "Cardinality: 0..1" ;
    skos:note "One and only one of the value(x) fields must be populated." ;
    linkml:examples "Example(value='', description=None)" .

linkml:organization__alias a owl:ObjectProperty,
        linkml:SlotDefinition ;
    rdfs:label "organization__alias" ;
    rdfs:domain <https://example.org/crdch_model/Organization> ;
    rdfs:range <https://example.org/crdch_model/Entity> ;
    skos:definition "A secondary name for the organization such as a short name or abbreviation (e.g. 'NCI')" ;
    skos:editorialNote "Cardinality: 0..1" ;
    linkml:examples "Example(value='', description=None)" .

linkml:organization__id a owl:ObjectProperty,
        linkml:SlotDefinition ;
    rdfs:label "organization__id" ;
    rdfs:domain <https://example.org/crdch_model/Organization> ;
    rdfs:range <https://example.org/crdch_model/Entity> ;
    skos:definition "The 'logical' identifier of the entity within the system of record.  The simple value of this attribute stands for an identifier of this data object within the system, it can be used as a reference from other objects within the same system (i.e. primary and foreign keys), and it should be unique per type of object. The same data object copied to a different system will likely have a different \"id\" in the new system since \"id\" values are system specific and do not represent persistent business identifiers. Business identifiers are assigned outside the information system and are captured in the \"identifier\" field. The \"id\" field is more likely to be a serially or randomly generated value that is assigned to the data object as it is created in a system." ;
    skos:editorialNote "Cardinality: 1..1" ;
    skos:note "FHIR naming conventions are followed here, where 'id' is used for logical identifiers, and 'identifier' for business identifiers.   The identified entity may have a different 'id' in a different system, and have many external business 'identifiers' associated with it. If an \"id\" value can also be considered to be a business identifier, and should be transmissible to other systems, it should be duplicated in the \"identifier\" attribute along with the additional metadata needed to give context to the value of \"id\". An entity in this model that does not have an \"id\" field is considered to be an embeddable entity that can not stand on its own. " ;
    linkml:examples "Example(value='', description=None)" .

linkml:organization__identifier a owl:ObjectProperty,
        linkml:SlotDefinition ;
    rdfs:label "organization__identifier" ;
    rdfs:domain <https://example.org/crdch_model/Organization> ;
    rdfs:range <https://example.org/crdch_model/Identifier> ;
    skos:definition "A 'business' identifier or accession number for the entity, typically as provided by an external system or authority, that are globally unique and persist across implementing systems. Also, since these identifiers are created outside the information system through a specific business process, the Identifier type has additional attributes to capture this additional metadata so the actual identifier values are qualified by the context that created those values. This additional context allows \"identifier\" instances to be transmitted as business data across systems while still being able to trace them back to the system of origin." ;
    skos:editorialNote "Cardinality: 0..m" ;
    skos:note "FHIR naming conventions are followed here, where 'id' is used for logical identifiers which are unique only within a given system, and 'identifier' for business identifiers, which are used to connect entities or share content across systems.  The complex 'Identifier' data type is used  to capture the identifier itself, along with metadata about its source." ;
    linkml:examples "Example(value='', description=None)" .

linkml:organization__name a owl:ObjectProperty,
        linkml:SlotDefinition ;
    rdfs:label "organization__name" ;
    rdfs:domain <https://example.org/crdch_model/Organization> ;
    rdfs:range <https://example.org/crdch_model/Entity> ;
    skos:definition "The full legal name by which the organization is known (e.g. 'National Cancer Institute')" ;
    skos:editorialNote "Cardinality: 0..1" ;
    linkml:examples "Example(value='', description=None)" .

linkml:organization__organization_type a owl:ObjectProperty,
        linkml:SlotDefinition ;
    rdfs:label "organization__organization_type" ;
    rdfs:domain <https://example.org/crdch_model/Organization> ;
    rdfs:range <https://example.org/crdch_model/Entity> ;
    skos:definition "The type of the organization (e.g. 'Cancer Genome Characterization Center')" ;
    skos:editorialNote "Cardinality: 0..1" ;
    skos:note "See dev issues column" ;
    linkml:examples "Example(value='', description=None)" .

linkml:quantity__unit a owl:ObjectProperty,
        linkml:SlotDefinition ;
    rdfs:label "quantity__unit" ;
    rdfs:domain <https://example.org/crdch_model/Quantity> ;
    rdfs:range <http://UNKNOWN.org/enum_CRDCH_Quantity_unit> ;
    skos:definition "A coded or free text (in the .text field) representation of the unit." ;
    skos:editorialNote "Cardinality: 0..1" ;
    linkml:examples "Example(value='', description=None)" .

linkml:quantity__valueCodeableConcept a owl:ObjectProperty,
        linkml:SlotDefinition ;
    rdfs:label "quantity__valueCodeableConcept" ;
    rdfs:domain <https://example.org/crdch_model/Quantity> ;
    rdfs:range <http://UNKNOWN.org/enum_CRDCH_Quantity_valueCodeableConcept> ;
    skos:definition "A coded value representing a quantity (e.g. \"Adjacent (< or = 2cm)\")" ;
    skos:editorialNote "Cardinality: 0..1" ;
    linkml:examples "Example(value='', description=None)" .

linkml:quantity__valueDecimal a owl:ObjectProperty,
        linkml:SlotDefinition ;
    rdfs:label "quantity__valueDecimal" ;
    rdfs:domain <https://example.org/crdch_model/Quantity> ;
    rdfs:range <https://example.org/crdch_model/Entity> ;
    skos:definition "An amount, in the given units (if specified)" ;
    skos:editorialNote "Cardinality: 0..1" ;
    linkml:examples "Example(value='', description=None)" .

linkml:researchProject__associated_timepoint a owl:ObjectProperty,
        linkml:SlotDefinition ;
    rdfs:label "researchProject__associated_timepoint" ;
    rdfs:domain <https://example.org/crdch_model/ResearchProject> ;
    rdfs:range <https://example.org/crdch_model/TimePoint> ;
    skos:definition "A collection of timepoint observations that are relevant to research projects (e.g. date of IACUC approval, date of IRB approval, date of embargo end, etc.)" ;
    skos:editorialNote "Cardinality: 0..m" ;
    linkml:examples "Example(value='', description=None)" .

linkml:researchProject__date_ended a owl:ObjectProperty,
        linkml:SlotDefinition ;
    rdfs:label "researchProject__date_ended" ;
    rdfs:domain <https://example.org/crdch_model/ResearchProject> ;
    rdfs:range <https://example.org/crdch_model/TimePoint> ;
    skos:definition "The date when the research project ended." ;
    skos:editorialNote "Cardinality: 0..1" ;
    linkml:examples "Example(value='', description=None)" .

linkml:researchProject__date_started a owl:ObjectProperty,
        linkml:SlotDefinition ;
    rdfs:label "researchProject__date_started" ;
    rdfs:domain <https://example.org/crdch_model/ResearchProject> ;
    rdfs:range <https://example.org/crdch_model/TimePoint> ;
    skos:definition "The date when the research project began." ;
    skos:editorialNote "Cardinality: 0..1" ;
    linkml:examples "Example(value='', description=None)" .

linkml:researchProject__description a owl:ObjectProperty,
        linkml:SlotDefinition ;
    rdfs:label "researchProject__description" ;
    rdfs:domain <https://example.org/crdch_model/ResearchProject> ;
    rdfs:range <https://example.org/crdch_model/Entity> ;
    skos:definition "An unabridged description of a research program, project, or study." ;
    skos:editorialNote "Cardinality: 0..1" ;
    linkml:examples "Example(value='', description=None)" .

linkml:researchProject__description_shortened a owl:ObjectProperty,
        linkml:SlotDefinition ;
    rdfs:label "researchProject__description_shortened" ;
    rdfs:domain <https://example.org/crdch_model/ResearchProject> ;
    rdfs:range <https://example.org/crdch_model/Entity> ;
    skos:definition "An abbreviated description of a research program, project, or study." ;
    skos:editorialNote "Cardinality: 0..1" ;
    linkml:examples "Example(value='', description=None)" .

linkml:researchProject__id a owl:ObjectProperty,
        linkml:SlotDefinition ;
    rdfs:label "researchProject__id" ;
    rdfs:domain <https://example.org/crdch_model/ResearchProject> ;
    rdfs:range <https://example.org/crdch_model/Entity> ;
    skos:definition "The 'logical' identifier of the entity within the system of record.  The simple value of this attribute stands for an identifier of this data object within the system, it can be used as a reference from other objects within the same system (i.e. primary and foreign keys), and it should be unique per type of object. The same data object copied to a different system will likely have a different \"id\" in the new system since \"id\" values are system specific and do not represent persistent business identifiers. Business identifiers are assigned outside the information system and are captured in the \"identifier\" field. The \"id\" field is more likely to be a serially or randomly generated value that is assigned to the data object as it is created in a system." ;
    skos:editorialNote "Cardinality: 0..1" ;
    skos:note "FHIR naming conventions are followed here, where 'id' is used for logical identifiers, and 'identifier' for business identifiers.   The identified entity may have a different 'id' in a different system, and have many external business 'identifiers' associated with it. If an \"id\" value can also be considered to be a business identifier, and should be transmissible to other systems, it should be duplicated in the \"identifier\" attribute along with the additional metadata needed to give context to the value of \"id\". An entity in this model that does not have an \"id\" field is considered to be an embeddable entity that can not stand on its own. " ;
    linkml:examples "Example(value='', description=None)" .

linkml:researchProject__identifier a owl:ObjectProperty,
        linkml:SlotDefinition ;
    rdfs:label "researchProject__identifier" ;
    rdfs:domain <https://example.org/crdch_model/ResearchProject> ;
    rdfs:range <https://example.org/crdch_model/Identifier> ;
    skos:definition "A 'business' identifier or accession number for the entity, typically as provided by an external system or authority, that are globally unique and persist across implementing systems. Also, since these identifiers are created outside the information system through a specific business process, the Identifier type has additional attributes to capture this additional metadata so the actual identifier values are qualified by the context that created those values. This additional context allows \"identifier\" instances to be transmitted as business data across systems while still being able to trace them back to the system of origin." ;
    skos:editorialNote "Cardinality: 0..m" ;
    skos:note "FHIR naming conventions are followed here, where 'id' is used for logical identifiers which are unique only within a given system, and 'identifier' for business identifiers, which are used to connect entities or share content across systems.  The complex 'Identifier' data type is used  to capture the identifier itself, along with metadata about its source." ;
    linkml:examples "Example(value='', description=None)" .

linkml:researchProject__name a owl:ObjectProperty,
        linkml:SlotDefinition ;
    rdfs:label "researchProject__name" ;
    rdfs:domain <https://example.org/crdch_model/ResearchProject> ;
    rdfs:range <https://example.org/crdch_model/Entity> ;
    skos:definition "An unabridged name of a research program, project, or study." ;
    skos:editorialNote "Cardinality: 0..1" ;
    linkml:examples "Example(value='', description=None)" .

linkml:researchProject__name_shortened a owl:ObjectProperty,
        linkml:SlotDefinition ;
    rdfs:label "researchProject__name_shortened" ;
    rdfs:domain <https://example.org/crdch_model/ResearchProject> ;
    rdfs:range <https://example.org/crdch_model/Entity> ;
    skos:definition "An abbreviated name of a research program, project, or study." ;
    skos:editorialNote "Cardinality: 0..1" ;
    linkml:examples "Example(value='', description=None)" .

linkml:researchProject__part_of a owl:ObjectProperty,
        linkml:SlotDefinition ;
    rdfs:label "researchProject__part_of" ;
    rdfs:domain <https://example.org/crdch_model/ResearchProject> ;
    rdfs:range <https://example.org/crdch_model/ResearchProject> ;
    skos:definition "A reference to a parent ResearchProject (e.g. a link to the overarching CPTAC ResearchProject from a substudy of CPTAC)" ;
    skos:editorialNote "Cardinality: 0..m" ;
    linkml:examples "Example(value='', description=None)" .

linkml:researchProject__primary_anatomic_site a owl:ObjectProperty,
        linkml:SlotDefinition ;
    rdfs:label "researchProject__primary_anatomic_site" ;
    rdfs:domain <https://example.org/crdch_model/ResearchProject> ;
    rdfs:range <https://example.org/crdch_model/BodySite> ;
    skos:definition "The text term used to describe the general location of the malignant disease, as categorized by the World Health Organization's (WHO) International Classification of Diseases for Oncology (ICD-O).  In the context of ResearchProject, this attribute captures the anatomic sites of research interest." ;
    skos:editorialNote "Cardinality: 0..m" ;
    linkml:examples "Example(value='', description=None)" .

linkml:researchProject__research_project_type a owl:ObjectProperty,
        linkml:SlotDefinition ;
    rdfs:label "researchProject__research_project_type" ;
    rdfs:domain <https://example.org/crdch_model/ResearchProject> ;
    rdfs:range <http://UNKNOWN.org/enum_CRDCH_ResearchProject_research_project_type> ;
    skos:definition "The 'type' of ResearchProject represented (e.g. a broad-based Program like 'CPTAC' or a more focused Project like 'CPTAC PDAC Discovery Study')" ;
    skos:editorialNote "Cardinality: 1..1" ;
    linkml:examples "Example(value='Clinical Trial', description=None)",
        "Example(value='Program', description=None)",
        "Example(value='Project', description=None)" .

linkml:researchProject__sponsor a owl:ObjectProperty,
        linkml:SlotDefinition ;
    rdfs:label "researchProject__sponsor" ;
    rdfs:domain <https://example.org/crdch_model/ResearchProject> ;
    rdfs:range <https://example.org/crdch_model/Entity> ;
    skos:definition "An entity that is responsible for the initiation, management, and/or financing of a research project." ;
    skos:editorialNote "Cardinality: 0..m" ;
    linkml:examples "Example(value='', description=None)" .

linkml:researchProject__url a owl:ObjectProperty,
        linkml:SlotDefinition ;
    rdfs:label "researchProject__url" ;
    rdfs:domain <https://example.org/crdch_model/ResearchProject> ;
    rdfs:range <https://example.org/crdch_model/Entity> ;
    skos:definition "A URL address for a resource that provides information about a research program, project, or study." ;
    skos:editorialNote "Cardinality: 0..m" ;
    linkml:examples "Example(value='', description=None)" .

linkml:researchSubject__age_at_enrollment a owl:ObjectProperty,
        linkml:SlotDefinition ;
    rdfs:label "researchSubject__age_at_enrollment" ;
    rdfs:domain <https://example.org/crdch_model/ResearchSubject> ;
    rdfs:range <https://example.org/crdch_model/Quantity> ;
    skos:definition "The age in days when the Subject enrolled on the ResearchProject" ;
    skos:editorialNote "Cardinality: 0..1" ;
    linkml:examples "Example(value='', description=None)" .

linkml:researchSubject__associated_subject a owl:ObjectProperty,
        linkml:SlotDefinition ;
    rdfs:label "researchSubject__associated_subject" ;
    rdfs:domain <https://example.org/crdch_model/ResearchSubject> ;
    rdfs:range <https://example.org/crdch_model/Subject> ;
    skos:definition "A reference to the Subject that is this ResearchSubject" ;
    skos:editorialNote "Cardinality: 1..1" ;
    linkml:examples "Example(value='', description=None)" .

linkml:researchSubject__comorbid_diagnosis a owl:ObjectProperty,
        linkml:SlotDefinition ;
    rdfs:label "researchSubject__comorbid_diagnosis" ;
    rdfs:domain <https://example.org/crdch_model/ResearchSubject> ;
    rdfs:range <https://example.org/crdch_model/Diagnosis> ;
    skos:definition "One or more diagnosis instance that are comorbid with the primary_diagnosis that qualified a subject for inclusion on a ResearchProject" ;
    skos:editorialNote "Cardinality: 0..m" ;
    skos:note "In cases where a data source has sufficiently detailed information on comorbid diagnoses related to the diagnosis that qualified a subject for inclusion on a ResearchProject, a Diagnosis entity should be instantiated and included here." ;
    linkml:examples "Example(value='', description=None)" .

linkml:researchSubject__description a owl:ObjectProperty,
        linkml:SlotDefinition ;
    rdfs:label "researchSubject__description" ;
    rdfs:domain <https://example.org/crdch_model/ResearchSubject> ;
    rdfs:range <https://example.org/crdch_model/Entity> ;
    skos:definition "A free text field to capture additional info/explanation about the research subject." ;
    skos:editorialNote "Cardinality: 0..1" ;
    linkml:examples "Example(value='', description=None)" .

linkml:researchSubject__id a owl:ObjectProperty,
        linkml:SlotDefinition ;
    rdfs:label "researchSubject__id" ;
    rdfs:domain <https://example.org/crdch_model/ResearchSubject> ;
    rdfs:range <https://example.org/crdch_model/Entity> ;
    skos:definition "The 'logical' identifier of the entity within the system of record.  The simple value of this attribute stands for an identifier of this data object within the system, it can be used as a reference from other objects within the same system (i.e. primary and foreign keys), and it should be unique per type of object. The same data object copied to a different system will likely have a different \"id\" in the new system since \"id\" values are system specific and do not represent persistent business identifiers. Business identifiers are assigned outside the information system and are captured in the \"identifier\" field. The \"id\" field is more likely to be a serially or randomly generated value that is assigned to the data object as it is created in a system." ;
    skos:editorialNote "Cardinality: 1..1" ;
    skos:note "FHIR naming conventions are followed here, where 'id' is used for logical identifiers, and 'identifier' for business identifiers.   The identified entity may have a different 'id' in a different system, and have many external business 'identifiers' associated with it. If an \"id\" value can also be considered to be a business identifier, and should be transmissible to other systems, it should be duplicated in the \"identifier\" attribute along with the additional metadata needed to give context to the value of \"id\". An entity in this model that does not have an \"id\" field is considered to be an embeddable entity that can not stand on its own. " ;
    linkml:examples "Example(value='', description=None)" .

linkml:researchSubject__identifier a owl:ObjectProperty,
        linkml:SlotDefinition ;
    rdfs:label "researchSubject__identifier" ;
    rdfs:domain <https://example.org/crdch_model/ResearchSubject> ;
    rdfs:range <https://example.org/crdch_model/Identifier> ;
    skos:definition "A 'business' identifier or accession number for the entity, typically as provided by an external system or authority, that are globally unique and persist across implementing systems. Also, since these identifiers are created outside the information system through a specific business process, the Identifier type has additional attributes to capture this additional metadata so the actual identifier values are qualified by the context that created those values. This additional context allows \"identifier\" instances to be transmitted as business data across systems while still being able to trace them back to the system of origin." ;
    skos:editorialNote "Cardinality: 0..m" ;
    skos:note "FHIR naming conventions are followed here, where 'id' is used for logical identifiers which are unique only within a given system, and 'identifier' for business identifiers, which are used to connect entities or share content across systems.  The complex 'Identifier' data type is used  to capture the identifier itself, along with metadata about its source." ;
    linkml:examples "Example(value='', description=None)" .

linkml:researchSubject__index_timepoint a owl:ObjectProperty,
        linkml:SlotDefinition ;
    rdfs:label "researchSubject__index_timepoint" ;
    rdfs:domain <https://example.org/crdch_model/ResearchSubject> ;
    rdfs:range <http://UNKNOWN.org/enum_CRDCH_ResearchSubject_index_timepoint> ;
    skos:definition "The text term used to describe the reference or anchor date used for date obfuscation, where a single date is obscured by creating one or more date ranges in relation to this date." ;
    skos:editorialNote "Cardinality: 0..1" ;
    linkml:examples "Example(value='', description=None)",
        "Example(value='Diagnosis', description=None)",
        "Example(value='First Patient Visit', description=None)",
        "Example(value='First Treatment', description=None)" .

linkml:researchSubject__member_of_research_project a owl:ObjectProperty,
        linkml:SlotDefinition ;
    rdfs:label "researchSubject__member_of_research_project" ;
    rdfs:domain <https://example.org/crdch_model/ResearchSubject> ;
    rdfs:range <https://example.org/crdch_model/ResearchProject> ;
    skos:definition "A reference to the Study(s) of which this ResearchSubject is a member" ;
    skos:editorialNote "Cardinality: 0..1" ;
    linkml:examples "Example(value='', description=None)" .

linkml:researchSubject__originating_site a owl:ObjectProperty,
        linkml:SlotDefinition ;
    rdfs:label "researchSubject__originating_site" ;
    rdfs:domain <https://example.org/crdch_model/ResearchSubject> ;
    rdfs:range <https://example.org/crdch_model/Organization> ;
    skos:definition "The Organization at which a subject was enrolled on a ResearchProject." ;
    skos:editorialNote "Cardinality: 0..1" ;
    linkml:examples "Example(value='', description=None)" .

linkml:researchSubject__primary_diagnosis a owl:ObjectProperty,
        linkml:SlotDefinition ;
    rdfs:label "researchSubject__primary_diagnosis" ;
    rdfs:domain <https://example.org/crdch_model/ResearchSubject> ;
    rdfs:range <https://example.org/crdch_model/Diagnosis> ;
    skos:definition "The diagnosis instance that qualified a subject for inclusion on a ResearchProject" ;
    skos:editorialNote "Cardinality: 0..m" ;
    skos:note "In cases where a data source has sufficiently detailed information on the diagnosis that qualifies a subject for inclusion on a ResearchProject, a Diagnosis entity should be instantiated and included here." ;
    linkml:examples "Example(value='', description=None)" .

linkml:researchSubject__primary_diagnosis_condition a owl:ObjectProperty,
        linkml:SlotDefinition ;
    rdfs:label "researchSubject__primary_diagnosis_condition" ;
    rdfs:domain <https://example.org/crdch_model/ResearchSubject> ;
    rdfs:range <http://UNKNOWN.org/enum_CRDCH_ResearchSubject_primary_diagnosis_condition> ;
    skos:definition "The text term used to describe the type of malignant disease, as categorized by the World Health Organization's (WHO) International Classification of Diseases for Oncology (ICD-O).   This attribute represents the disease that qualified the subject for inclusion on the ResearchProject" ;
    skos:editorialNote "Cardinality: 0..1" ;
    skos:note "In cases where a data source does not have sufficiently detailed information on the diagnosis that qualified a subject for inclusion on a ResearchProject in order to instantiate a Diagnosis entity, the primary_diagnosis_condition attribute should be populated when available." ;
    linkml:examples "Example(value='', description=None)",
        "Example(value='Acinar Cell Neoplasms', description=None)",
        "Example(value='Adenomas and Adenocarcinomas', description=None)",
        "Example(value='Adnexal and Skin Appendage Neoplasms', description=None)" .

linkml:researchSubject__primary_diagnosis_site a owl:ObjectProperty,
        linkml:SlotDefinition ;
    rdfs:label "researchSubject__primary_diagnosis_site" ;
    rdfs:domain <https://example.org/crdch_model/ResearchSubject> ;
    rdfs:range <https://example.org/crdch_model/BodySite> ;
    skos:definition "The text term used to describe the primary site of disease, as categorized by the World Health Organization's (WHO) International Classification of Diseases for Oncology (ICD-O). This categorization groups cases into general categories.  This attribute represents the primary site of disease that qualified the subject for inclusion on the ResearchProject." ;
    skos:editorialNote "Cardinality: 0..1" ;
    skos:note "In cases where a data source does not have sufficiently detailed information on the diagnosis that qualified a subject for inclusion on a ResearchProject in order to instantiate a Diagnosis entity, the primary_diagnosis_site attribute should be populated when available." ;
    linkml:examples "Example(value='', description=None)",
        "Example(value='Accessory sinuses', description=None)",
        "Example(value='Adrenal gland', description=None)",
        "Example(value='Anus and anal canal', description=None)" .

linkml:specimenContainer__additive a owl:ObjectProperty,
        linkml:SlotDefinition ;
    rdfs:label "specimenContainer__additive" ;
    rdfs:domain <https://example.org/crdch_model/SpecimenContainer> ;
    rdfs:range <https://example.org/crdch_model/Substance> ;
    skos:definition "A material substance added to the container (typically to support the primary contained object - e.g. culture media to support cell growth)" ;
    skos:editorialNote "Cardinality: 0..m" ;
    linkml:examples "Example(value='DMEM', description=None)",
        "Example(value='DMEM+Serum', description=None)",
        "Example(value='RPMI', description=None)",
        "Example(value='RPMI+Serum', description=None)" .

linkml:specimenContainer__container_number a owl:ObjectProperty,
        linkml:SlotDefinition ;
    rdfs:label "specimenContainer__container_number" ;
    rdfs:domain <https://example.org/crdch_model/SpecimenContainer> ;
    rdfs:range <https://example.org/crdch_model/Entity> ;
    skos:definition "Informal number by which the container is referenced  or identified (e.g. a slide number, or a well number in a plate)" ;
    skos:editorialNote "Cardinality: 0..1" ;
    linkml:examples "Example(value='', description=None)" .

linkml:specimenContainer__container_type a owl:ObjectProperty,
        linkml:SlotDefinition ;
    rdfs:label "specimenContainer__container_type" ;
    rdfs:domain <https://example.org/crdch_model/SpecimenContainer> ;
    rdfs:range <http://UNKNOWN.org/enum_CRDCH_SpecimenContainer_container_type> ;
    skos:definition "The kind of the container." ;
    skos:editorialNote "Cardinality: 0..1" ;
    linkml:examples "Example(value='Capillary blood collection tube', description=None)",
        "Example(value='Cell culture flask', description=None)",
        "Example(value='Glass slide', description=None)",
        "Example(value='Sputum specimen container', description=None)" .

linkml:specimenContainer__id a owl:ObjectProperty,
        linkml:SlotDefinition ;
    rdfs:label "specimenContainer__id" ;
    rdfs:domain <https://example.org/crdch_model/SpecimenContainer> ;
    rdfs:range <https://example.org/crdch_model/Entity> ;
    skos:definition "The 'logical' identifier of the entity within the system of record.  The simple value of this attribute stands for an identifier of this data object within the system, it can be used as a reference from other objects within the same system (i.e. primary and foreign keys), and it should be unique per type of object. The same data object copied to a different system will likely have a different \"id\" in the new system since \"id\" values are system specific and do not represent persistent business identifiers. Business identifiers are assigned outside the information system and are captured in the \"identifier\" field. The \"id\" field is more likely to be a serially or randomly generated value that is assigned to the data object as it is created in a system." ;
    skos:editorialNote "Cardinality: 0..1" ;
    skos:note "FHIR naming conventions are followed here, where 'id' is used for logical identifiers, and 'identifier' for business identifiers.   The identified entity may have a different 'id' in a different system, and have many external business 'identifiers' associated with it. If an \"id\" value can also be considered to be a business identifier, and should be transmissible to other systems, it should be duplicated in the \"identifier\" attribute along with the additional metadata needed to give context to the value of \"id\". An entity in this model that does not have an \"id\" field is considered to be an embeddable entity that can not stand on its own. " ;
    linkml:examples "Example(value='', description=None)" .

linkml:specimenContainer__identifier a owl:ObjectProperty,
        linkml:SlotDefinition ;
    rdfs:label "specimenContainer__identifier" ;
    rdfs:domain <https://example.org/crdch_model/SpecimenContainer> ;
    rdfs:range <https://example.org/crdch_model/Identifier> ;
    skos:definition "A 'business' identifier or accession number for the entity, typically as provided by an external system or authority, that are globally unique and persist across implementing systems. Also, since these identifiers are created outside the information system through a specific business process, the Identifier type has additional attributes to capture this additional metadata so the actual identifier values are qualified by the context that created those values. This additional context allows \"identifier\" instances to be transmitted as business data across systems while still being able to trace them back to the system of origin." ;
    skos:editorialNote "Cardinality: 0..m" ;
    skos:note "FHIR naming conventions are followed here, where 'id' is used for logical identifiers which are unique only within a given system, and 'identifier' for business identifiers, which are used to connect entities or share content across systems.  The complex 'Identifier' data type is used  to capture the identifier itself, along with metadata about its source." ;
    linkml:examples "Example(value='', description=None)" .

linkml:specimenContainer__parent_container a owl:ObjectProperty,
        linkml:SlotDefinition ;
    rdfs:label "specimenContainer__parent_container" ;
    rdfs:domain <https://example.org/crdch_model/SpecimenContainer> ;
    rdfs:range <https://example.org/crdch_model/SpecimenContainer> ;
    skos:definition "A larger container of which this container is a part (e.g. the complete 96-well plate of which a single well is a part)" ;
    skos:editorialNote "Cardinality: 0..1" ;
    linkml:examples "Example(value='', description=None)" .

linkml:specimenCreationActivity__activity_type a owl:ObjectProperty,
        linkml:SlotDefinition ;
    rdfs:label "specimenCreationActivity__activity_type" ;
    rdfs:domain <https://example.org/crdch_model/SpecimenCreationActivity> ;
    rdfs:range <http://UNKNOWN.org/enum_CRDCH_SpecimenCreationActivity_activity_type> ;
    skos:definition "The high-level type of creation activity." ;
    skos:editorialNote "Cardinality: 0..1" ;
    skos:note "At present our model collapses two types of processes through which specimens are created (initial collection from source, and derivation from an existing specimen).  The 'category' is a flag to indicate which applies to a given instance, so that more specific recommendations about data entry in certain fields can be specified." ;
    linkml:examples "Example(value='Collection from Source', description=None)",
        "Example(value='Derivation from Specimen', description=None)" .

linkml:specimenCreationActivity__additive a owl:ObjectProperty,
        linkml:SlotDefinition ;
    rdfs:label "specimenCreationActivity__additive" ;
    rdfs:domain <https://example.org/crdch_model/SpecimenCreationActivity> ;
    rdfs:range <https://example.org/crdch_model/Substance> ;
    skos:definition "A type of material or reagent used applied as input when creating a specimen." ;
    skos:editorialNote "Cardinality: 0..m" ;
    linkml:examples "Example(value='', description=None)" .

linkml:specimenCreationActivity__collection_method_type a owl:ObjectProperty,
        linkml:SlotDefinition ;
    rdfs:label "specimenCreationActivity__collection_method_type" ;
    rdfs:domain <https://example.org/crdch_model/SpecimenCreationActivity> ;
    rdfs:range <http://UNKNOWN.org/enum_CRDCH_SpecimenCreationActivity_collection_method_type> ;
    skos:definition "The type of method applied in collecting a sample from its original source." ;
    skos:editorialNote "Cardinality: 0..1" ;
    skos:note "This attribute applies only when the Specimen.category = 'original'." ;
    linkml:examples "Example(value='Anterior Resection of Rectum', description=None)",
        "Example(value='Ascites Drainage', description=None)",
        "Example(value='Excisional Biopsy', description=None)",
        "Example(value='Specimen Pooling', description=None)" .

linkml:specimenCreationActivity__collection_site a owl:ObjectProperty,
        linkml:SlotDefinition ;
    rdfs:label "specimenCreationActivity__collection_site" ;
    rdfs:domain <https://example.org/crdch_model/SpecimenCreationActivity> ;
    rdfs:range <https://example.org/crdch_model/BodySite> ;
    skos:definition "The anatomic site from which a specimen was collected." ;
    skos:editorialNote "Cardinality: 0..1" ;
    skos:note "This attribute is used when SpecimenCreationActivity.activity_type = 'Collection from Source'." ;
    linkml:examples "Example(value='Abdomen', description=None)",
        "Example(value='Abdominal Wall', description=None)",
        "Example(value='Acetabulum', description=None)" .

linkml:specimenCreationActivity__date_ended a owl:ObjectProperty,
        linkml:SlotDefinition ;
    rdfs:label "specimenCreationActivity__date_ended" ;
    rdfs:domain <https://example.org/crdch_model/SpecimenCreationActivity> ;
    rdfs:range <https://example.org/crdch_model/TimePoint> ;
    skos:definition "The date when the activity ended (in this case, a specimen creation event)." ;
    skos:editorialNote "Cardinality: 0..1" ;
    skos:note "To allow for more precise specification of dates when an activity was performed, we provide date_started and date_ended attributes.  If source data only provides a single date, it SHOULD be entered as both the date_started and date_ended." ;
    linkml:examples "Example(value='', description=None)" .

linkml:specimenCreationActivity__date_started a owl:ObjectProperty,
        linkml:SlotDefinition ;
    rdfs:label "specimenCreationActivity__date_started" ;
    rdfs:domain <https://example.org/crdch_model/SpecimenCreationActivity> ;
    rdfs:range <https://example.org/crdch_model/TimePoint> ;
    skos:definition "The date when the activity began (in this case, a specimen creation event)." ;
    skos:editorialNote "Cardinality: 0..1" ;
    skos:note "To allow for more precise specification of dates when an activity was performed, we provide date_started and date_ended attributes.  If source data only provides a single date, it SHOULD be entered as both the date_started and date_ended." ;
    linkml:examples "Example(value='', description=None)" .

linkml:specimenCreationActivity__derivation_method_type a owl:ObjectProperty,
        linkml:SlotDefinition ;
    rdfs:label "specimenCreationActivity__derivation_method_type" ;
    rdfs:domain <https://example.org/crdch_model/SpecimenCreationActivity> ;
    rdfs:range <http://UNKNOWN.org/enum_CRDCH_SpecimenCreationActivity_derivation_method_type> ;
    skos:definition "The type of method applied to derive a new specimen from an existing one." ;
    skos:editorialNote "Cardinality: 0..1" ;
    skos:note "This attribute applies only when Specimen.category = 'portion', 'aliquot', 'analyte', or 'slide'." ;
    linkml:examples "Example(value='Cryosectioning', description=None)",
        "Example(value='NotReported', description=None)",
        "Example(value='Other', description=None)",
        "Example(value='Sectioning', description=None)",
        "Example(value='Slidingmicrotome', description=None)",
        "Example(value='Tissuemolds', description=None)",
        "Example(value='Unknown', description=None)",
        "Example(value='Vibratome', description=None)" .

linkml:specimenCreationActivity__execution_condition_observation a owl:ObjectProperty,
        linkml:SlotDefinition ;
    rdfs:label "specimenCreationActivity__execution_condition_observation" ;
    rdfs:domain <https://example.org/crdch_model/SpecimenCreationActivity> ;
    rdfs:range <https://example.org/crdch_model/ExecutionConditionObservation> ;
    skos:definition "Information describing the environmental conditions in which an activity, or a specific part of an activity, was performed." ;
    skos:editorialNote "Cardinality: 0..m" ;
    linkml:examples "Example(value='', description=None)" .

linkml:specimenCreationActivity__execution_time_observation a owl:ObjectProperty,
        linkml:SlotDefinition ;
    rdfs:label "specimenCreationActivity__execution_time_observation" ;
    rdfs:domain <https://example.org/crdch_model/SpecimenCreationActivity> ;
    rdfs:range <https://example.org/crdch_model/ExecutionTimeObservation> ;
    skos:definition "Information describing how long certain parts on an activity took to complete." ;
    skos:editorialNote "Cardinality: 0..m" ;
    linkml:examples "Example(value='', description=None)" .

linkml:specimenCreationActivity__performed_by a owl:ObjectProperty,
        linkml:SlotDefinition ;
    rdfs:label "specimenCreationActivity__performed_by" ;
    rdfs:domain <https://example.org/crdch_model/SpecimenCreationActivity> ;
    rdfs:range <https://example.org/crdch_model/Organization> ;
    skos:definition "The organization or group that performed the activity." ;
    skos:editorialNote "Cardinality: 0..1" ;
    linkml:examples "Example(value='', description=None)" .

linkml:specimenCreationActivity__quantity_collected a owl:ObjectProperty,
        linkml:SlotDefinition ;
    rdfs:label "specimenCreationActivity__quantity_collected" ;
    rdfs:domain <https://example.org/crdch_model/SpecimenCreationActivity> ;
    rdfs:range <https://example.org/crdch_model/Quantity> ;
    skos:definition "The quantity of material in the specimen as originally collected from its original source material (prior to downstream portioning or processing)" ;
    skos:editorialNote "Cardinality: 0..1" ;
    skos:note "This attribute applies only when Specimen.category='initial sample'." ;
    linkml:examples "Example(value='', description=None)" .

linkml:specimenCreationActivity__specimen_order a owl:ObjectProperty,
        linkml:SlotDefinition ;
    rdfs:label "specimenCreationActivity__specimen_order" ;
    rdfs:domain <https://example.org/crdch_model/SpecimenCreationActivity> ;
    rdfs:range <https://example.org/crdch_model/Entity> ;
    skos:definition "A numeric value that represents the sequential order of this creation activity relative to those producing other specimens from the same source material or parent specimen." ;
    skos:editorialNote "Cardinality: 0..1" ;
    linkml:examples "Example(value='', description=None)" .

linkml:specimenProcessingActivity__activity_type a owl:ObjectProperty,
        linkml:SlotDefinition ;
    rdfs:label "specimenProcessingActivity__activity_type" ;
    rdfs:domain <https://example.org/crdch_model/SpecimenProcessingActivity> ;
    rdfs:range <http://UNKNOWN.org/enum_CRDCH_SpecimenProcessingActivity_activity_type> ;
    skos:definition "The high-level type of processing activity" ;
    skos:editorialNote "Cardinality: 0..1" ;
    linkml:examples "Example(value='Fixation', description=None)",
        "Example(value='Freezing', description=None)",
        "Example(value='Mounting', description=None)",
        "Example(value='Preservation', description=None)" .

linkml:specimenProcessingActivity__additive a owl:ObjectProperty,
        linkml:SlotDefinition ;
    rdfs:label "specimenProcessingActivity__additive" ;
    rdfs:domain <https://example.org/crdch_model/SpecimenProcessingActivity> ;
    rdfs:range <https://example.org/crdch_model/Substance> ;
    skos:definition "A type of material or reagent used as input when processing the specimen" ;
    skos:editorialNote "Cardinality: 0..m" ;
    linkml:examples "Example(value='Formalin', description=None)" .

linkml:specimenProcessingActivity__date_ended a owl:ObjectProperty,
        linkml:SlotDefinition ;
    rdfs:label "specimenProcessingActivity__date_ended" ;
    rdfs:domain <https://example.org/crdch_model/SpecimenProcessingActivity> ;
    rdfs:range <https://example.org/crdch_model/TimePoint> ;
    skos:definition "The date when the activity began (in this case, a specimen processing event)." ;
    skos:editorialNote "Cardinality: 0..1" ;
    skos:note "To allow for more precise specification of dates when an activity was performed, we provide date_started and date_ended attributes.  If source data only provides a single date, it SHOULD be entered as both the date_started and date_ended." ;
    linkml:examples "Example(value='', description=None)" .

linkml:specimenProcessingActivity__date_started a owl:ObjectProperty,
        linkml:SlotDefinition ;
    rdfs:label "specimenProcessingActivity__date_started" ;
    rdfs:domain <https://example.org/crdch_model/SpecimenProcessingActivity> ;
    rdfs:range <https://example.org/crdch_model/TimePoint> ;
    skos:definition "The date when the activity began (in this case, a specimen processing event)." ;
    skos:editorialNote "Cardinality: 0..1" ;
    skos:note "To allow for more precise specification of dates when an activity was performed, we provide date_started and date_ended attributes.  If source data only provides a single date, it SHOULD be entered as both the date_started and date_ended." ;
    linkml:examples "Example(value='', description=None)" .

linkml:specimenProcessingActivity__duration a owl:ObjectProperty,
        linkml:SlotDefinition ;
    rdfs:label "specimenProcessingActivity__duration" ;
    rdfs:domain <https://example.org/crdch_model/SpecimenProcessingActivity> ;
    rdfs:range <https://example.org/crdch_model/Quantity> ;
    skos:definition "The length of time over which the activity was performed." ;
    linkml:examples "Example(value='', description=None)" .

linkml:specimenProcessingActivity__execution_condition_observation a owl:ObjectProperty,
        linkml:SlotDefinition ;
    rdfs:label "specimenProcessingActivity__execution_condition_observation" ;
    rdfs:domain <https://example.org/crdch_model/SpecimenProcessingActivity> ;
    rdfs:range <https://example.org/crdch_model/ExecutionConditionObservation> ;
    skos:definition "Information describing the environmental conditions in which an activity, or a specific part of an activity, was performed." ;
    skos:editorialNote "Cardinality: 0..m" ;
    linkml:examples "Example(value='', description=None)" .

linkml:specimenProcessingActivity__execution_time_observation a owl:ObjectProperty,
        linkml:SlotDefinition ;
    rdfs:label "specimenProcessingActivity__execution_time_observation" ;
    rdfs:domain <https://example.org/crdch_model/SpecimenProcessingActivity> ;
    rdfs:range <https://example.org/crdch_model/ExecutionTimeObservation> ;
    skos:definition "Information describing how long certain parts on an activity took to complete." ;
    skos:editorialNote "Cardinality: 0..m" ;
    linkml:examples "Example(value='', description=None)" .

linkml:specimenProcessingActivity__method_type a owl:ObjectProperty,
        linkml:SlotDefinition ;
    rdfs:label "specimenProcessingActivity__method_type" ;
    rdfs:domain <https://example.org/crdch_model/SpecimenProcessingActivity> ;
    rdfs:range <http://UNKNOWN.org/enum_CRDCH_SpecimenProcessingActivity_method_type> ;
    skos:definition "A specific type of method or procedure performed to process the specimen" ;
    skos:editorialNote "Cardinality: 0..1" ;
    linkml:examples "Example(value='Cryopreservation in dry ice (dead tissue)', description=None)",
        "Example(value='Cryopreservation in liquid nitrogen (dead tissue)', description=None)",
        "Example(value='Formalin fixed paraffin embedded (FFPE)', description=None)",
        "Example(value='Formalin fixed-buffered', description=None)",
        "Example(value='Formalin fixed-unbuffered', description=None)",
        "Example(value='OCT', description=None)",
        "Example(value='Snap Freezing', description=None)" .

linkml:specimenProcessingActivity__performed_by a owl:ObjectProperty,
        linkml:SlotDefinition ;
    rdfs:label "specimenProcessingActivity__performed_by" ;
    rdfs:domain <https://example.org/crdch_model/SpecimenProcessingActivity> ;
    rdfs:range <https://example.org/crdch_model/Organization> ;
    skos:definition "The organization or group that performed the activity." ;
    skos:editorialNote "Cardinality: 0..1" ;
    linkml:examples "Example(value='', description=None)" .

linkml:specimenQualityObservation__category a owl:ObjectProperty,
        linkml:SlotDefinition ;
    rdfs:label "specimenQualityObservation__category" ;
    rdfs:domain <https://example.org/crdch_model/SpecimenQualityObservation> ;
    rdfs:range <http://UNKNOWN.org/enum_CRDCH_SpecimenQualityObservation_category> ;
    skos:definition "The general category of observation described" ;
    skos:editorialNote "Cardinality: 0..0" ;
    skos:note "Use only if we don't define named subtypes of Observation for specific categories." ;
    linkml:examples "Example(value='', description=None)" .

linkml:specimenQualityObservation__focus a owl:ObjectProperty,
        linkml:SlotDefinition ;
    rdfs:label "specimenQualityObservation__focus" ;
    rdfs:domain <https://example.org/crdch_model/SpecimenQualityObservation> ;
    rdfs:range <https://example.org/crdch_model/Entity> ;
    skos:definition "The entity or entities directly observed/measured in generating an observation result." ;
    skos:editorialNote "Cardinality: 0..m" ;
    skos:note "The 'focus', 'subject', and 'specimen' fields are useful when data creators want an Observation object to stand on its own, so it can point back to the entities it is about.  These fields are not needed when an Observation is embedded in a Specimen or other entity, where focus, subject, and specimen can be determined from context. " ;
    linkml:examples "Example(value='', description=None)" .

linkml:specimenQualityObservation__id a owl:ObjectProperty,
        linkml:SlotDefinition ;
    rdfs:label "specimenQualityObservation__id" ;
    rdfs:domain <https://example.org/crdch_model/SpecimenQualityObservation> ;
    rdfs:range <https://example.org/crdch_model/Entity> ;
    skos:definition "The 'logical' identifier of the entity within the system of record.  The simple value of this attribute stands for an identifier of this data object within the system, it can be used as a reference from other objects within the same system (i.e. primary and foreign keys), and it should be unique per type of object. The same data object copied to a different system will likely have a different \"id\" in the new system since \"id\" values are system specific and do not represent persistent business identifiers. Business identifiers are assigned outside the information system and are captured in the \"identifier\" field. The \"id\" field is more likely to be a serially or randomly generated value that is assigned to the data object as it is created in a system." ;
    skos:editorialNote "Cardinality: 0..0" ;
    skos:note "FHIR naming conventions are followed here, where 'id' is used for logical identifiers, and 'identifier' for business identifiers.   The identified entity may have a different 'id' in a different system, and have many external business 'identifiers' associated with it. If an \"id\" value can also be considered to be a business identifier, and should be transmissible to other systems, it should be duplicated in the \"identifier\" attribute along with the additional metadata needed to give context to the value of \"id\". An entity in this model that does not have an \"id\" field is considered to be an embeddable entity that can not stand on its own. " ;
    linkml:examples "Example(value='', description=None)" .

linkml:specimenQualityObservation__method_type a owl:ObjectProperty,
        linkml:SlotDefinition ;
    rdfs:label "specimenQualityObservation__method_type" ;
    rdfs:domain <https://example.org/crdch_model/SpecimenQualityObservation> ;
    rdfs:range <http://UNKNOWN.org/enum_CRDCH_SpecimenQualityObservation_method_type> ;
    skos:definition "A type of method used in generating the Observation result." ;
    skos:editorialNote "Cardinality: 0..m" ;
    skos:note "This may be a type of observational, measurement, experimental, or computational method specifying how to generate data (e.g. 'manual counting', 'bright field microscopy',). Or a Guideline or SOP specifying how to interpret data and/or encode the result of an  Observation (e.g. a Cancer Staging system such as that defined by the AJCC, or variant interpretation guideline such as that provided by the ACMG)." ;
    linkml:examples "Example(value='', description=None)" .

linkml:specimenQualityObservation__observation_type a owl:ObjectProperty,
        linkml:SlotDefinition ;
    rdfs:label "specimenQualityObservation__observation_type" ;
    rdfs:domain <https://example.org/crdch_model/SpecimenQualityObservation> ;
    rdfs:range <http://UNKNOWN.org/enum_CRDCH_SpecimenQualityObservation_observation_type> ;
    skos:definition "The specific type of observation made - i.e. the feature or characteristic that was observed, measured, estimated, etc.." ;
    skos:editorialNote "Cardinality: 1..1" ;
    skos:note "This field holds the 'key' in the core key-value pair comprised of the observation_type field and the relevant value(s) field." ;
    linkml:examples "Example(value='', description=None)" .

linkml:specimenQualityObservation__performed_by a owl:ObjectProperty,
        linkml:SlotDefinition ;
    rdfs:label "specimenQualityObservation__performed_by" ;
    rdfs:domain <https://example.org/crdch_model/SpecimenQualityObservation> ;
    rdfs:range <https://example.org/crdch_model/Organization> ;
    skos:definition "The organization or group that performed the observation activity." ;
    skos:editorialNote "Cardinality: 0..1" ;
    linkml:examples "Example(value='', description=None)" .

linkml:specimenQualityObservation__subject a owl:ObjectProperty,
        linkml:SlotDefinition ;
    rdfs:label "specimenQualityObservation__subject" ;
    rdfs:domain <https://example.org/crdch_model/SpecimenQualityObservation> ;
    rdfs:range <https://example.org/crdch_model/Subject> ;
    skos:definition "The patient that the observation is about (if not the direct focus).  e.g. observations are often made on specimens derived from a patient, or other entities related to a patient, that ultimately tell us something about the patient of interest." ;
    skos:editorialNote "Cardinality: 0..1" ;
    linkml:examples "Example(value='', description=None)" .

linkml:specimenQualityObservation__valueQuantity a owl:ObjectProperty,
        linkml:SlotDefinition ;
    rdfs:label "specimenQualityObservation__valueQuantity" ;
    rdfs:domain <https://example.org/crdch_model/SpecimenQualityObservation> ;
    rdfs:range <https://example.org/crdch_model/Quantity> ;
    skos:definition "The result of the observation, encoded as a free-text Quantity." ;
    skos:editorialNote "Cardinality: 1..1" ;
    skos:note "One and only one of the value(x) fields must be populated." ;
    linkml:examples "Example(value='', description=None)" .

linkml:specimenQuantityObservation__category a owl:ObjectProperty,
        linkml:SlotDefinition ;
    rdfs:label "specimenQuantityObservation__category" ;
    rdfs:domain <https://example.org/crdch_model/SpecimenQuantityObservation> ;
    rdfs:range <http://UNKNOWN.org/enum_CRDCH_SpecimenQuantityObservation_category> ;
    skos:definition "The general category of observation described" ;
    skos:editorialNote "Cardinality: 0..0" ;
    skos:note "Use only if we don't define named subtypes of Observation for specific categories." ;
    linkml:examples "Example(value='', description=None)" .

linkml:specimenQuantityObservation__focus a owl:ObjectProperty,
        linkml:SlotDefinition ;
    rdfs:label "specimenQuantityObservation__focus" ;
    rdfs:domain <https://example.org/crdch_model/SpecimenQuantityObservation> ;
    rdfs:range <https://example.org/crdch_model/Entity> ;
    skos:definition "The entity or entities directly observed/measured in generating an observation result." ;
    skos:editorialNote "Cardinality: 0..m" ;
    skos:note "The 'focus', 'subject', and 'specimen' fields are useful when data creators want an Observation object to stand on its own, so it can point back to the entities it is about.  These fields are not needed when an Observation is embedded in a Specimen or other entity, where focus, subject, and specimen can be determined from context. " ;
    linkml:examples "Example(value='', description=None)" .

linkml:specimenQuantityObservation__id a owl:ObjectProperty,
        linkml:SlotDefinition ;
    rdfs:label "specimenQuantityObservation__id" ;
    rdfs:domain <https://example.org/crdch_model/SpecimenQuantityObservation> ;
    rdfs:range <https://example.org/crdch_model/Entity> ;
    skos:definition "The 'logical' identifier of the entity within the system of record.  The simple value of this attribute stands for an identifier of this data object within the system, it can be used as a reference from other objects within the same system (i.e. primary and foreign keys), and it should be unique per type of object. The same data object copied to a different system will likely have a different \"id\" in the new system since \"id\" values are system specific and do not represent persistent business identifiers. Business identifiers are assigned outside the information system and are captured in the \"identifier\" field. The \"id\" field is more likely to be a serially or randomly generated value that is assigned to the data object as it is created in a system." ;
    skos:editorialNote "Cardinality: 0..0" ;
    skos:note "FHIR naming conventions are followed here, where 'id' is used for logical identifiers, and 'identifier' for business identifiers.   The identified entity may have a different 'id' in a different system, and have many external business 'identifiers' associated with it. If an \"id\" value can also be considered to be a business identifier, and should be transmissible to other systems, it should be duplicated in the \"identifier\" attribute along with the additional metadata needed to give context to the value of \"id\". An entity in this model that does not have an \"id\" field is considered to be an embeddable entity that can not stand on its own. " ;
    linkml:examples "Example(value='', description=None)" .

linkml:specimenQuantityObservation__method_type a owl:ObjectProperty,
        linkml:SlotDefinition ;
    rdfs:label "specimenQuantityObservation__method_type" ;
    rdfs:domain <https://example.org/crdch_model/SpecimenQuantityObservation> ;
    rdfs:range <http://UNKNOWN.org/enum_CRDCH_SpecimenQuantityObservation_method_type> ;
    skos:definition "A type of method used in generating the Observation result." ;
    skos:editorialNote "Cardinality: 0..m" ;
    skos:note "This may be a type of observational, measurement, experimental, or computational method specifying how to generate data (e.g. 'manual counting', 'bright field microscopy',). Or a Guideline or SOP specifying how to interpret data and/or encode the result of an  Observation (e.g. a Cancer Staging system such as that defined by the AJCC, or variant interpretation guideline such as that provided by the ACMG)." ;
    linkml:examples "Example(value='', description=None)" .

linkml:specimenQuantityObservation__observation_type a owl:ObjectProperty,
        linkml:SlotDefinition ;
    rdfs:label "specimenQuantityObservation__observation_type" ;
    rdfs:domain <https://example.org/crdch_model/SpecimenQuantityObservation> ;
    rdfs:range <http://UNKNOWN.org/enum_CRDCH_SpecimenQuantityObservation_observation_type> ;
    skos:definition "The specific type of observation made - i.e. the feature or characteristic that was observed, measured, estimated, etc.." ;
    skos:editorialNote "Cardinality: 1..1" ;
    skos:note "This field holds the 'key' in the core key-value pair comprised of the observation_type field and the relevant value(s) field." ;
    linkml:examples "Example(value='', description=None)" .

linkml:specimenQuantityObservation__performed_by a owl:ObjectProperty,
        linkml:SlotDefinition ;
    rdfs:label "specimenQuantityObservation__performed_by" ;
    rdfs:domain <https://example.org/crdch_model/SpecimenQuantityObservation> ;
    rdfs:range <https://example.org/crdch_model/Organization> ;
    skos:definition "The organization or group that performed the observation activity." ;
    skos:editorialNote "Cardinality: 0..1" ;
    linkml:examples "Example(value='', description=None)" .

linkml:specimenQuantityObservation__subject a owl:ObjectProperty,
        linkml:SlotDefinition ;
    rdfs:label "specimenQuantityObservation__subject" ;
    rdfs:domain <https://example.org/crdch_model/SpecimenQuantityObservation> ;
    rdfs:range <https://example.org/crdch_model/Subject> ;
    skos:definition "The patient that the observation is about (if not the direct focus).  e.g. observations are often made on specimens derived from a patient, or other entities related to a patient, that ultimately tell us something about the patient of interest." ;
    skos:editorialNote "Cardinality: 0..1" ;
    linkml:examples "Example(value='', description=None)" .

linkml:specimenQuantityObservation__valueQuantity a owl:ObjectProperty,
        linkml:SlotDefinition ;
    rdfs:label "specimenQuantityObservation__valueQuantity" ;
    rdfs:domain <https://example.org/crdch_model/SpecimenQuantityObservation> ;
    rdfs:range <https://example.org/crdch_model/Quantity> ;
    skos:definition "The result of the observation, encoded as a free-text Quantity." ;
    skos:editorialNote "Cardinality: 1..1" ;
    skos:note "One and only one of the value(x) fields must be populated." ;
    linkml:examples "Example(value='', description=None)" .

linkml:specimenStorageActivity__container a owl:ObjectProperty,
        linkml:SlotDefinition ;
    rdfs:label "specimenStorageActivity__container" ;
    rdfs:domain <https://example.org/crdch_model/SpecimenStorageActivity> ;
    rdfs:range <https://example.org/crdch_model/SpecimenContainer> ;
    skos:definition "A container in which the specimen is held or affixed during its storage." ;
    skos:editorialNote "Cardinality: 0..m" ;
    linkml:examples "Example(value='', description=None)" .

linkml:specimenStorageActivity__date_ended a owl:ObjectProperty,
        linkml:SlotDefinition ;
    rdfs:label "specimenStorageActivity__date_ended" ;
    rdfs:domain <https://example.org/crdch_model/SpecimenStorageActivity> ;
    rdfs:range <https://example.org/crdch_model/TimePoint> ;
    skos:definition "The date when the activity ended (in this case, a storage event)." ;
    skos:editorialNote "Cardinality: 0..1" ;
    skos:note "To allow for more precise specification of dates when an activity was performed, we provide date_started and date_ended attributes.  If source data only provides a single date, it SHOULD be entered as both the date_started and date_ended." ;
    linkml:examples "Example(value='', description=None)" .

linkml:specimenStorageActivity__date_started a owl:ObjectProperty,
        linkml:SlotDefinition ;
    rdfs:label "specimenStorageActivity__date_started" ;
    rdfs:domain <https://example.org/crdch_model/SpecimenStorageActivity> ;
    rdfs:range <https://example.org/crdch_model/TimePoint> ;
    skos:definition "The date when the activity began (in this case, a storage event)." ;
    skos:editorialNote "Cardinality: 0..1" ;
    skos:note "To allow for more precise specification of dates when an activity was performed, we provide date_started and date_ended attributes.  If source data only provides a single date, it SHOULD be entered as both the date_started and date_ended." ;
    linkml:examples "Example(value='', description=None)" .

linkml:specimenStorageActivity__duration a owl:ObjectProperty,
        linkml:SlotDefinition ;
    rdfs:label "specimenStorageActivity__duration" ;
    rdfs:domain <https://example.org/crdch_model/SpecimenStorageActivity> ;
    rdfs:range <https://example.org/crdch_model/Quantity> ;
    skos:definition "The length of time over which the activity was performed." ;
    skos:editorialNote "Cardinality: 0..1" ;
    skos:note "Quantity.unit MUST be a unit of time. " ;
    linkml:examples "Example(value='', description=None)" .

linkml:specimenStorageActivity__method_type a owl:ObjectProperty,
        linkml:SlotDefinition ;
    rdfs:label "specimenStorageActivity__method_type" ;
    rdfs:domain <https://example.org/crdch_model/SpecimenStorageActivity> ;
    rdfs:range <http://UNKNOWN.org/enum_CRDCH_SpecimenStorageActivity_method_type> ;
    skos:definition "A specific type of method or procedure performed to store the specimen" ;
    skos:editorialNote "Cardinality: 0..1" ;
    linkml:examples "Example(value='RNAlater at 4C', description=None)",
        "Example(value='ambient temperature', description=None)",
        "Example(value='cut slide', description=None)",
        "Example(value='fresh', description=None)",
        "Example(value='frozen at -150C', description=None)",
        "Example(value='frozen at -70C', description=None)",
        "Example(value='frozen in liquid nitrogen', description=None)",
        "Example(value='frozen in vapor phase', description=None)",
        "Example(value='paraffin block', description=None)" .

linkml:specimenStorageActivity__performed_by a owl:ObjectProperty,
        linkml:SlotDefinition ;
    rdfs:label "specimenStorageActivity__performed_by" ;
    rdfs:domain <https://example.org/crdch_model/SpecimenStorageActivity> ;
    rdfs:range <https://example.org/crdch_model/Organization> ;
    skos:definition "The organization or group that performed the activity." ;
    skos:editorialNote "Cardinality: 0..1" ;
    linkml:examples "Example(value='', description=None)" .

linkml:specimenTransportActivity__date_ended a owl:ObjectProperty,
        linkml:SlotDefinition ;
    rdfs:label "specimenTransportActivity__date_ended" ;
    rdfs:domain <https://example.org/crdch_model/SpecimenTransportActivity> ;
    rdfs:range <https://example.org/crdch_model/TimePoint> ;
    skos:definition "The date when the activity ended (in this case, a transport event)." ;
    skos:editorialNote "Cardinality: 0..1" ;
    skos:note "To allow for more precise specification of dates when an activity was performed, we provide date_started and date_ended attributes.  If source data only provides a single date, it SHOULD be entered as both the date_started and date_ended." ;
    linkml:examples "Example(value='', description=None)" .

linkml:specimenTransportActivity__date_started a owl:ObjectProperty,
        linkml:SlotDefinition ;
    rdfs:label "specimenTransportActivity__date_started" ;
    rdfs:domain <https://example.org/crdch_model/SpecimenTransportActivity> ;
    rdfs:range <https://example.org/crdch_model/TimePoint> ;
    skos:definition "The date when the activity began (in this case, a transport event)." ;
    skos:editorialNote "Cardinality: 0..1" ;
    skos:note "To allow for more precise specification of dates when an activity was performed, we provide date_started and date_ended attributes.  If source data only provides a single date, it SHOULD be entered as both the date_started and date_ended." ;
    linkml:examples "Example(value='', description=None)" .

linkml:specimenTransportActivity__duration a owl:ObjectProperty,
        linkml:SlotDefinition ;
    rdfs:label "specimenTransportActivity__duration" ;
    rdfs:domain <https://example.org/crdch_model/SpecimenTransportActivity> ;
    rdfs:range <https://example.org/crdch_model/Entity> ;
    skos:definition "The length of time over which the activity was performed." ;
    linkml:examples "Example(value='', description=None)" .

linkml:specimenTransportActivity__execution_condition_observation a owl:ObjectProperty,
        linkml:SlotDefinition ;
    rdfs:label "specimenTransportActivity__execution_condition_observation" ;
    rdfs:domain <https://example.org/crdch_model/SpecimenTransportActivity> ;
    rdfs:range <https://example.org/crdch_model/ExecutionConditionObservation> ;
    skos:definition "Information describing the environmental conditions in which an activity, or a specific part of an activity, was performed." ;
    skos:editorialNote "Cardinality: 0..m" ;
    skos:note "e.g. that a specimen was shipped with an ice pack, or at a specific temperature. " ;
    linkml:examples "Example(value='', description=None)" .

linkml:specimenTransportActivity__performed_by a owl:ObjectProperty,
        linkml:SlotDefinition ;
    rdfs:label "specimenTransportActivity__performed_by" ;
    rdfs:domain <https://example.org/crdch_model/SpecimenTransportActivity> ;
    rdfs:range <https://example.org/crdch_model/Organization> ;
    skos:definition "The organization or group that performed the activity." ;
    skos:editorialNote "Cardinality: 0..1" ;
    linkml:examples "Example(value='', description=None)" .

linkml:specimenTransportActivity__transport_destination a owl:ObjectProperty,
        linkml:SlotDefinition ;
    rdfs:label "specimenTransportActivity__transport_destination" ;
    rdfs:domain <https://example.org/crdch_model/SpecimenTransportActivity> ;
    rdfs:range <https://example.org/crdch_model/Organization> ;
    skos:definition "An organization (facility, site, lab, etc) to which the specimen is delivered as a result of the activity." ;
    skos:editorialNote "Cardinality: 0..1" ;
    linkml:examples "Example(value='', description=None)" .

linkml:specimenTransportActivity__transport_origin a owl:ObjectProperty,
        linkml:SlotDefinition ;
    rdfs:label "specimenTransportActivity__transport_origin" ;
    rdfs:domain <https://example.org/crdch_model/SpecimenTransportActivity> ;
    rdfs:range <https://example.org/crdch_model/Organization> ;
    skos:definition "An organization (facility, site, lab, etc) from which the specimen was transported as a result of the activity." ;
    skos:editorialNote "Cardinality: 0..1" ;
    linkml:examples "Example(value='', description=None)" .

linkml:specimen__analyte_type a owl:ObjectProperty,
        linkml:SlotDefinition ;
    rdfs:label "specimen__analyte_type" ;
    rdfs:domain <https://example.org/crdch_model/Specimen> ;
    rdfs:range <http://UNKNOWN.org/enum_CRDCH_Specimen_analyte_type> ;
    skos:definition "For specimens of type 'analyte' (or an 'aliquot' derived from an analyte), this is the category of chemcial the analyte of interest represents (e.g. DNA, RNA)" ;
    skos:editorialNote "Cardinality: 0..1" ;
    linkml:examples "Example(value='DNA', description=None)",
        "Example(value='FFPE DNA', description=None)",
        "Example(value='FFPE RNA', description=None)",
        "Example(value='GenomePlex (Rubicon) Amplified DNA', description=None)",
        "Example(value='RNA', description=None)",
        "Example(value='Repli-G (Qiagen) DNA', description=None)" .

linkml:specimen__associated_project a owl:ObjectProperty,
        linkml:SlotDefinition ;
    rdfs:label "specimen__associated_project" ;
    rdfs:domain <https://example.org/crdch_model/Specimen> ;
    rdfs:range <https://example.org/crdch_model/ResearchProject> ;
    skos:definition "The Project associated with the specimen." ;
    skos:editorialNote "Cardinality: 0..1" ;
    linkml:examples "Example(value='', description=None)" .

linkml:specimen__cellular_composition_type a owl:ObjectProperty,
        linkml:SlotDefinition ;
    rdfs:label "specimen__cellular_composition_type" ;
    rdfs:domain <https://example.org/crdch_model/Specimen> ;
    rdfs:range <http://UNKNOWN.org/enum_CRDCH_Specimen_cellular_composition_type> ;
    skos:definition "A term describing the type of cell or cellular material comprising a specimen." ;
    skos:editorialNote "Cardinality: 0..1" ;
    linkml:examples "Example(value='2D Classical Conditionally Reprogrammed Cells', description=None)",
        "Example(value='Adherent Cell Line', description=None)",
        "Example(value='Bone Marrow Components', description=None)",
        "Example(value='Buccal Cells', description=None)",
        "Example(value='Buffy Coat', description=None)",
        "Example(value='Derived Cell Line', description=None)",
        "Example(value='Granulocytes', description=None)",
        "Example(value='Human Original Cells', description=None)",
        "Example(value='Liquid Suspension Cell Line', description=None)",
        "Example(value='Pleural Effusion', description=None)" .

linkml:specimen__contained_in a owl:ObjectProperty,
        linkml:SlotDefinition ;
    rdfs:label "specimen__contained_in" ;
    rdfs:domain <https://example.org/crdch_model/Specimen> ;
    rdfs:range <https://example.org/crdch_model/SpecimenContainer> ;
    skos:definition "A physical container in which a specimen is presently held or attached -  as storage for future use,  a substrate for growth (e.g. a cell culture dish), or a vessel to enable analysis (e.g. a microscope slide or 96-well plate)" ;
    skos:editorialNote "Cardinality: 0..1" ;
    skos:note "The 0..1 cardinality on this attribute means that you cannot directly references multiple nested containers holding a sample. To capture this scenario, use the 'parent_container' attribute of the Container entity.  " ;
    linkml:examples "Example(value='', description=None)" .

linkml:specimen__creation_activity a owl:ObjectProperty,
        linkml:SlotDefinition ;
    rdfs:label "specimen__creation_activity" ;
    rdfs:domain <https://example.org/crdch_model/Specimen> ;
    rdfs:range <https://example.org/crdch_model/SpecimenCreationActivity> ;
    skos:definition "The activity through which a specimen was created, by removing material from an biological subject, or deriving material from an existing specimen." ;
    skos:editorialNote "Cardinality: 0..1" ;
    skos:note "Note that a given specimen is the result of only one and only one SpecimenCreationActivity, but may be subject to many processing events that subsequently modify or derive new specimens from it." ;
    linkml:examples "Example(value='', description=None)" .

linkml:specimen__data_provider a owl:ObjectProperty,
        linkml:SlotDefinition ;
    rdfs:label "specimen__data_provider" ;
    rdfs:domain <https://example.org/crdch_model/Specimen> ;
    rdfs:range <https://example.org/crdch_model/Organization> ;
    skos:definition "The organization (e.g.a laboratory, processing center, or research site) that provided data associated with a specimen." ;
    skos:editorialNote "Cardinality: 0..1" ;
    linkml:examples "Example(value='', description=None)" .

linkml:specimen__degree_of_dysplasia a owl:ObjectProperty,
        linkml:SlotDefinition ;
    rdfs:label "specimen__degree_of_dysplasia" ;
    rdfs:domain <https://example.org/crdch_model/Specimen> ;
    rdfs:range <http://UNKNOWN.org/enum_CRDCH_Specimen_degree_of_dysplasia> ;
    skos:definition "A term describing the nature/extent of abnormal cells  that are not cancer, as observed upon microscopic assessment of a specimen. Records the degree of dysplasia for the cyst or lesion under consideration." ;
    skos:editorialNote "Cardinality: 0..1" ;
    linkml:examples "Example(value='Carcinoma in Situ', description=None)",
        "Example(value='Mild dysplasia', description=None)",
        "Example(value='Moderate dysplasia', description=None)",
        "Example(value='Normal or basal cell hyperplasia or metaplasia', description=None)",
        "Example(value='Severe dysplasia', description=None)",
        "Example(value='Unknown', description=None)" .

linkml:specimen__derived_product a owl:ObjectProperty,
        linkml:SlotDefinition ;
    rdfs:label "specimen__derived_product" ;
    rdfs:domain <https://example.org/crdch_model/Specimen> ;
    rdfs:range <https://example.org/crdch_model/BiologicProduct> ;
    skos:definition "A 'living' biologically active product that was derived from the specimen (e.g. a cell culture, tissue culture, or organoid)" ;
    skos:editorialNote "Cardinality: 0..m" ;
    linkml:examples "Example(value='', description=None)" .

linkml:specimen__description a owl:ObjectProperty,
        linkml:SlotDefinition ;
    rdfs:label "specimen__description" ;
    rdfs:domain <https://example.org/crdch_model/Specimen> ;
    rdfs:range <https://example.org/crdch_model/Entity> ;
    skos:definition "A free text field to capture additional information or explanation about the specimen." ;
    skos:editorialNote "Cardinality: 0..1" ;
    linkml:examples "Example(value='', description=None)" .

linkml:specimen__dimensional_measures a owl:ObjectProperty,
        linkml:SlotDefinition ;
    rdfs:label "specimen__dimensional_measures" ;
    rdfs:domain <https://example.org/crdch_model/Specimen> ;
    rdfs:range <https://example.org/crdch_model/DimensionalObservationSet> ;
    skos:definition "Observations about the current physical dimensions of an object (e.g. length, width, area)." ;
    skos:editorialNote "Cardinality: 0..1" ;
    skos:note "Observations are flexible containers for capturing a specific type of observation/measurement data about an object, along with metadata about how it was generated. The specific type of observation made is captured as data in the Observation object." ;
    linkml:examples "Example(value='', description=None)" .

linkml:specimen__distance_from_paired_specimen a owl:ObjectProperty,
        linkml:SlotDefinition ;
    rdfs:label "specimen__distance_from_paired_specimen" ;
    rdfs:domain <https://example.org/crdch_model/Specimen> ;
    rdfs:range <https://example.org/crdch_model/Quantity> ;
    skos:definition "The observed distance in the body of the specimen from a 'paired specimen' at the time of collection. (e.g. the distance between the in vivo location of a tumor tissue specimen and its paired normal specimen)" ;
    skos:editorialNote "Cardinality: 0..1" ;
    linkml:examples "Example(value='', description=None)" .

linkml:specimen__dysplasia_fraction a owl:ObjectProperty,
        linkml:SlotDefinition ;
    rdfs:label "specimen__dysplasia_fraction" ;
    rdfs:domain <https://example.org/crdch_model/Specimen> ;
    rdfs:range <https://example.org/crdch_model/Entity> ;
    skos:definition "Resulting value to represent the number of pieces of dysplasia divided by the total number of pieces." ;
    skos:editorialNote "Cardinality: 0..1" ;
    linkml:examples "Example(value='', description=None)" .

linkml:specimen__general_tissue_morphology a owl:ObjectProperty,
        linkml:SlotDefinition ;
    rdfs:label "specimen__general_tissue_morphology" ;
    rdfs:domain <https://example.org/crdch_model/Specimen> ;
    rdfs:range <http://UNKNOWN.org/enum_CRDCH_Specimen_general_tissue_morphology> ;
    skos:definition "The high-level kind of tissue collected when generating a specimen, based on its disease status or proximity to tumor tissue (e.g. is it normal, abnormal, tumor, tumor-adjacent)." ;
    skos:editorialNote "Cardinality: 0..1" ;
    linkml:examples "Example(value='Abnormal', description=None)",
        "Example(value='Normal', description=None)",
        "Example(value='Peritumoral', description=None)",
        "Example(value='Tumor', description=None)",
        "Example(value='not applicable', description=None)" .

linkml:specimen__histological_composition_measures a owl:ObjectProperty,
        linkml:SlotDefinition ;
    rdfs:label "specimen__histological_composition_measures" ;
    rdfs:domain <https://example.org/crdch_model/Specimen> ;
    rdfs:range <https://example.org/crdch_model/HistologicalCompositionObservationSet> ;
    skos:definition "A set of one or more observations that quantify the relative or absolute composition of a specimen at cellular level - e.g. how many cells in the specimen are of a given type, or exhibit a particular cellular phenotype." ;
    skos:editorialNote "Cardinality: 0..m" ;
    skos:note "Observations are flexible containers for capturing a specific type of observation/measurement data about an object, along with metadata about how it was generated. The specific type of observation made is captured as data in the Observation object." ;
    linkml:examples "Example(value='', description=None)" .

linkml:specimen__id a owl:ObjectProperty,
        linkml:SlotDefinition ;
    rdfs:label "specimen__id" ;
    rdfs:domain <https://example.org/crdch_model/Specimen> ;
    rdfs:range <https://example.org/crdch_model/Entity> ;
    skos:definition "The 'logical' identifier of the entity within the system of record.  The simple value of this attribute stands for an identifier of this data object within the system, it can be used as a reference from other objects within the same system (i.e. primary and foreign keys), and it should be unique per type of object. The same data object copied to a different system will likely have a different \"id\" in the new system since \"id\" values are system specific and do not represent persistent business identifiers. Business identifiers are assigned outside the information system and are captured in the \"identifier\" field. The \"id\" field is more likely to be a serially or randomly generated value that is assigned to the data object as it is created in a system." ;
    skos:editorialNote "Cardinality: 0..1" ;
    skos:note "FHIR naming conventions are followed here, where 'id' is used for logical identifiers, and 'identifier' for business identifiers.   The identified entity may have a different 'id' in a different system, and have many external business 'identifiers' associated with it. If an \"id\" value can also be considered to be a business identifier, and should be transmissible to other systems, it should be duplicated in the \"identifier\" attribute along with the additional metadata needed to give context to the value of \"id\". An entity in this model that does not have an \"id\" field is considered to be an embeddable entity that can not stand on its own. " ;
    linkml:examples "Example(value='', description=None)" .

linkml:specimen__identifier a owl:ObjectProperty,
        linkml:SlotDefinition ;
    rdfs:label "specimen__identifier" ;
    rdfs:domain <https://example.org/crdch_model/Specimen> ;
    rdfs:range <https://example.org/crdch_model/Identifier> ;
    skos:definition "A 'business' identifier or accession number for the entity, typically as provided by an external system or authority, that are globally unique and persist across implementing systems. Also, since these identifiers are created outside the information system through a specific business process, the Identifier type has additional attributes to capture this additional metadata so the actual identifier values are qualified by the context that created those values. This additional context allows \"identifier\" instances to be transmitted as business data across systems while still being able to trace them back to the system of origin." ;
    skos:editorialNote "Cardinality: 0..m" ;
    skos:note "FHIR naming conventions are followed here, where 'id' is used for logical identifiers which are unique only within a given system, and 'identifier' for business identifiers, which are used to connect entities or share content across systems.  The complex 'Identifier' data type is used  to capture the identifier itself, along with metadata about its source." ;
    linkml:examples "Example(value='', description=None)" .

linkml:specimen__morphology_assessment_method a owl:ObjectProperty,
        linkml:SlotDefinition ;
    rdfs:label "specimen__morphology_assessment_method" ;
    rdfs:domain <https://example.org/crdch_model/Specimen> ;
    rdfs:range <http://UNKNOWN.org/enum_CRDCH_Specimen_morphology_assessment_method> ;
    skos:definition "The general method used to assess a specimens specific tissue morphology" ;
    skos:editorialNote "Cardinality: 0..1" ;
    linkml:examples "Example(value='Digital', description=None)",
        "Example(value='Microscopy', description=None)",
        "Example(value='Other', description=None)",
        "Example(value='Unknown', description=None)" .

linkml:specimen__morphology_assessor_role a owl:ObjectProperty,
        linkml:SlotDefinition ;
    rdfs:label "specimen__morphology_assessor_role" ;
    rdfs:domain <https://example.org/crdch_model/Specimen> ;
    rdfs:range <http://UNKNOWN.org/enum_CRDCH_Specimen_morphology_assessor_role> ;
    skos:definition "A term describing the role of the person who histologically assessed the specific tissue morphology of a specimen" ;
    skos:editorialNote "Cardinality: 0..1" ;
    linkml:examples "Example(value='Other', description=None)",
        "Example(value='Pathologist', description=None)",
        "Example(value='Research Scientist', description=None)",
        "Example(value='Unknown', description=None)" .

linkml:specimen__morphology_pathologically_confirmed a owl:ObjectProperty,
        linkml:SlotDefinition ;
    rdfs:label "specimen__morphology_pathologically_confirmed" ;
    rdfs:domain <https://example.org/crdch_model/Specimen> ;
    rdfs:range <https://example.org/crdch_model/Entity> ;
    skos:definition "A flag indicating whether the histologic assessment of specific morphology was confirmed by pathologist review." ;
    skos:editorialNote "Cardinality: 0..1" ;
    linkml:examples "Example(value='', description=None)" .

linkml:specimen__parent_specimen a owl:ObjectProperty,
        linkml:SlotDefinition ;
    rdfs:label "specimen__parent_specimen" ;
    rdfs:domain <https://example.org/crdch_model/Specimen> ;
    rdfs:range <https://example.org/crdch_model/Specimen> ;
    skos:definition "An existing specimen from which the specimen of interest was directly derived (i.e its immediate parent specimen)." ;
    skos:editorialNote "Cardinality: 0..m" ;
    skos:note "This property indicates only the direct parent specimen(s).  Cardinality is 0..m to account for specimens derived from pooling of multiple specimens." ;
    linkml:examples "Example(value='', description=None)" .

linkml:specimen__preinvasive_tissue_morphology a owl:ObjectProperty,
        linkml:SlotDefinition ;
    rdfs:label "specimen__preinvasive_tissue_morphology" ;
    rdfs:domain <https://example.org/crdch_model/Specimen> ;
    rdfs:range <http://UNKNOWN.org/enum_CRDCH_Specimen_preinvasive_tissue_morphology> ;
    skos:definition "A term describing the specific pathology exhibited by pre-invasive tissue comprising a specimen." ;
    skos:editorialNote "Cardinality: 0..1" ;
    linkml:examples "Example(value='', description=None)" .

linkml:specimen__processing_activity a owl:ObjectProperty,
        linkml:SlotDefinition ;
    rdfs:label "specimen__processing_activity" ;
    rdfs:domain <https://example.org/crdch_model/Specimen> ;
    rdfs:range <https://example.org/crdch_model/SpecimenProcessingActivity> ;
    skos:definition "An activity that modifies the physical structure, composition, or state of a specimen." ;
    skos:editorialNote "Cardinality: 0..m" ;
    skos:note "Note that a given specimen may undergo more than one distinct processing activity, through application of different methodologies that modify its physical state. However, if an activity generates a new specimen (e.g. via portioning, slicing) it is considered a SpeciemnCreationActivity." ;
    linkml:examples "Example(value='', description=None)" .

linkml:specimen__quality_measure a owl:ObjectProperty,
        linkml:SlotDefinition ;
    rdfs:label "specimen__quality_measure" ;
    rdfs:domain <https://example.org/crdch_model/Specimen> ;
    rdfs:range <https://example.org/crdch_model/SpecimenQualityObservation> ;
    skos:definition "An observation about characteristics of a specimen that are indicative of its quality or suitability for use." ;
    skos:editorialNote "Cardinality: 0..m" ;
    skos:note "Observations are flexible containers for capturing a specific type of observation/measurement data about an object, along with metadata about how it was generated. The specific type of observation made is captured as data in the Observation object." ;
    linkml:examples "Example(value='', description=None)" .

linkml:specimen__quantity_measure a owl:ObjectProperty,
        linkml:SlotDefinition ;
    rdfs:label "specimen__quantity_measure" ;
    rdfs:domain <https://example.org/crdch_model/Specimen> ;
    rdfs:range <https://example.org/crdch_model/SpecimenQuantityObservation> ;
    skos:definition "An observation related to the present quantity of a specimen - e.g. its weight, volume, or analyte concentration." ;
    skos:editorialNote "Cardinality: 0..m" ;
    skos:note "Observations are flexible containers for capturing a specific type of observation/measurement data about an object, along with metadata about how it was generated. The specific type of observation made is captured as data in the Observation object." ;
    linkml:examples "Example(value='', description=None)" .

linkml:specimen__related_document a owl:ObjectProperty,
        linkml:SlotDefinition ;
    rdfs:label "specimen__related_document" ;
    rdfs:domain <https://example.org/crdch_model/Specimen> ;
    rdfs:range <https://example.org/crdch_model/Document> ;
    skos:definition "A reference to an external document that is about or related to the specimen (e.g. a publication related to the study it is a part of, pathology report containing additional details about it, protocol describing how it was collected)" ;
    skos:editorialNote "Cardinality: 0..m" ;
    linkml:examples "Example(value='', description=None)" .

linkml:specimen__section_location a owl:ObjectProperty,
        linkml:SlotDefinition ;
    rdfs:label "specimen__section_location" ;
    rdfs:domain <https://example.org/crdch_model/Specimen> ;
    rdfs:range <http://UNKNOWN.org/enum_CRDCH_Specimen_section_location> ;
    skos:definition "The location in a parent specimen from which a section/portion was excised (e.g. top, middle, bottom)" ;
    skos:editorialNote "Cardinality: 0..1" ;
    skos:note "This attribute applies only to Specimens that are of type 'portion' or 'slide'." ;
    linkml:examples "Example(value='Bottom', description=None)",
        "Example(value='Top', description=None)",
        "Example(value='Unknown', description=None)" .

linkml:specimen__source_material_type a owl:ObjectProperty,
        linkml:SlotDefinition ;
    rdfs:label "specimen__source_material_type" ;
    rdfs:domain <https://example.org/crdch_model/Specimen> ;
    rdfs:range <http://UNKNOWN.org/enum_CRDCH_Specimen_source_material_type> ;
    skos:definition "The general kind of material from which the specimen was derived." ;
    skos:editorialNote "Cardinality: 0..1" ;
    skos:note "Values captured here may describe the type of molecular mixture, cell, tissue, organ, body fluid, embryo, excretory substance, or experimental system from which a specimen was derived." ;
    linkml:examples "Example(value='Cell Line', description=None)",
        "Example(value='Expanded Next Generation Cancer Model', description=None)",
        "Example(value='Pleural Effusion', description=None)",
        "Example(value='Tissue, Blood, Tumor Aspirate', description=None)",
        "Example(value='Xenograft Tissue', description=None)" .

linkml:specimen__source_subject a owl:ObjectProperty,
        linkml:SlotDefinition ;
    rdfs:label "specimen__source_subject" ;
    rdfs:domain <https://example.org/crdch_model/Specimen> ;
    rdfs:range <https://example.org/crdch_model/Subject> ;
    skos:definition "A specific Subject from which the specimen was directly or indirectly derived." ;
    skos:editorialNote "Cardinality: 0..1" ;
    linkml:examples "Example(value='', description=None)" .

linkml:specimen__specific_tissue_morphology a owl:ObjectProperty,
        linkml:SlotDefinition ;
    rdfs:label "specimen__specific_tissue_morphology" ;
    rdfs:domain <https://example.org/crdch_model/Specimen> ;
    rdfs:range <http://UNKNOWN.org/enum_CRDCH_Specimen_specific_tissue_morphology> ;
    skos:definition "A term describing the specific pathology exhibited by the tissue comprising a specimen." ;
    skos:editorialNote "Cardinality: 0..1" ;
    linkml:examples "Example(value='00', description=None)",
        "Example(value='01', description=None)",
        "Example(value='02', description=None)",
        "Example(value='Atypical melanocytic proliferation', description=None)",
        "Example(value='CNS, medulloblastoma', description=None)",
        "Example(value='Lung Cancer (all types)', description=None)",
        "Example(value='Melanocytic hyperplasia', description=None)",
        "Example(value='Melanoma in situ, superficial spreading', description=None)",
        "Example(value='Non cancerous tissue', description=None)" .

linkml:specimen__specimen_type a owl:ObjectProperty,
        linkml:SlotDefinition ;
    rdfs:label "specimen__specimen_type" ;
    rdfs:domain <https://example.org/crdch_model/Specimen> ;
    rdfs:range <http://UNKNOWN.org/enum_CRDCH_Specimen_specimen_type> ;
    skos:definition "The high-level type of the specimen, based on its derivation provenance (i.e. how far removed it is from the original sample extracted from a source)." ;
    skos:editorialNote "Cardinality: 0..1" ;
    skos:note "Our model defines a single 'Specimen' type to cover speific subtypes of specimens delineated in some CRDC node models (e.g. GDC 'Sample', 'Portion', 'Aliquot', 'Analyte', and 'Slide'). The 'specimen_type' field is used to indicate which subtype a given Specimen instance represents.  The enumerated values are meant to be mutually exclusive, such that only one can be applied to a given specimen." ;
    linkml:examples "Example(value='Aliquot', description=None)",
        "Example(value='Analyte', description=None)",
        "Example(value='Initial Sample', description=None)",
        "Example(value='Portion', description=None)",
        "Example(value='Slide', description=None)" .

linkml:specimen__storage_activity a owl:ObjectProperty,
        linkml:SlotDefinition ;
    rdfs:label "specimen__storage_activity" ;
    rdfs:domain <https://example.org/crdch_model/Specimen> ;
    rdfs:range <https://example.org/crdch_model/SpecimenStorageActivity> ;
    skos:definition "An activity that results in the storage or maintenance of a specimen in a particular location, container, or state." ;
    skos:editorialNote "Cardinality: 0..m" ;
    skos:note "The 0..m cardinality of this attribute reflects the fact that a given specimen may undergo many separate periods of storage, in different locations and/or under different conditions " ;
    linkml:examples "Example(value='', description=None)" .

linkml:specimen__transport_activity a owl:ObjectProperty,
        linkml:SlotDefinition ;
    rdfs:label "specimen__transport_activity" ;
    rdfs:domain <https://example.org/crdch_model/Specimen> ;
    rdfs:range <https://example.org/crdch_model/SpecimenTransportActivity> ;
    skos:definition "An activity through which the specimen is transported between locations." ;
    skos:editorialNote "Cardinality: 0..m" ;
    skos:note "The 0..m cardinality of this attribute reflects the fact that a given specimen may undergo many separate transport processes at different periods of time." ;
    linkml:examples "Example(value='', description=None)" .

linkml:specimen__tumor_status_at_collection a owl:ObjectProperty,
        linkml:SlotDefinition ;
    rdfs:label "specimen__tumor_status_at_collection" ;
    rdfs:domain <https://example.org/crdch_model/Specimen> ;
    rdfs:range <http://UNKNOWN.org/enum_CRDCH_Specimen_tumor_status_at_collection> ;
    skos:definition "The status of the tumor at the time the specimen was collected (e.g. if it was primary, recurrent, metastatic, etc)." ;
    skos:editorialNote "Cardinality: 0..1" ;
    linkml:examples "Example(value='Additional Primary', description=None)",
        "Example(value='Local recurrence', description=None)",
        "Example(value='Metastatic', description=None)",
        "Example(value='NOS', description=None)",
        "Example(value='Premalignant', description=None)",
        "Example(value='Primary', description=None)",
        "Example(value='Recurrent', description=None)",
        "Example(value='Xenograft', description=None)" .

linkml:subject__age_at_death a owl:ObjectProperty,
        linkml:SlotDefinition ;
    rdfs:label "subject__age_at_death" ;
    rdfs:domain <https://example.org/crdch_model/Subject> ;
    rdfs:range <https://example.org/crdch_model/Quantity> ;
    skos:definition "The age of an individual at the time of death, expressed in days since birth" ;
    skos:editorialNote "Cardinality: 0..1" ;
    linkml:examples "Example(value='', description=None)" .

linkml:subject__breed a owl:ObjectProperty,
        linkml:SlotDefinition ;
    rdfs:label "subject__breed" ;
    rdfs:domain <https://example.org/crdch_model/Subject> ;
    rdfs:range <http://UNKNOWN.org/enum_CRDCH_Subject_breed> ;
    skos:definition "A label given to a group of animals homogeneous in appearance and other characteristics that distinguish it from other animals of the same species." ;
    skos:editorialNote "Cardinality: 0..1" ;
    linkml:examples "Example(value='Affenpinscher', description=None)",
        "Example(value='Afghan Hound', description=None)",
        "Example(value='Airedale Terrier', description=None)",
        "Example(value='Akita', description=None)" .

linkml:subject__cause_of_death a owl:ObjectProperty,
        linkml:SlotDefinition ;
    rdfs:label "subject__cause_of_death" ;
    rdfs:domain <https://example.org/crdch_model/Subject> ;
    rdfs:range <http://UNKNOWN.org/enum_CRDCH_Subject_cause_of_death> ;
    skos:definition "Coded value indicating the circumstance or condition that results in the death of the subject." ;
    skos:editorialNote "Cardinality: 0..1" ;
    linkml:examples "Example(value='', description=None)",
        "Example(value='Cancer Related', description=None)",
        "Example(value='Cardiovascular Disorder, NOS', description=None)",
        "Example(value='End-stage Renal Disease', description=None)" .

linkml:subject__ethnicity a owl:ObjectProperty,
        linkml:SlotDefinition ;
    rdfs:label "subject__ethnicity" ;
    rdfs:domain <https://example.org/crdch_model/Subject> ;
    rdfs:range <http://UNKNOWN.org/enum_CRDCH_Subject_ethnicity> ;
    skos:definition "An individual's self-described social and cultural grouping, specifically whether an individual describes themselves as Hispanic or Latino. The provided values are based on the categories defined by the U.S. Office of Management and Business and used by the U.S. Census Bureau" ;
    skos:editorialNote "Cardinality: 0..1" ;
    skos:note "Applicable only when Subject.species is Homo Sapiens" ;
    linkml:examples "Example(value='Hispanic or Latino', description=None)",
        "Example(value='Not Allowed To Collect', description=None)",
        "Example(value='Not Hispanic or Latino', description=None)",
        "Example(value='Not Reported', description=None)",
        "Example(value='Unknown', description=None)" .

linkml:subject__id a owl:ObjectProperty,
        linkml:SlotDefinition ;
    rdfs:label "subject__id" ;
    rdfs:domain <https://example.org/crdch_model/Subject> ;
    rdfs:range <https://example.org/crdch_model/Entity> ;
    skos:definition "The 'logical' identifier of the entity within the system of record.  The simple value of this attribute stands for an identifier of this data object within the system, it can be used as a reference from other objects within the same system (i.e. primary and foreign keys), and it should be unique per type of object. The same data object copied to a different system will likely have a different \"id\" in the new system since \"id\" values are system specific and do not represent persistent business identifiers. Business identifiers are assigned outside the information system and are captured in the \"identifier\" field. The \"id\" field is more likely to be a serially or randomly generated value that is assigned to the data object as it is created in a system." ;
    skos:editorialNote "Cardinality: 1..1" ;
    skos:note "FHIR naming conventions are followed here, where 'id' is used for logical identifiers, and 'identifier' for business identifiers.   The identified entity may have a different 'id' in a different system, and have many external business 'identifiers' associated with it. If an \"id\" value can also be considered to be a business identifier, and should be transmissible to other systems, it should be duplicated in the \"identifier\" attribute along with the additional metadata needed to give context to the value of \"id\". An entity in this model that does not have an \"id\" field is considered to be an embeddable entity that can not stand on its own. " ;
    linkml:examples "Example(value='', description=None)" .

linkml:subject__identifier a owl:ObjectProperty,
        linkml:SlotDefinition ;
    rdfs:label "subject__identifier" ;
    rdfs:domain <https://example.org/crdch_model/Subject> ;
    rdfs:range <https://example.org/crdch_model/Identifier> ;
    skos:definition "A 'business' identifier or accession number for the entity, typically as provided by an external system or authority, that are globally unique and persist across implementing systems. Also, since these identifiers are created outside the information system through a specific business process, the Identifier type has additional attributes to capture this additional metadata so the actual identifier values are qualified by the context that created those values. This additional context allows \"identifier\" instances to be transmitted as business data across systems while still being able to trace them back to the system of origin." ;
    skos:editorialNote "Cardinality: 0..m" ;
    skos:note "FHIR naming conventions are followed here, where 'id' is used for logical identifiers which are unique only within a given system, and 'identifier' for business identifiers, which are used to connect entities or share content across systems.  The complex 'Identifier' data type is used  to capture the identifier itself, along with metadata about its source." ;
    linkml:examples "Example(value='', description=None)" .

linkml:subject__race a owl:ObjectProperty,
        linkml:SlotDefinition ;
    rdfs:label "subject__race" ;
    rdfs:domain <https://example.org/crdch_model/Subject> ;
    rdfs:range <http://UNKNOWN.org/enum_CRDCH_Subject_race> ;
    skos:definition "An arbitrary classification of a taxonomic group that is a division of a species. It usually arises as a consequence of geographical isolation within a species and is characterized by shared heredity, physical attributes and behavior, and in the case of humans, by common history, nationality, or geographic distribution. The provided values are based on the categories defined by the U.S. Office of Management and Business and used by the U.S. Census Bureau." ;
    skos:editorialNote "Cardinality: 0..m" ;
    linkml:examples "Example(value='American Indian or Alaska Native', description=None)",
        "Example(value='Asian', description=None)",
        "Example(value='Black or African American', description=None)",
        "Example(value='Native Hawaiian or other Pacific Islander', description=None)",
        "Example(value='Not Allowed To Collect', description=None)",
        "Example(value='Not Reported', description=None)",
        "Example(value='Unknown', description=None)",
        "Example(value='White', description=None)" .

linkml:subject__sex a owl:ObjectProperty,
        linkml:SlotDefinition ;
    rdfs:label "subject__sex" ;
    rdfs:domain <https://example.org/crdch_model/Subject> ;
    rdfs:range <http://UNKNOWN.org/enum_CRDCH_Subject_sex> ;
    skos:definition "The biologic character or quality that distinguishes male and female from one another as expressed by analysis of the person's gonadal, morphologic (internal and external), chromosomal, and hormonal characteristics." ;
    skos:editorialNote "Cardinality: 0..1" ;
    linkml:examples "Example(value='Female', description=None)",
        "Example(value='Intersex', description=None)",
        "Example(value='Male', description=None)",
        "Example(value='Not Reported', description=None)",
        "Example(value='Unknown', description=None)",
        "Example(value='Unspecified', description=None)" .

linkml:subject__species a owl:ObjectProperty,
        linkml:SlotDefinition ;
    rdfs:label "subject__species" ;
    rdfs:domain <https://example.org/crdch_model/Subject> ;
    rdfs:range <http://UNKNOWN.org/enum_CRDCH_Subject_species> ;
    skos:definition "The scientific binomial name for the species of the subject (e.g. Homo sapiens, Mus musculus, etc.)" ;
    skos:editorialNote "Cardinality: 0..1" ;
    linkml:examples "Example(value='Canis familiaris', description=None)",
        "Example(value='Homo sapiens', description=None)",
        "Example(value='Mus musculus', description=None)" .

linkml:subject__vital_status a owl:ObjectProperty,
        linkml:SlotDefinition ;
    rdfs:label "subject__vital_status" ;
    rdfs:domain <https://example.org/crdch_model/Subject> ;
    rdfs:range <http://UNKNOWN.org/enum_CRDCH_Subject_vital_status> ;
    skos:definition "Coded value indicating the state or condition of being living or deceased; also includes the case where the vital status is unknown." ;
    skos:editorialNote "Cardinality: 0..1" ;
    linkml:examples "Example(value='Alive', description=None)",
        "Example(value='Dead', description=None)",
        "Example(value='Not Reported', description=None)",
        "Example(value='Unknown', description=None)" .

linkml:subject__year_of_birth a owl:ObjectProperty,
        linkml:SlotDefinition ;
    rdfs:label "subject__year_of_birth" ;
    rdfs:domain <https://example.org/crdch_model/Subject> ;
    rdfs:range <https://example.org/crdch_model/Entity> ;
    skos:definition "Numeric value to represent the calendar year in which an individual was born." ;
    skos:editorialNote "Cardinality: 0..1" ;
    skos:note "Applicable only when Subject.species is Homo Sapiens" ;
    linkml:examples "Example(value='', description=None)" .

linkml:subject__year_of_death a owl:ObjectProperty,
        linkml:SlotDefinition ;
    rdfs:label "subject__year_of_death" ;
    rdfs:domain <https://example.org/crdch_model/Subject> ;
    rdfs:range <https://example.org/crdch_model/Entity> ;
    skos:definition "Numeric value to represent the calendar year in which an individual died." ;
    skos:editorialNote "Cardinality: 0..1" ;
    linkml:examples "Example(value='', description=None)" .

linkml:substance__role a owl:ObjectProperty,
        linkml:SlotDefinition ;
    rdfs:label "substance__role" ;
    rdfs:domain <https://example.org/crdch_model/Substance> ;
    rdfs:range <http://UNKNOWN.org/enum_CRDCH_Substance_role> ;
    skos:definition "A role played by the substance in a particular application (e.g. the role of a lysis buffer when applied in a specimen creation activity, or the role of fixative when applied in specimen processing)" ;
    skos:editorialNote "Cardinality: 0..m" ;
    linkml:examples "Example(value='collection media', description=None)",
        "Example(value='fixative', description=None)",
        "Example(value='lysis buffer', description=None)",
        "Example(value='mounting medium', description=None)" .

linkml:substance__substance_quantity a owl:ObjectProperty,
        linkml:SlotDefinition ;
    rdfs:label "substance__substance_quantity" ;
    rdfs:domain <https://example.org/crdch_model/Substance> ;
    rdfs:range <https://example.org/crdch_model/Quantity> ;
    skos:definition "The quantity of substance this instance stands for." ;
    skos:editorialNote "Cardinality: 0..1" ;
    linkml:examples "Example(value='', description=None)" .

linkml:substance__substance_type a owl:ObjectProperty,
        linkml:SlotDefinition ;
    rdfs:label "substance__substance_type" ;
    rdfs:domain <https://example.org/crdch_model/Substance> ;
    rdfs:range <http://UNKNOWN.org/enum_CRDCH_Substance_substance_type> ;
    skos:definition "The specific type of the substance - at as granular a level as possible. May be a specific chemical compound, or the name of a formulation/preparation made up of many compounds." ;
    skos:editorialNote "Cardinality: 0..1" ;
    linkml:examples "Example(value='DMEM', description=None)",
        "Example(value='formalin', description=None)",
        "Example(value='toluene', description=None)" .

linkml:timePeriod__periodEnd_end a owl:ObjectProperty,
        linkml:SlotDefinition ;
    rdfs:label "timePeriod__periodEnd_end" ;
    rdfs:domain <https://example.org/crdch_model/TimePeriod> ;
    rdfs:range <https://example.org/crdch_model/TimePoint> ;
    skos:definition "When a period of time ended." ;
    skos:editorialNote "Cardinality: 0..1" ;
    linkml:examples "Example(value='', description=None)" .

linkml:timePeriod__periodStart_start a owl:ObjectProperty,
        linkml:SlotDefinition ;
    rdfs:label "timePeriod__periodStart_start" ;
    rdfs:domain <https://example.org/crdch_model/TimePeriod> ;
    rdfs:range <https://example.org/crdch_model/TimePoint> ;
    skos:definition "When a period of time started." ;
    skos:editorialNote "Cardinality: 0..1" ;
    linkml:examples "Example(value='', description=None)" .

linkml:timePoint__dateTime a owl:ObjectProperty,
        linkml:SlotDefinition ;
    rdfs:label "timePoint__dateTime" ;
    rdfs:domain <https://example.org/crdch_model/TimePoint> ;
    rdfs:range <https://example.org/crdch_model/Entity> ;
    skos:definition "An explicitly specified timepoint described in terms of a date and optionally a time on that date." ;
    skos:editorialNote "Cardinality: 0..1" ;
    skos:note "Use when the TimePeriod is just  a single instant / point in time. " ;
    linkml:examples "Example(value='', description=None)" .

linkml:timePoint__eventType a owl:ObjectProperty,
        linkml:SlotDefinition ;
    rdfs:label "timePoint__eventType" ;
    rdfs:domain <https://example.org/crdch_model/TimePoint> ;
    rdfs:range <http://UNKNOWN.org/enum_CRDCH_TimePoint_eventType> ;
    skos:definition "An event that occurred at the point in time specified by this TimePoint." ;
    skos:editorialNote "Cardinality: 0..m" ;
    skos:note "eventType can be used to associate a label for a particular event (e.g. IACUC approval, embargo lifted, etc.) to a dateTime." ;
    linkml:examples "Example(value='', description=None)" .

linkml:timePoint__id a owl:ObjectProperty,
        linkml:SlotDefinition ;
    rdfs:label "timePoint__id" ;
    rdfs:domain <https://example.org/crdch_model/TimePoint> ;
    rdfs:range <https://example.org/crdch_model/Entity> ;
    skos:definition "The 'logical' identifier of the entity within the system of record.  The simple value of this attribute stands for an identifier of this data object within the system, it can be used as a reference from other objects within the same system (i.e. primary and foreign keys), and it should be unique per type of object. The same data object copied to a different system will likely have a different \"id\" in the new system since \"id\" values are system specific and do not represent persistent business identifiers. Business identifiers are assigned outside the information system and are captured in the \"identifier\" field. The \"id\" field is more likely to be a serially or randomly generated value that is assigned to the data object as it is created in a system." ;
    skos:editorialNote "Cardinality: 0..1" ;
    skos:note "FHIR naming conventions are followed here, where 'id' is used for logical identifiers, and 'identifier' for business identifiers.   The identified entity may have a different 'id' in a different system, and have many external business 'identifiers' associated with it. If an \"id\" value can also be considered to be a business identifier, and should be transmissible to other systems, it should be duplicated in the \"identifier\" attribute along with the additional metadata needed to give context to the value of \"id\". An entity in this model that does not have an \"id\" field is considered to be an embeddable entity that can not stand on its own. " ;
    linkml:examples "Example(value='', description=None)" .

linkml:timePoint__indexTimePoint a owl:ObjectProperty,
        linkml:SlotDefinition ;
    rdfs:label "timePoint__indexTimePoint" ;
    rdfs:domain <https://example.org/crdch_model/TimePoint> ;
    rdfs:range <https://example.org/crdch_model/TimePoint> ;
    skos:definition "Another TimePoint from which this point is offset." ;
    skos:editorialNote "Cardinality: 0..1" ;
    linkml:examples "Example(value='', description=None)" .

linkml:timePoint__offsetFromIndex a owl:ObjectProperty,
        linkml:SlotDefinition ;
    rdfs:label "timePoint__offsetFromIndex" ;
    rdfs:domain <https://example.org/crdch_model/TimePoint> ;
    rdfs:range <https://example.org/crdch_model/Quantity> ;
    skos:definition "A quantity of time that, together with the index date or event, can be used to derive a specific timepoint." ;
    skos:editorialNote "Cardinality: 0..1" ;
    skos:note "Quantity.unit MUST be a unit of time, and SHOULD be set to 'days'." ;
    linkml:examples "Example(value='', description=None)" .

linkml:tobaccoExposureObservation__category a owl:ObjectProperty,
        linkml:SlotDefinition ;
    rdfs:label "tobaccoExposureObservation__category" ;
    rdfs:domain <https://example.org/crdch_model/TobaccoExposureObservation> ;
    rdfs:range <http://UNKNOWN.org/enum_CRDCH_TobaccoExposureObservation_category> ;
    skos:definition "The general category of observation described" ;
    skos:editorialNote "Cardinality: 0..0" ;
    linkml:examples "Example(value='', description=None)" .

linkml:tobaccoExposureObservation__focus a owl:ObjectProperty,
        linkml:SlotDefinition ;
    rdfs:label "tobaccoExposureObservation__focus" ;
    rdfs:domain <https://example.org/crdch_model/TobaccoExposureObservation> ;
    rdfs:range <https://example.org/crdch_model/Entity> ;
    skos:definition "The entity or entities directly observed/measured in generating an observation result." ;
    skos:editorialNote "Cardinality: 0..0" ;
    skos:note "The 'focus', 'subject', and 'specimen' fields are useful when data creators want an Observation object to stand on its own, so it can point back to the entities it is about.  These fields are not needed when an Observation is embedded in a Specimen or other entity, where focus, subject, and specimen can be determined from context. " ;
    linkml:examples "Example(value='', description=None)" .

linkml:tobaccoExposureObservation__id a owl:ObjectProperty,
        linkml:SlotDefinition ;
    rdfs:label "tobaccoExposureObservation__id" ;
    rdfs:domain <https://example.org/crdch_model/TobaccoExposureObservation> ;
    rdfs:range <https://example.org/crdch_model/Entity> ;
    skos:definition "The 'logical' identifier of the entity within the system of record.  The simple value of this attribute stands for an identifier of this data object within the system, it can be used as a reference from other objects within the same system (i.e. primary and foreign keys), and it should be unique per type of object. The same data object copied to a different system will likely have a different \"id\" in the new system since \"id\" values are system specific and do not represent persistent business identifiers. Business identifiers are assigned outside the information system and are captured in the \"identifier\" field. The \"id\" field is more likely to be a serially or randomly generated value that is assigned to the data object as it is created in a system." ;
    skos:editorialNote "Cardinality: 0..0" ;
    skos:note "FHIR naming conventions are followed here, where 'id' is used for logical identifiers, and 'identifier' for business identifiers.   The identified entity may have a different 'id' in a different system, and have many external business 'identifiers' associated with it. If an \"id\" value can also be considered to be a business identifier, and should be transmissible to other systems, it should be duplicated in the \"identifier\" attribute along with the additional metadata needed to give context to the value of \"id\". An entity in this model that does not have an \"id\" field is considered to be an embeddable entity that can not stand on its own. " ;
    linkml:examples "Example(value='', description=None)" .

linkml:tobaccoExposureObservation__method_type a owl:ObjectProperty,
        linkml:SlotDefinition ;
    rdfs:label "tobaccoExposureObservation__method_type" ;
    rdfs:domain <https://example.org/crdch_model/TobaccoExposureObservation> ;
    rdfs:range <http://UNKNOWN.org/enum_CRDCH_TobaccoExposureObservation_method_type> ;
    skos:definition "A type of method used in generating the Observation result." ;
    skos:editorialNote "Cardinality: 0..0" ;
    skos:note "This may be a type of observational, measurement, experimental, or computational method specifying how to generate data (e.g. 'manual counting', 'bright field microscopy',). Or a Guideline or SOP specifying how to interpret data and/or encode the result of an  Observation (e.g. a Cancer Staging system such as that defined by the AJCC, or variant interpretation guideline such as that provided by the ACMG)." ;
    linkml:examples "Example(value='', description=None)" .

linkml:tobaccoExposureObservation__observation_type a owl:ObjectProperty,
        linkml:SlotDefinition ;
    rdfs:label "tobaccoExposureObservation__observation_type" ;
    rdfs:domain <https://example.org/crdch_model/TobaccoExposureObservation> ;
    rdfs:range <http://UNKNOWN.org/enum_CRDCH_TobaccoExposureObservation_observation_type> ;
    skos:definition "The specific type of tobacco exposure observation made - i.e. the feature or characteristic that was observed, measured, estimated, etc.." ;
    skos:editorialNote "Cardinality: 1..1" ;
    skos:note "This field holds the 'key' in the core key-value pair comprised of the observation_type field and the relevant value(s) field." ;
    linkml:examples "Example(value='cigarettes_per_day', description=None)",
        "Example(value='environmental_tobacco_smoke_exposure', description=None)",
        "Example(value='pack_years_smoked', description=None)",
        "Example(value='smoking_frequency', description=None)",
        "Example(value='time_between_waking_and_first_smoke', description=None)",
        "Example(value='tobacco_smoking_onset_year', description=None)",
        "Example(value='tobacco_smoking_quit_year', description=None)",
        "Example(value='tobacco_smoking_status', description=None)",
        "Example(value='type_of_tobacco_used', description=None)",
        "Example(value='years_smoked', description=None)" .

linkml:tobaccoExposureObservation__performed_by a owl:ObjectProperty,
        linkml:SlotDefinition ;
    rdfs:label "tobaccoExposureObservation__performed_by" ;
    rdfs:domain <https://example.org/crdch_model/TobaccoExposureObservation> ;
    rdfs:range <https://example.org/crdch_model/Organization> ;
    skos:definition "The organization or group that performed the observation activity." ;
    skos:editorialNote "Cardinality: 0..0" ;
    linkml:examples "Example(value='', description=None)" .

linkml:tobaccoExposureObservation__subject a owl:ObjectProperty,
        linkml:SlotDefinition ;
    rdfs:label "tobaccoExposureObservation__subject" ;
    rdfs:domain <https://example.org/crdch_model/TobaccoExposureObservation> ;
    rdfs:range <https://example.org/crdch_model/Subject> ;
    skos:definition "The patient that the observation is about (if not the direct focus).  e.g. observations are often made on specimens derived from a patient, or other entities related to a patient, that ultimately tell us something about the patient of interest." ;
    skos:editorialNote "Cardinality: 0..0" ;
    linkml:examples "Example(value='', description=None)" .

linkml:tobaccoExposureObservation__valueCodeableConcept a owl:ObjectProperty,
        linkml:SlotDefinition ;
    rdfs:label "tobaccoExposureObservation__valueCodeableConcept" ;
    rdfs:domain <https://example.org/crdch_model/TobaccoExposureObservation> ;
    rdfs:range <http://UNKNOWN.org/enum_CRDCH_TobaccoExposureObservation_valueCodeableConcept> ;
    skos:definition "The result of the observation, encoded as a CodeableConcept." ;
    skos:editorialNote "Cardinality: 0..1" ;
    skos:note "One and only one of the value(x) fields must be populated." ;
    linkml:examples "Example(value='', description=None)" .

linkml:tobaccoExposureObservation__valueInteger a owl:ObjectProperty,
        linkml:SlotDefinition ;
    rdfs:label "tobaccoExposureObservation__valueInteger" ;
    rdfs:domain <https://example.org/crdch_model/TobaccoExposureObservation> ;
    rdfs:range <https://example.org/crdch_model/Entity> ;
    skos:definition "The result of the observation, encoded as an integer." ;
    skos:editorialNote "Cardinality: 0..1" ;
    skos:note "One and only one of the value(x) fields must be populated." ;
    linkml:examples "Example(value='', description=None)" .

linkml:treatment__concurrent_treatment a owl:ObjectProperty,
        linkml:SlotDefinition ;
    rdfs:label "treatment__concurrent_treatment" ;
    rdfs:domain <https://example.org/crdch_model/Treatment> ;
    rdfs:range <https://example.org/crdch_model/Treatment> ;
    skos:definition "Treatment instance(s) that are concurrent with this treatment." ;
    skos:editorialNote "Cardinality: 0..m" ;
    linkml:examples "Example(value='', description=None)" .

linkml:treatment__date_ended a owl:ObjectProperty,
        linkml:SlotDefinition ;
    rdfs:label "treatment__date_ended" ;
    rdfs:domain <https://example.org/crdch_model/Treatment> ;
    rdfs:range <https://example.org/crdch_model/TimePoint> ;
    skos:definition "The timepoint at which the treatment ended." ;
    skos:editorialNote "Cardinality: 0..1" ;
    linkml:examples "Example(value='', description=None)" .

linkml:treatment__date_started a owl:ObjectProperty,
        linkml:SlotDefinition ;
    rdfs:label "treatment__date_started" ;
    rdfs:domain <https://example.org/crdch_model/Treatment> ;
    rdfs:range <https://example.org/crdch_model/TimePoint> ;
    skos:definition "The timepoint at which the treatment started." ;
    skos:editorialNote "Cardinality: 0..1" ;
    linkml:examples "Example(value='', description=None)" .

linkml:treatment__id a owl:ObjectProperty,
        linkml:SlotDefinition ;
    rdfs:label "treatment__id" ;
    rdfs:domain <https://example.org/crdch_model/Treatment> ;
    rdfs:range <https://example.org/crdch_model/Entity> ;
    skos:definition "The 'logical' identifier of the entity within the system of record.  The simple value of this attribute stands for an identifier of this data object within the system, it can be used as a reference from other objects within the same system (i.e. primary and foreign keys), and it should be unique per type of object. The same data object copied to a different system will likely have a different \"id\" in the new system since \"id\" values are system specific and do not represent persistent business identifiers. Business identifiers are assigned outside the information system and are captured in the \"identifier\" field. The \"id\" field is more likely to be a serially or randomly generated value that is assigned to the data object as it is created in a system." ;
    skos:editorialNote "Cardinality: 0..1" ;
    skos:note "FHIR naming conventions are followed here, where 'id' is used for logical identifiers, and 'identifier' for business identifiers.   The identified entity may have a different 'id' in a different system, and have many external business 'identifiers' associated with it. If an \"id\" value can also be considered to be a business identifier, and should be transmissible to other systems, it should be duplicated in the \"identifier\" attribute along with the additional metadata needed to give context to the value of \"id\". An entity in this model that does not have an \"id\" field is considered to be an embeddable entity that can not stand on its own. " ;
    linkml:examples "Example(value='', description=None)" .

linkml:treatment__identifier a owl:ObjectProperty,
        linkml:SlotDefinition ;
    rdfs:label "treatment__identifier" ;
    rdfs:domain <https://example.org/crdch_model/Treatment> ;
    rdfs:range <https://example.org/crdch_model/Identifier> ;
    skos:definition "A 'business' identifier or accession number for the entity, typically as provided by an external system or authority, that are globally unique and persist across implementing systems. Also, since these identifiers are created outside the information system through a specific business process, the Identifier type has additional attributes to capture this additional metadata so the actual identifier values are qualified by the context that created those values. This additional context allows \"identifier\" instances to be transmitted as business data across systems while still being able to trace them back to the system of origin." ;
    skos:editorialNote "Cardinality: 0..m" ;
    skos:note "FHIR naming conventions are followed here, where 'id' is used for logical identifiers which are unique only within a given system, and 'identifier' for business identifiers, which are used to connect entities or share content across systems.  The complex 'Identifier' data type is used  to capture the identifier itself, along with metadata about its source." ;
    linkml:examples "Example(value='', description=None)" .

linkml:treatment__number_of_cycles a owl:ObjectProperty,
        linkml:SlotDefinition ;
    rdfs:label "treatment__number_of_cycles" ;
    rdfs:domain <https://example.org/crdch_model/Treatment> ;
    rdfs:range <https://example.org/crdch_model/Entity> ;
    skos:definition "The number of treatment cycles the subject received." ;
    skos:editorialNote "Cardinality: 0..1" ;
    linkml:examples "Example(value='', description=None)" .

linkml:treatment__regimen a owl:ObjectProperty,
        linkml:SlotDefinition ;
    rdfs:label "treatment__regimen" ;
    rdfs:domain <https://example.org/crdch_model/Treatment> ;
    rdfs:range <http://UNKNOWN.org/enum_CRDCH_Treatment_regimen> ;
    skos:definition "The regimen or line of therapy" ;
    skos:editorialNote "Cardinality: 0..1" ;
    linkml:examples "Example(value='', description=None)" .

linkml:treatment__subject a owl:ObjectProperty,
        linkml:SlotDefinition ;
    rdfs:label "treatment__subject" ;
    rdfs:domain <https://example.org/crdch_model/Treatment> ;
    rdfs:range <https://example.org/crdch_model/Subject> ;
    skos:definition "The subject (person, animal, model system) to which the treatment was administered." ;
    skos:editorialNote "Cardinality: 0..1" ;
    linkml:examples "Example(value='', description=None)" .

linkml:treatment__therapeutic_agent a owl:ObjectProperty,
        linkml:SlotDefinition ;
    rdfs:label "treatment__therapeutic_agent" ;
    rdfs:domain <https://example.org/crdch_model/Treatment> ;
    rdfs:range <https://example.org/crdch_model/Substance> ;
    skos:definition "One or more therapeutic agents that are administered as part of this treatment." ;
    skos:editorialNote "Cardinality: 0..1" ;
    linkml:examples "Example(value='', description=None)" .

linkml:treatment__treatment_anatomic_site a owl:ObjectProperty,
        linkml:SlotDefinition ;
    rdfs:label "treatment__treatment_anatomic_site" ;
    rdfs:domain <https://example.org/crdch_model/Treatment> ;
    rdfs:range <https://example.org/crdch_model/BodySite> ;
    skos:definition "The anatomical site that the treatment targets." ;
    skos:editorialNote "Cardinality: 0..1" ;
    linkml:examples "Example(value='', description=None)" .

linkml:treatment__treatment_effect a owl:ObjectProperty,
        linkml:SlotDefinition ;
    rdfs:label "treatment__treatment_effect" ;
    rdfs:domain <https://example.org/crdch_model/Treatment> ;
    rdfs:range <http://UNKNOWN.org/enum_CRDCH_Treatment_treatment_effect> ;
    skos:definition "The effect of a treatment on the diagnosis or tumor." ;
    skos:editorialNote "Cardinality: 0..1" ;
    linkml:examples "Example(value='Complete Necrosis (No Viable Tumor)', description=None)",
        "Example(value='No Necrosis', description=None)" .

linkml:treatment__treatment_end_reason a owl:ObjectProperty,
        linkml:SlotDefinition ;
    rdfs:label "treatment__treatment_end_reason" ;
    rdfs:domain <https://example.org/crdch_model/Treatment> ;
    rdfs:range <http://UNKNOWN.org/enum_CRDCH_Treatment_treatment_end_reason> ;
    skos:definition "The reason the treatment ended." ;
    skos:editorialNote "Cardinality: 0..m" ;
    linkml:examples "Example(value='Adverse Event Course of Therapy Completed', description=None)",
        "Example(value='Death', description=None)",
        "Example(value='Disease Progression', description=None)",
        "Example(value='Other', description=None)" .

linkml:treatment__treatment_for_diagnosis a owl:ObjectProperty,
        linkml:SlotDefinition ;
    rdfs:label "treatment__treatment_for_diagnosis" ;
    rdfs:domain <https://example.org/crdch_model/Treatment> ;
    rdfs:range <https://example.org/crdch_model/Diagnosis> ;
    skos:definition "The diagnosis for which this treatment is intended." ;
    skos:editorialNote "Cardinality: 0..m" ;
    linkml:examples "Example(value='', description=None)" .

linkml:treatment__treatment_frequency a owl:ObjectProperty,
        linkml:SlotDefinition ;
    rdfs:label "treatment__treatment_frequency" ;
    rdfs:domain <https://example.org/crdch_model/Treatment> ;
    rdfs:range <http://UNKNOWN.org/enum_CRDCH_Treatment_treatment_frequency> ;
    skos:definition "The frequency of using the substance described by this instance." ;
    skos:editorialNote "Cardinality: 0..1" ;
    linkml:examples "Example(value='Every Hour', description=None)",
        "Example(value='Five Times Daily', description=None)",
        "Example(value='Four Times Daily', description=None)",
        "Example(value='Three Times Daily', description=None)" .

linkml:treatment__treatment_intent a owl:ObjectProperty,
        linkml:SlotDefinition ;
    rdfs:label "treatment__treatment_intent" ;
    rdfs:domain <https://example.org/crdch_model/Treatment> ;
    rdfs:range <http://UNKNOWN.org/enum_CRDCH_Treatment_treatment_intent> ;
    skos:definition "The medical intent of the treatment." ;
    skos:editorialNote "Cardinality: 0..1" ;
    linkml:examples "Example(value='Adjuvant', description=None)",
        "Example(value='Cure', description=None)",
        "Example(value='Palliative', description=None)" .

linkml:treatment__treatment_outcome a owl:ObjectProperty,
        linkml:SlotDefinition ;
    rdfs:label "treatment__treatment_outcome" ;
    rdfs:domain <https://example.org/crdch_model/Treatment> ;
    rdfs:range <http://UNKNOWN.org/enum_CRDCH_Treatment_treatment_outcome> ;
    skos:definition "The final outcome of the treatment." ;
    skos:editorialNote "Cardinality: 0..1" ;
    linkml:examples "Example(value='Complete Response', description=None)",
        "Example(value='Mixed Response', description=None)",
        "Example(value='No Measurable Disease', description=None)",
        "Example(value='No Response', description=None)",
        "Example(value='Partial Response', description=None)",
        "Example(value='Persistent Disease', description=None)" .

linkml:treatment__treatment_type a owl:ObjectProperty,
        linkml:SlotDefinition ;
    rdfs:label "treatment__treatment_type" ;
    rdfs:domain <https://example.org/crdch_model/Treatment> ;
    rdfs:range <http://UNKNOWN.org/enum_CRDCH_Treatment_treatment_type> ;
    skos:definition "The type of treatment administered, which may include medication/therapeutics or other procedures." ;
    skos:editorialNote "Cardinality: 0..1" ;
    linkml:examples "Example(value='Ablation', description=None)",
        "Example(value='Ablation, Cryo Ablation', description=None)",
        "Example(value='Ethanol Injection Ablation', description=None)",
        "Example(value='Microwave Ablation', description=None)",
        "Example(value='Radiofrequency', description=None)",
        "Example(value='Stem Cell Transplantation', description=None)" .

linkml:Boolean a owl:Class,
        linkml:TypeDefinition ;
    rdfs:label "boolean" ;
    rdfs:subClassOf [ a owl:Restriction ;
            owl:onDataRange xsd:boolean ;
            owl:onProperty linkml:topValue ;
            owl:qualifiedCardinality 1 ] ;
    skos:definition "A binary (true or false) value" .

linkml:Datetime a owl:Class,
        linkml:TypeDefinition ;
    rdfs:label "datetime" ;
    rdfs:subClassOf [ a owl:Restriction ;
            owl:onDataRange xsd:dateTime ;
            owl:onProperty linkml:topValue ;
            owl:qualifiedCardinality 1 ] ;
    skos:definition "The combination of a date and time" .

linkml:Decimal a owl:Class,
        linkml:TypeDefinition ;
    rdfs:label "decimal" ;
    rdfs:subClassOf [ a owl:Restriction ;
            owl:onDataRange xsd:decimal ;
            owl:onProperty linkml:topValue ;
            owl:qualifiedCardinality 1 ] ;
    skos:definition "A real number with arbitrary precision that conforms to the xsd:decimal specification" .

linkml:Integer a owl:Class,
        linkml:TypeDefinition ;
    rdfs:label "integer" ;
    rdfs:subClassOf [ a owl:Restriction ;
            owl:onDataRange xsd:integer ;
            owl:onProperty linkml:topValue ;
            owl:qualifiedCardinality 1 ] ;
    skos:definition "An integer" .

linkml:Uriorcurie a owl:Class,
        linkml:TypeDefinition ;
    rdfs:label "uriorcurie" ;
    rdfs:subClassOf [ a owl:Restriction ;
            owl:onDataRange xsd:anyURI ;
            owl:onProperty linkml:topValue ;
            owl:qualifiedCardinality 1 ] ;
    skos:definition "a URI or a CURIE" .

<https://example.org/crdch_model/CodeableConcept> a owl:Class,
        linkml:ClassDefinition ;
    rdfs:label "CodeableConcept" ;
    rdfs:subClassOf [ a owl:Restriction ;
            owl:allValuesFrom <https://example.org/crdch_model/Coding> ;
            owl:onProperty linkml:coding ],
        [ a owl:Restriction ;
            owl:maxQualifiedCardinality 1 ;
            owl:onClass <https://example.org/crdch_model/Entity> ;
            owl:onProperty linkml:text ],
        <https://example.org/crdch_model/Entity> ;
    skos:definition "A representation of a concept that may be defined by or mapped to one or more codes in code systems (terminologies, ontologies, dictionaries, code sets, etc) - but may also be defined by the provision of text." ;
    skos:editorialNote "Derived from [CodeableConcept in sheet CodeableConcept](https://docs.google.com/spreadsheets/d/1oWS7cao-fgz2MKWtyr8h2dEL9unX__0bJrWKv6mQmM4/edit#gid=1820375300)" ;
    skos:note "More than one code may be used in CodeableConcept. The concept may be coded multiple times in different code systems (or even multiple times in the same code systems, where multiple forms are possible). Each Coding is a representation of the concept as described above and may have slightly different granularity due to the differences in the definitions of the underlying codes. There is no meaning associated with the ordering of Coding within a CodeableConcept. A typical use of CodeableConcept is to send the local code that the concept was coded with, and also one or more translations to publicly defined code systems such as LOINC or SNOMED CT. " .

<https://example.org/crdch_model/TimePeriod> a owl:Class,
        linkml:ClassDefinition ;
    rdfs:label "TimePeriod" ;
    rdfs:subClassOf [ a owl:Restriction ;
            owl:maxQualifiedCardinality 1 ;
            owl:onClass <https://example.org/crdch_model/TimePoint> ;
            owl:onProperty linkml:periodEnd_end ],
        [ a owl:Restriction ;
            owl:maxQualifiedCardinality 1 ;
            owl:onClass <https://example.org/crdch_model/TimePoint> ;
            owl:onProperty linkml:periodStart_start ],
        <https://example.org/crdch_model/Entity> ;
    skos:definition "A period of time between a start and end time point." ;
    skos:editorialNote "Derived from [TimePeriod in sheet TimePeriod](https://docs.google.com/spreadsheets/d/1oWS7cao-fgz2MKWtyr8h2dEL9unX__0bJrWKv6mQmM4/edit#gid=1590126992)" .

linkml:String a owl:Class,
        linkml:TypeDefinition ;
    rdfs:label "string" ;
    rdfs:subClassOf [ a owl:Restriction ;
            owl:onDataRange xsd:string ;
            owl:onProperty linkml:topValue ;
            owl:qualifiedCardinality 1 ] ;
    skos:definition "A character string" .

<https://example.org/crdch_model/Exposure> a owl:Class,
        linkml:ClassDefinition ;
    rdfs:label "Exposure" ;
    rdfs:subClassOf [ a owl:Restriction ;
            owl:onClass <https://example.org/crdch_model/Entity> ;
            owl:onProperty linkml:id ;
            owl:qualifiedCardinality 1 ],
        [ a owl:Restriction ;
            owl:maxQualifiedCardinality 1 ;
            owl:onClass <https://example.org/crdch_model/Subject> ;
            owl:onProperty linkml:subject ],
        [ a owl:Restriction ;
            owl:allValuesFrom <https://example.org/crdch_model/TobaccoExposureObservation> ;
            owl:onProperty linkml:tobacco_exposure ],
        [ a owl:Restriction ;
            owl:allValuesFrom <https://example.org/crdch_model/Identifier> ;
            owl:onProperty linkml:identifier ],
        [ a owl:Restriction ;
            owl:allValuesFrom <https://example.org/crdch_model/AlcoholExposureObservation> ;
            owl:onProperty linkml:alcohol_exposure ],
        [ a owl:Restriction ;
            owl:allValuesFrom <https://example.org/crdch_model/EnvironmentalExposureObservation> ;
            owl:onProperty linkml:environmental_exposure ],
        <https://example.org/crdch_model/Entity> ;
    skos:definition "Contact between an agent and a target. A state of contact or close proximity to a medicinal product, chemical, pathogen, radioisotope or other substance." ;
    skos:editorialNote "Derived from [Exposure in sheet Exposure](https://docs.google.com/spreadsheets/d/1oWS7cao-fgz2MKWtyr8h2dEL9unX__0bJrWKv6mQmM4/edit#gid=1402410931)" .

<https://example.org/crdch_model/Coding> a owl:Class,
        linkml:ClassDefinition ;
    rdfs:label "Coding" ;
    rdfs:subClassOf [ a owl:Restriction ;
            owl:maxQualifiedCardinality 1 ;
            owl:onClass <https://example.org/crdch_model/Entity> ;
            owl:onProperty linkml:label ],
        [ a owl:Restriction ;
            owl:maxQualifiedCardinality 1 ;
            owl:onClass <https://example.org/crdch_model/Entity> ;
            owl:onProperty linkml:systemURL ],
        [ a owl:Restriction ;
            owl:onClass <https://example.org/crdch_model/Entity> ;
            owl:onProperty linkml:code ;
            owl:qualifiedCardinality 1 ],
        [ a owl:Restriction ;
            owl:onClass <https://example.org/crdch_model/Entity> ;
            owl:onProperty linkml:system ;
            owl:qualifiedCardinality 1 ],
        [ a owl:Restriction ;
            owl:maxQualifiedCardinality 1 ;
            owl:onClass <https://example.org/crdch_model/Entity> ;
            owl:onProperty linkml:systemVersion ],
        <https://example.org/crdch_model/Entity> ;
    skos:definition "A structured representation of a coded/enumerated data value, that includes additional metadata about the code and code system." ;
    skos:editorialNote "Derived from [Coding in sheet Coding](https://docs.google.com/spreadsheets/d/1oWS7cao-fgz2MKWtyr8h2dEL9unX__0bJrWKv6mQmM4/edit#gid=1218588936)" .

<https://example.org/crdch_model/ObservationSet> a owl:Class,
        linkml:ClassDefinition ;
    rdfs:label "ObservationSet" ;
    rdfs:subClassOf [ a owl:Restriction ;
            owl:allValuesFrom <https://example.org/crdch_model/Observation> ;
            owl:onProperty linkml:observations ],
        [ a owl:Restriction ;
            owl:allValuesFrom <https://example.org/crdch_model/Entity> ;
            owl:onProperty linkml:focus ],
        [ a owl:Restriction ;
            owl:onClass <http://UNKNOWN.org/enum_CRDCH_ObservationSet_category> ;
            owl:onProperty linkml:category ;
            owl:qualifiedCardinality 1 ],
        [ a owl:Restriction ;
            owl:maxQualifiedCardinality 1 ;
            owl:onClass <https://example.org/crdch_model/Subject> ;
            owl:onProperty linkml:subject ],
        [ a owl:Restriction ;
            owl:allValuesFrom <http://UNKNOWN.org/enum_CRDCH_ObservationSet_method_type> ;
            owl:onProperty linkml:method_type ],
        [ a owl:Restriction ;
            owl:maxQualifiedCardinality 1 ;
            owl:onClass <https://example.org/crdch_model/Organization> ;
            owl:onProperty linkml:performed_by ],
        [ a owl:Restriction ;
            owl:onClass <https://example.org/crdch_model/Entity> ;
            owl:onProperty linkml:id ;
            owl:qualifiedCardinality 1 ],
        <https://example.org/crdch_model/Entity> ;
    skos:definition "A structured object to hold related data items about an entity, as generated through a point-in-time observation, measurement, or interpretation." ;
    skos:editorialNote "Derived from [ObservationSet in sheet ObservationSet](https://docs.google.com/spreadsheets/d/1oWS7cao-fgz2MKWtyr8h2dEL9unX__0bJrWKv6mQmM4/edit#gid=1243450201)" ;
    skos:note "An Observation Set is comprised of one or more logically related Observations made about the same entity. The Observations in a set may be grouped because they were generated on a single occasion using a common methodology (e.g. a blood panel), and/or or because describe aspects of the same underlying feature of an entity and as such are considered together as a logical unit of information (e.g. diastolic and systolic measures that comprise a blood pressure observation, or T, N, and M components of a Cancer Staging observation)." .

<https://example.org/crdch_model/BiologicProduct> a owl:Class,
        linkml:ClassDefinition ;
    rdfs:label "BiologicProduct" ;
    rdfs:subClassOf [ a owl:Restriction ;
            owl:maxQualifiedCardinality 1 ;
            owl:onClass <https://example.org/crdch_model/Entity> ;
            owl:onProperty linkml:description ],
        [ a owl:Restriction ;
            owl:allValuesFrom <https://example.org/crdch_model/Entity> ;
            owl:onProperty linkml:passage_number ],
        [ a owl:Restriction ;
            owl:allValuesFrom <https://example.org/crdch_model/Identifier> ;
            owl:onProperty linkml:identifier ],
        [ a owl:Restriction ;
            owl:maxQualifiedCardinality 1 ;
            owl:onClass <http://UNKNOWN.org/enum_CRDCH_BiologicProduct_product_type> ;
            owl:onProperty linkml:product_type ],
        [ a owl:Restriction ;
            owl:maxQualifiedCardinality 1 ;
            owl:onClass <https://example.org/crdch_model/Entity> ;
            owl:onProperty linkml:id ],
        [ a owl:Restriction ;
            owl:allValuesFrom <https://example.org/crdch_model/Entity> ;
            owl:onProperty linkml:growth_rate ],
        <https://example.org/crdch_model/Entity> ;
    skos:definition "A living organism, or a metabolically active biological system such as a cell culture, tissue culture, or organoid that is maintained or propagated in vitro." ;
    skos:editorialNote "Derived from [BiologicProduct in sheet BiologicProduct](https://docs.google.com/spreadsheets/d/1oWS7cao-fgz2MKWtyr8h2dEL9unX__0bJrWKv6mQmM4/edit#gid=1097989080)" .

<https://example.org/crdch_model/Document> a owl:Class,
        linkml:ClassDefinition ;
    rdfs:label "Document" ;
    rdfs:subClassOf [ a owl:Restriction ;
            owl:maxQualifiedCardinality 1 ;
            owl:onClass <https://example.org/crdch_model/Entity> ;
            owl:onProperty linkml:id ],
        [ a owl:Restriction ;
            owl:maxQualifiedCardinality 1 ;
            owl:onClass <https://example.org/crdch_model/Entity> ;
            owl:onProperty linkml:description ],
        [ a owl:Restriction ;
            owl:allValuesFrom <https://example.org/crdch_model/Entity> ;
            owl:onProperty linkml:url ],
        [ a owl:Restriction ;
            owl:allValuesFrom <https://example.org/crdch_model/Identifier> ;
            owl:onProperty linkml:identifier ],
        [ a owl:Restriction ;
            owl:maxQualifiedCardinality 1 ;
            owl:onClass <http://UNKNOWN.org/enum_CRDCH_Document_document_type> ;
            owl:onProperty linkml:document_type ],
        [ a owl:Restriction ;
            owl:maxQualifiedCardinality 1 ;
            owl:onClass <https://example.org/crdch_model/Entity> ;
            owl:onProperty linkml:focus ],
        <https://example.org/crdch_model/Entity> ;
    skos:definition "A collection of information intented to be understood together as a whole, and codified in human-readable form." ;
    skos:editorialNote "Derived from [Document in sheet Document](https://docs.google.com/spreadsheets/d/1oWS7cao-fgz2MKWtyr8h2dEL9unX__0bJrWKv6mQmM4/edit#gid=809861603)" .

<https://example.org/crdch_model/SpecimenStorageActivity> a owl:Class,
        linkml:ClassDefinition ;
    rdfs:label "SpecimenStorageActivity" ;
    rdfs:subClassOf [ a owl:Restriction ;
            owl:maxQualifiedCardinality 1 ;
            owl:onClass <https://example.org/crdch_model/TimePoint> ;
            owl:onProperty linkml:date_started ],
        [ a owl:Restriction ;
            owl:maxQualifiedCardinality 1 ;
            owl:onClass <https://example.org/crdch_model/Organization> ;
            owl:onProperty linkml:performed_by ],
        [ a owl:Restriction ;
            owl:allValuesFrom <https://example.org/crdch_model/SpecimenContainer> ;
            owl:onProperty linkml:container ],
        [ a owl:Restriction ;
            owl:maxQualifiedCardinality 1 ;
            owl:onClass <http://UNKNOWN.org/enum_CRDCH_SpecimenStorageActivity_method_type> ;
            owl:onProperty linkml:method_type ],
        [ a owl:Restriction ;
            owl:maxQualifiedCardinality 1 ;
            owl:onClass <https://example.org/crdch_model/Quantity> ;
            owl:onProperty linkml:duration ],
        [ a owl:Restriction ;
            owl:maxQualifiedCardinality 1 ;
            owl:onClass <https://example.org/crdch_model/TimePoint> ;
            owl:onProperty linkml:date_ended ],
        <https://example.org/crdch_model/Entity> ;
    skos:definition """An activity in which a specimen is stored or maintained in a particular location, container, or state. Unlike 'processing' activities, storage does not alter the 
intrinsic physical nature of a specimen.""" ;
    skos:editorialNote "Derived from [SpecimenStorageActivity in sheet SpecimenStorageActivity](https://docs.google.com/spreadsheets/d/1oWS7cao-fgz2MKWtyr8h2dEL9unX__0bJrWKv6mQmM4/edit#gid=1583133214)" ;
    skos:note "Think of the StorageActivity as being one of many possible periods when the specimen was stored at some location and in some state or condition.  We may want to capture storage dates and conditions for each." .

<https://example.org/crdch_model/CancerGradeObservation> a owl:Class,
        linkml:ClassDefinition ;
    rdfs:label "CancerGradeObservation" ;
    rdfs:subClassOf [ a owl:Restriction ;
            owl:maxQualifiedCardinality 1 ;
            owl:onClass <https://example.org/crdch_model/Entity> ;
            owl:onProperty linkml:id ],
        [ a owl:Restriction ;
            owl:onClass <http://UNKNOWN.org/enum_CRDCH_CancerGradeObservation_observation_type> ;
            owl:onProperty linkml:observation_type ;
            owl:qualifiedCardinality 1 ],
        [ a owl:Restriction ;
            owl:maxQualifiedCardinality 1 ;
            owl:onClass <http://UNKNOWN.org/enum_CRDCH_CancerGradeObservation_method_type> ;
            owl:onProperty linkml:method_type ],
        [ a owl:Restriction ;
            owl:maxQualifiedCardinality 1 ;
            owl:onClass <http://UNKNOWN.org/enum_CRDCH_CancerGradeObservation_category> ;
            owl:onProperty linkml:category ],
        [ a owl:Restriction ;
            owl:maxQualifiedCardinality 1 ;
            owl:onClass <https://example.org/crdch_model/Subject> ;
            owl:onProperty linkml:subject ],
        [ a owl:Restriction ;
            owl:onClass <http://UNKNOWN.org/enum_CRDCH_CancerGradeObservation_valueCodeableConcept> ;
            owl:onProperty linkml:valueCodeableConcept ;
            owl:qualifiedCardinality 1 ],
        [ a owl:Restriction ;
            owl:maxQualifiedCardinality 1 ;
            owl:onClass <https://example.org/crdch_model/Entity> ;
            owl:onProperty linkml:focus ],
        <https://example.org/crdch_model/Entity> ;
    skos:definition "A data structure with key (observation_type) and value (valueCodeableConcept) attributes that represents a single cancer grade observation" ;
    skos:editorialNote "Derived from [CancerGradeObservation in sheet CancerGradeObservation](https://docs.google.com/spreadsheets/d/1oWS7cao-fgz2MKWtyr8h2dEL9unX__0bJrWKv6mQmM4/edit#gid=1099484640)" .

<https://example.org/crdch_model/CancerGradeObservationSet> a owl:Class,
        linkml:ClassDefinition ;
    rdfs:label "CancerGradeObservationSet" ;
    rdfs:subClassOf [ a owl:Restriction ;
            owl:allValuesFrom <https://example.org/crdch_model/Entity> ;
            owl:onProperty linkml:focus ],
        [ a owl:Restriction ;
            owl:maxQualifiedCardinality 1 ;
            owl:onClass <http://UNKNOWN.org/enum_CRDCH_CancerGradeObservationSet_category> ;
            owl:onProperty linkml:category ],
        [ a owl:Restriction ;
            owl:maxQualifiedCardinality 1 ;
            owl:onClass <https://example.org/crdch_model/Entity> ;
            owl:onProperty linkml:id ],
        [ a owl:Restriction ;
            owl:maxQualifiedCardinality 1 ;
            owl:onClass <https://example.org/crdch_model/Subject> ;
            owl:onProperty linkml:subject ],
        [ a owl:Restriction ;
            owl:maxQualifiedCardinality 1 ;
            owl:onClass <https://example.org/crdch_model/Organization> ;
            owl:onProperty linkml:performed_by ],
        [ a owl:Restriction ;
            owl:allValuesFrom <https://example.org/crdch_model/CancerGradeObservation> ;
            owl:onProperty linkml:observations ],
        [ a owl:Restriction ;
            owl:allValuesFrom <http://UNKNOWN.org/enum_CRDCH_CancerGradeObservationSet_method_type> ;
            owl:onProperty linkml:method_type ],
        <https://example.org/crdch_model/Entity> ;
    skos:definition "A structured object to hold related data items about the grade of cancer (e.g. overall, primary gleason, secondary gleason, etc.)." ;
    skos:editorialNote "Derived from [CancerGradeObservationSet in sheet CancerGradeObservationSet](https://docs.google.com/spreadsheets/d/1oWS7cao-fgz2MKWtyr8h2dEL9unX__0bJrWKv6mQmM4/edit#gid=1025765903)" .

<https://example.org/crdch_model/CancerStageObservationSet> a owl:Class,
        linkml:ClassDefinition ;
    rdfs:label "CancerStageObservationSet" ;
    rdfs:subClassOf [ a owl:Restriction ;
            owl:allValuesFrom <https://example.org/crdch_model/CancerStageObservation> ;
            owl:onProperty linkml:observations ],
        [ a owl:Restriction ;
            owl:maxQualifiedCardinality 1 ;
            owl:onClass <https://example.org/crdch_model/Entity> ;
            owl:onProperty linkml:id ],
        [ a owl:Restriction ;
            owl:allValuesFrom <https://example.org/crdch_model/Entity> ;
            owl:onProperty linkml:focus ],
        [ a owl:Restriction ;
            owl:allValuesFrom <http://UNKNOWN.org/enum_CRDCH_CancerStageObservationSet_method_type> ;
            owl:onProperty linkml:method_type ],
        [ a owl:Restriction ;
            owl:maxQualifiedCardinality 1 ;
            owl:onClass <https://example.org/crdch_model/Organization> ;
            owl:onProperty linkml:performed_by ],
        [ a owl:Restriction ;
            owl:maxQualifiedCardinality 1 ;
            owl:onClass <https://example.org/crdch_model/Subject> ;
            owl:onProperty linkml:subject ],
        [ a owl:Restriction ;
            owl:maxQualifiedCardinality 1 ;
            owl:onClass <http://UNKNOWN.org/enum_CRDCH_CancerStageObservationSet_category> ;
            owl:onProperty linkml:category ],
        <https://example.org/crdch_model/Entity> ;
    skos:definition "A structured object to hold related data items about the staging of cancer (e.g. overall, T, N, and M components of a Cancer Staging observation)." ;
    skos:editorialNote "Derived from [CancerStageObservationSet in sheet CancerStageObservationSet](https://docs.google.com/spreadsheets/d/1oWS7cao-fgz2MKWtyr8h2dEL9unX__0bJrWKv6mQmM4/edit#gid=1668576212)" .

<https://example.org/crdch_model/HistologicalCompositionObservationSet> a owl:Class,
        linkml:ClassDefinition ;
    rdfs:label "HistologicalCompositionObservationSet" ;
    rdfs:subClassOf [ a owl:Restriction ;
            owl:allValuesFrom <http://UNKNOWN.org/enum_CRDCH_HistologicalCompositionObservationSet_method_type> ;
            owl:onProperty linkml:method_type ],
        [ a owl:Restriction ;
            owl:onClass <https://example.org/crdch_model/Entity> ;
            owl:onProperty linkml:id ;
            owl:qualifiedCardinality 1 ],
        [ a owl:Restriction ;
            owl:allValuesFrom <https://example.org/crdch_model/HistologicalCompositionObservation> ;
            owl:onProperty linkml:observations ],
        [ a owl:Restriction ;
            owl:maxQualifiedCardinality 1 ;
            owl:onClass <https://example.org/crdch_model/Organization> ;
            owl:onProperty linkml:performed_by ],
        [ a owl:Restriction ;
            owl:allValuesFrom <https://example.org/crdch_model/Entity> ;
            owl:onProperty linkml:focus ],
        [ a owl:Restriction ;
            owl:maxQualifiedCardinality 1 ;
            owl:onClass <https://example.org/crdch_model/Subject> ;
            owl:onProperty linkml:subject ],
        [ a owl:Restriction ;
            owl:onClass <http://UNKNOWN.org/enum_CRDCH_HistologicalCompositionObservationSet_category> ;
            owl:onProperty linkml:category ;
            owl:qualifiedCardinality 1 ],
        <https://example.org/crdch_model/Entity> ;
    skos:definition "A set of one or more discrete observations that quantify the relative or absolute composition of a specimen at cellular level - e.g. how many cells in the specimen are of a given type, or exhibit a particular cellular phenotype." ;
    skos:editorialNote "Derived from [HistologicalCompositionObservationSet in sheet HistologicalCompositionObservationSet](https://docs.google.com/spreadsheets/d/1oWS7cao-fgz2MKWtyr8h2dEL9unX__0bJrWKv6mQmM4/edit#gid=815777747)" ;
    skos:note "An Observation Set is comprised of one or more logically related Observations made about the same entity. The Observations in a set may be grouped because they were generated on a single occasion using a common methodology (e.g. a blood panel), and/or or because describe aspects of the same underlying feature of an entity and as such are considered together as a logical unit of information (e.g. diastolic and systolic measures that comprise a blood pressure observation, or T, N, and M components of a Cancer Staging observation)." .

<https://example.org/crdch_model/SpecimenTransportActivity> a owl:Class,
        linkml:ClassDefinition ;
    rdfs:label "SpecimenTransportActivity" ;
    rdfs:subClassOf [ a owl:Restriction ;
            owl:maxQualifiedCardinality 1 ;
            owl:onClass <https://example.org/crdch_model/TimePoint> ;
            owl:onProperty linkml:date_started ],
        [ a owl:Restriction ;
            owl:allValuesFrom <https://example.org/crdch_model/ExecutionConditionObservation> ;
            owl:onProperty linkml:execution_condition_observation ],
        [ a owl:Restriction ;
            owl:maxQualifiedCardinality 1 ;
            owl:onClass <https://example.org/crdch_model/Organization> ;
            owl:onProperty linkml:transport_destination ],
        [ a owl:Restriction ;
            owl:maxQualifiedCardinality 1 ;
            owl:onClass <https://example.org/crdch_model/Organization> ;
            owl:onProperty linkml:performed_by ],
        [ a owl:Restriction ;
            owl:allValuesFrom <https://example.org/crdch_model/Entity> ;
            owl:onProperty linkml:duration ],
        [ a owl:Restriction ;
            owl:maxQualifiedCardinality 1 ;
            owl:onClass <https://example.org/crdch_model/Organization> ;
            owl:onProperty linkml:transport_origin ],
        [ a owl:Restriction ;
            owl:maxQualifiedCardinality 1 ;
            owl:onClass <https://example.org/crdch_model/TimePoint> ;
            owl:onProperty linkml:date_ended ],
        <https://example.org/crdch_model/Entity> ;
    skos:definition "An activity through which a specimen is transported between locations or organizations." ;
    skos:editorialNote "Derived from [SpecimenTransportActivity in sheet SpecimenTransportActivity](https://docs.google.com/spreadsheets/d/1oWS7cao-fgz2MKWtyr8h2dEL9unX__0bJrWKv6mQmM4/edit#gid=359352096)" ;
    skos:note "Think of the TransportActivity as being one of many possible occasions when the specimen was moved from one location to another, in some state or condition.  We may want to capture dates and conditions for each." .

<https://example.org/crdch_model/DimensionalObservation> a owl:Class,
        linkml:ClassDefinition ;
    rdfs:label "DimensionalObservation" ;
    rdfs:subClassOf [ a owl:Restriction ;
            owl:allValuesFrom <http://UNKNOWN.org/enum_CRDCH_DimensionalObservation_method_type> ;
            owl:onProperty linkml:method_type ],
        [ a owl:Restriction ;
            owl:onClass <https://example.org/crdch_model/Quantity> ;
            owl:onProperty linkml:valueQuantity ;
            owl:qualifiedCardinality 1 ],
        [ a owl:Restriction ;
            owl:maxQualifiedCardinality 1 ;
            owl:onClass <https://example.org/crdch_model/Entity> ;
            owl:onProperty linkml:id ],
        [ a owl:Restriction ;
            owl:maxQualifiedCardinality 1 ;
            owl:onClass <https://example.org/crdch_model/Subject> ;
            owl:onProperty linkml:subject ],
        [ a owl:Restriction ;
            owl:maxQualifiedCardinality 1 ;
            owl:onClass <https://example.org/crdch_model/Organization> ;
            owl:onProperty linkml:performed_by ],
        [ a owl:Restriction ;
            owl:onClass <http://UNKNOWN.org/enum_CRDCH_DimensionalObservation_observation_type> ;
            owl:onProperty linkml:observation_type ;
            owl:qualifiedCardinality 1 ],
        [ a owl:Restriction ;
            owl:maxQualifiedCardinality 1 ;
            owl:onClass <http://UNKNOWN.org/enum_CRDCH_DimensionalObservation_category> ;
            owl:onProperty linkml:category ],
        [ a owl:Restriction ;
            owl:allValuesFrom <https://example.org/crdch_model/Entity> ;
            owl:onProperty linkml:focus ],
        <https://example.org/crdch_model/Entity> ;
    skos:definition "A structured object that describes a single data item about the physical dimensions  of an entity (e.g. length width, area), as generated through a point-in-time observation or measurement." ;
    skos:editorialNote "Derived from [DimensionalObservation in sheet DimensionalObservation](https://docs.google.com/spreadsheets/d/1oWS7cao-fgz2MKWtyr8h2dEL9unX__0bJrWKv6mQmM4/edit#gid=1045447308)" ;
    skos:note "At the core of an Observation is a flexible key-value pair (or a structured collection of key-value pairs), where a 'key' field defines the type of observation made, and the 'value' field describes the value or outcome of the observation. The fact that the type of observation captured is defined in the data allow Observation to convey a broad range of observation data." .

<https://example.org/crdch_model/EnvironmentalExposureObservation> a owl:Class,
        linkml:ClassDefinition ;
    rdfs:label "EnvironmentalExposureObservation" ;
    rdfs:subClassOf [ a owl:Restriction ;
            owl:maxQualifiedCardinality 1 ;
            owl:onClass <https://example.org/crdch_model/Subject> ;
            owl:onProperty linkml:subject ],
        [ a owl:Restriction ;
            owl:maxQualifiedCardinality 1 ;
            owl:onClass <http://UNKNOWN.org/enum_CRDCH_EnvironmentalExposureObservation_category> ;
            owl:onProperty linkml:category ],
        [ a owl:Restriction ;
            owl:maxQualifiedCardinality 1 ;
            owl:onClass <https://example.org/crdch_model/Entity> ;
            owl:onProperty linkml:focus ],
        [ a owl:Restriction ;
            owl:onClass <http://UNKNOWN.org/enum_CRDCH_EnvironmentalExposureObservation_observation_type> ;
            owl:onProperty linkml:observation_type ;
            owl:qualifiedCardinality 1 ],
        [ a owl:Restriction ;
            owl:onClass <http://UNKNOWN.org/enum_CRDCH_EnvironmentalExposureObservation_valueCodeableConcept> ;
            owl:onProperty linkml:valueCodeableConcept ;
            owl:qualifiedCardinality 1 ],
        [ a owl:Restriction ;
            owl:maxQualifiedCardinality 1 ;
            owl:onClass <http://UNKNOWN.org/enum_CRDCH_EnvironmentalExposureObservation_method_type> ;
            owl:onProperty linkml:method_type ],
        [ a owl:Restriction ;
            owl:maxQualifiedCardinality 1 ;
            owl:onClass <https://example.org/crdch_model/Entity> ;
            owl:onProperty linkml:id ],
        [ a owl:Restriction ;
            owl:maxQualifiedCardinality 1 ;
            owl:onClass <https://example.org/crdch_model/Organization> ;
            owl:onProperty linkml:performed_by ],
        <https://example.org/crdch_model/Entity> ;
    skos:definition "A structured object that describes a single data item about an individual's exposure to an environmental factor, as generated through a point-in-time observation, measurement, or interpretation." ;
    skos:editorialNote "Derived from [EnvironmentalExposureObservation in sheet EnvironmentalExposureObservation](https://docs.google.com/spreadsheets/d/1oWS7cao-fgz2MKWtyr8h2dEL9unX__0bJrWKv6mQmM4/edit#gid=274611680)" .

<https://example.org/crdch_model/HistologicalCompositionObservation> a owl:Class,
        linkml:ClassDefinition ;
    rdfs:label "HistologicalCompositionObservation" ;
    rdfs:subClassOf [ a owl:Restriction ;
            owl:onClass <https://example.org/crdch_model/Quantity> ;
            owl:onProperty linkml:valueQuantity ;
            owl:qualifiedCardinality 1 ],
        [ a owl:Restriction ;
            owl:maxQualifiedCardinality 1 ;
            owl:onClass <https://example.org/crdch_model/Entity> ;
            owl:onProperty linkml:id ],
        [ a owl:Restriction ;
            owl:maxQualifiedCardinality 1 ;
            owl:onClass <https://example.org/crdch_model/Subject> ;
            owl:onProperty linkml:subject ],
        [ a owl:Restriction ;
            owl:allValuesFrom <https://example.org/crdch_model/Entity> ;
            owl:onProperty linkml:focus ],
        [ a owl:Restriction ;
            owl:allValuesFrom <http://UNKNOWN.org/enum_CRDCH_HistologicalCompositionObservation_method_type> ;
            owl:onProperty linkml:method_type ],
        [ a owl:Restriction ;
            owl:onClass <http://UNKNOWN.org/enum_CRDCH_HistologicalCompositionObservation_observation_type> ;
            owl:onProperty linkml:observation_type ;
            owl:qualifiedCardinality 1 ],
        [ a owl:Restriction ;
            owl:maxQualifiedCardinality 1 ;
            owl:onClass <https://example.org/crdch_model/Organization> ;
            owl:onProperty linkml:performed_by ],
        [ a owl:Restriction ;
            owl:maxQualifiedCardinality 1 ;
            owl:onClass <http://UNKNOWN.org/enum_CRDCH_HistologicalCompositionObservation_category> ;
            owl:onProperty linkml:category ],
        <https://example.org/crdch_model/Entity> ;
    skos:definition "An observation about characteristics of a specimen at a microscopic level - typically related to its cellular or tissue composition. (e.g. how many cells in the specimen are of a given type, or exhibit a particular cellular phenotype)." ;
    skos:editorialNote "Derived from [HistologicalCompositionObservation in sheet HistologicalCompositionObservation](https://docs.google.com/spreadsheets/d/1oWS7cao-fgz2MKWtyr8h2dEL9unX__0bJrWKv6mQmM4/edit#gid=1411171873)" .

<https://example.org/crdch_model/SpecimenQualityObservation> a owl:Class,
        linkml:ClassDefinition ;
    rdfs:label "SpecimenQualityObservation" ;
    rdfs:subClassOf [ a owl:Restriction ;
            owl:allValuesFrom <http://UNKNOWN.org/enum_CRDCH_SpecimenQualityObservation_method_type> ;
            owl:onProperty linkml:method_type ],
        [ a owl:Restriction ;
            owl:maxQualifiedCardinality 1 ;
            owl:onClass <http://UNKNOWN.org/enum_CRDCH_SpecimenQualityObservation_category> ;
            owl:onProperty linkml:category ],
        [ a owl:Restriction ;
            owl:onClass <https://example.org/crdch_model/Quantity> ;
            owl:onProperty linkml:valueQuantity ;
            owl:qualifiedCardinality 1 ],
        [ a owl:Restriction ;
            owl:allValuesFrom <https://example.org/crdch_model/Entity> ;
            owl:onProperty linkml:focus ],
        [ a owl:Restriction ;
            owl:maxQualifiedCardinality 1 ;
            owl:onClass <https://example.org/crdch_model/Organization> ;
            owl:onProperty linkml:performed_by ],
        [ a owl:Restriction ;
            owl:maxQualifiedCardinality 1 ;
            owl:onClass <https://example.org/crdch_model/Entity> ;
            owl:onProperty linkml:id ],
        [ a owl:Restriction ;
            owl:onClass <http://UNKNOWN.org/enum_CRDCH_SpecimenQualityObservation_observation_type> ;
            owl:onProperty linkml:observation_type ;
            owl:qualifiedCardinality 1 ],
        [ a owl:Restriction ;
            owl:maxQualifiedCardinality 1 ;
            owl:onClass <https://example.org/crdch_model/Subject> ;
            owl:onProperty linkml:subject ],
        <https://example.org/crdch_model/Entity> ;
    skos:definition "A structured object that describes a characteristic of a specimen indicative of its quality or suitability for use, as generated through a point-in-time observation or measurement." ;
    skos:editorialNote "Derived from [SpecimenQualityObservation in sheet SpecimenQualityObservation](https://docs.google.com/spreadsheets/d/1oWS7cao-fgz2MKWtyr8h2dEL9unX__0bJrWKv6mQmM4/edit#gid=97281875)" .

<https://example.org/crdch_model/SpecimenQuantityObservation> a owl:Class,
        linkml:ClassDefinition ;
    rdfs:label "SpecimenQuantityObservation" ;
    rdfs:subClassOf [ a owl:Restriction ;
            owl:maxQualifiedCardinality 1 ;
            owl:onClass <https://example.org/crdch_model/Subject> ;
            owl:onProperty linkml:subject ],
        [ a owl:Restriction ;
            owl:onClass <https://example.org/crdch_model/Quantity> ;
            owl:onProperty linkml:valueQuantity ;
            owl:qualifiedCardinality 1 ],
        [ a owl:Restriction ;
            owl:maxQualifiedCardinality 1 ;
            owl:onClass <http://UNKNOWN.org/enum_CRDCH_SpecimenQuantityObservation_category> ;
            owl:onProperty linkml:category ],
        [ a owl:Restriction ;
            owl:maxQualifiedCardinality 1 ;
            owl:onClass <https://example.org/crdch_model/Organization> ;
            owl:onProperty linkml:performed_by ],
        [ a owl:Restriction ;
            owl:maxQualifiedCardinality 1 ;
            owl:onClass <https://example.org/crdch_model/Entity> ;
            owl:onProperty linkml:id ],
        [ a owl:Restriction ;
            owl:allValuesFrom <http://UNKNOWN.org/enum_CRDCH_SpecimenQuantityObservation_method_type> ;
            owl:onProperty linkml:method_type ],
        [ a owl:Restriction ;
            owl:allValuesFrom <https://example.org/crdch_model/Entity> ;
            owl:onProperty linkml:focus ],
        [ a owl:Restriction ;
            owl:onClass <http://UNKNOWN.org/enum_CRDCH_SpecimenQuantityObservation_observation_type> ;
            owl:onProperty linkml:observation_type ;
            owl:qualifiedCardinality 1 ],
        <https://example.org/crdch_model/Entity> ;
    skos:definition "A structured object that describes a single data item about the quantity of an entity, as generated through a point-in-time observation or measurement." ;
    skos:editorialNote "Derived from [SpecimenQuantityObservation in sheet SpecimenQuantityObservation](https://docs.google.com/spreadsheets/d/1oWS7cao-fgz2MKWtyr8h2dEL9unX__0bJrWKv6mQmM4/edit#gid=9917708)" ;
    skos:note "At the core of an Observation is a flexible key-value pair (or a structured collection of key-value pairs), where a 'key' field defines the type of observation made, and the 'value' field describes the value or outcome of the observation. The fact that the type of observation captured is defined in the data allow Observation to convey a broad range of observation data." .

<https://example.org/crdch_model/AlcoholExposureObservation> a owl:Class,
        linkml:ClassDefinition ;
    rdfs:label "AlcoholExposureObservation" ;
    rdfs:subClassOf [ a owl:Restriction ;
            owl:maxQualifiedCardinality 1 ;
            owl:onClass <https://example.org/crdch_model/Entity> ;
            owl:onProperty linkml:id ],
        [ a owl:Restriction ;
            owl:maxQualifiedCardinality 1 ;
            owl:onClass <https://example.org/crdch_model/Entity> ;
            owl:onProperty linkml:focus ],
        [ a owl:Restriction ;
            owl:maxQualifiedCardinality 1 ;
            owl:onClass <http://UNKNOWN.org/enum_CRDCH_AlcoholExposureObservation_method_type> ;
            owl:onProperty linkml:method_type ],
        [ a owl:Restriction ;
            owl:maxQualifiedCardinality 1 ;
            owl:onClass <https://example.org/crdch_model/Subject> ;
            owl:onProperty linkml:subject ],
        [ a owl:Restriction ;
            owl:maxQualifiedCardinality 1 ;
            owl:onClass <https://example.org/crdch_model/Entity> ;
            owl:onProperty linkml:valueInteger ],
        [ a owl:Restriction ;
            owl:maxQualifiedCardinality 1 ;
            owl:onClass <http://UNKNOWN.org/enum_CRDCH_AlcoholExposureObservation_category> ;
            owl:onProperty linkml:category ],
        [ a owl:Restriction ;
            owl:maxQualifiedCardinality 1 ;
            owl:onClass <https://example.org/crdch_model/Organization> ;
            owl:onProperty linkml:performed_by ],
        [ a owl:Restriction ;
            owl:maxQualifiedCardinality 1 ;
            owl:onClass <http://UNKNOWN.org/enum_CRDCH_AlcoholExposureObservation_valueCodeableConcept> ;
            owl:onProperty linkml:valueCodeableConcept ],
        [ a owl:Restriction ;
            owl:onClass <http://UNKNOWN.org/enum_CRDCH_AlcoholExposureObservation_observation_type> ;
            owl:onProperty linkml:observation_type ;
            owl:qualifiedCardinality 1 ],
        <https://example.org/crdch_model/Entity> ;
    skos:definition "A structured object that describes a single data item about an individual's exposure to alcohol, as generated through a point-in-time observation, measurement, or interpretation." ;
    skos:editorialNote "Derived from [AlcoholExposureObservation in sheet AlcoholExposureObservation](https://docs.google.com/spreadsheets/d/1oWS7cao-fgz2MKWtyr8h2dEL9unX__0bJrWKv6mQmM4/edit#gid=1894439514)" .

<https://example.org/crdch_model/CancerStageObservation> a owl:Class,
        linkml:ClassDefinition ;
    rdfs:label "CancerStageObservation" ;
    rdfs:subClassOf [ a owl:Restriction ;
            owl:maxQualifiedCardinality 1 ;
            owl:onClass <https://example.org/crdch_model/Entity> ;
            owl:onProperty linkml:valueEntity ],
        [ a owl:Restriction ;
            owl:maxQualifiedCardinality 1 ;
            owl:onClass <http://UNKNOWN.org/enum_CRDCH_CancerStageObservation_category> ;
            owl:onProperty linkml:category ],
        [ a owl:Restriction ;
            owl:maxQualifiedCardinality 1 ;
            owl:onClass <https://example.org/crdch_model/Subject> ;
            owl:onProperty linkml:subject ],
        [ a owl:Restriction ;
            owl:maxQualifiedCardinality 1 ;
            owl:onClass <https://example.org/crdch_model/Organization> ;
            owl:onProperty linkml:performed_by ],
        [ a owl:Restriction ;
            owl:onClass <http://UNKNOWN.org/enum_CRDCH_CancerStageObservation_valueCodeableConcept> ;
            owl:onProperty linkml:valueCodeableConcept ;
            owl:qualifiedCardinality 1 ],
        [ a owl:Restriction ;
            owl:onClass <http://UNKNOWN.org/enum_CRDCH_CancerStageObservation_observation_type> ;
            owl:onProperty linkml:observation_type ;
            owl:qualifiedCardinality 1 ],
        [ a owl:Restriction ;
            owl:maxQualifiedCardinality 1 ;
            owl:onClass <http://UNKNOWN.org/enum_CRDCH_CancerStageObservation_method_type> ;
            owl:onProperty linkml:method_type ],
        [ a owl:Restriction ;
            owl:maxQualifiedCardinality 1 ;
            owl:onClass <https://example.org/crdch_model/Entity> ;
            owl:onProperty linkml:focus ],
        [ a owl:Restriction ;
            owl:maxQualifiedCardinality 1 ;
            owl:onClass <https://example.org/crdch_model/Entity> ;
            owl:onProperty linkml:id ],
        <https://example.org/crdch_model/Entity> ;
    skos:definition "A data structure with key (observation_type) and value (valueCodeableConcept) attributes that represents a single cancer staging observation, such as the Clinical Metastasis (M) component of a clinical TNM staging." ;
    skos:editorialNote "Derived from [CancerStageObservation in sheet CancerStageObservation](https://docs.google.com/spreadsheets/d/1oWS7cao-fgz2MKWtyr8h2dEL9unX__0bJrWKv6mQmM4/edit#gid=1189722404)" .

<https://example.org/crdch_model/DimensionalObservationSet> a owl:Class,
        linkml:ClassDefinition ;
    rdfs:label "DimensionalObservationSet" ;
    rdfs:subClassOf [ a owl:Restriction ;
            owl:maxQualifiedCardinality 1 ;
            owl:onClass <http://UNKNOWN.org/enum_CRDCH_DimensionalObservationSet_category> ;
            owl:onProperty linkml:category ],
        [ a owl:Restriction ;
            owl:allValuesFrom <https://example.org/crdch_model/Entity> ;
            owl:onProperty linkml:focus ],
        [ a owl:Restriction ;
            owl:maxQualifiedCardinality 1 ;
            owl:onClass <https://example.org/crdch_model/Entity> ;
            owl:onProperty linkml:id ],
        [ a owl:Restriction ;
            owl:maxQualifiedCardinality 1 ;
            owl:onClass <https://example.org/crdch_model/Subject> ;
            owl:onProperty linkml:subject ],
        [ a owl:Restriction ;
            owl:maxQualifiedCardinality 1 ;
            owl:onClass <https://example.org/crdch_model/Organization> ;
            owl:onProperty linkml:performed_by ],
        [ a owl:Restriction ;
            owl:allValuesFrom <https://example.org/crdch_model/DimensionalObservation> ;
            owl:onProperty linkml:observations ],
        [ a owl:Restriction ;
            owl:allValuesFrom <http://UNKNOWN.org/enum_CRDCH_DimensionalObservationSet_method_type> ;
            owl:onProperty linkml:method_type ],
        <https://example.org/crdch_model/Entity> ;
    skos:definition "A set of one or more discrete observations about the physical dimensions of an object (e.g. length, width, area)." ;
    skos:editorialNote "Derived from [DimensionalObservationSet in sheet DimensionalObservationSet](https://docs.google.com/spreadsheets/d/1oWS7cao-fgz2MKWtyr8h2dEL9unX__0bJrWKv6mQmM4/edit#gid=1118507095)" .

<https://example.org/crdch_model/SpecimenProcessingActivity> a owl:Class,
        linkml:ClassDefinition ;
    rdfs:label "SpecimenProcessingActivity" ;
    rdfs:subClassOf [ a owl:Restriction ;
            owl:maxQualifiedCardinality 1 ;
            owl:onClass <https://example.org/crdch_model/TimePoint> ;
            owl:onProperty linkml:date_ended ],
        [ a owl:Restriction ;
            owl:allValuesFrom <https://example.org/crdch_model/Substance> ;
            owl:onProperty linkml:additive ],
        [ a owl:Restriction ;
            owl:maxQualifiedCardinality 1 ;
            owl:onClass <https://example.org/crdch_model/Organization> ;
            owl:onProperty linkml:performed_by ],
        [ a owl:Restriction ;
            owl:allValuesFrom <https://example.org/crdch_model/ExecutionConditionObservation> ;
            owl:onProperty linkml:execution_condition_observation ],
        [ a owl:Restriction ;
            owl:allValuesFrom <https://example.org/crdch_model/ExecutionTimeObservation> ;
            owl:onProperty linkml:execution_time_observation ],
        [ a owl:Restriction ;
            owl:maxQualifiedCardinality 1 ;
            owl:onClass <https://example.org/crdch_model/TimePoint> ;
            owl:onProperty linkml:date_started ],
        [ a owl:Restriction ;
            owl:maxQualifiedCardinality 1 ;
            owl:onClass <http://UNKNOWN.org/enum_CRDCH_SpecimenProcessingActivity_activity_type> ;
            owl:onProperty linkml:activity_type ],
        [ a owl:Restriction ;
            owl:allValuesFrom <https://example.org/crdch_model/Quantity> ;
            owl:onProperty linkml:duration ],
        [ a owl:Restriction ;
            owl:maxQualifiedCardinality 1 ;
            owl:onClass <http://UNKNOWN.org/enum_CRDCH_SpecimenProcessingActivity_method_type> ;
            owl:onProperty linkml:method_type ],
        <https://example.org/crdch_model/Entity> ;
    skos:definition "An activity that modifies the physical structure, composition, or state of a specimen. Unlike SpecimenCreation, SpecimenProcessing activities do not result in the generation of new entities - they take a single specimen as input, and output that same specimen." ;
    skos:editorialNote "Derived from [SpecimenProcessingActivity in sheet SpecimenProcessingActivity](https://docs.google.com/spreadsheets/d/1oWS7cao-fgz2MKWtyr8h2dEL9unX__0bJrWKv6mQmM4/edit#gid=1726416617)" ;
    skos:note "\"Processing\" as defined here alters the physical nature of a specimen, such that storage or transport activities do not qualify as processing activities. When instantiating this class, create a separate instances for each type/method of processing performed (e.g. each method of fixation, freezing, labeling, etc. that is applied)." .

<https://example.org/crdch_model/Substance> a owl:Class,
        linkml:ClassDefinition ;
    rdfs:label "Substance" ;
    rdfs:subClassOf [ a owl:Restriction ;
            owl:maxQualifiedCardinality 1 ;
            owl:onClass <https://example.org/crdch_model/Quantity> ;
            owl:onProperty linkml:substance_quantity ],
        [ a owl:Restriction ;
            owl:allValuesFrom <http://UNKNOWN.org/enum_CRDCH_Substance_role> ;
            owl:onProperty linkml:role ],
        [ a owl:Restriction ;
            owl:maxQualifiedCardinality 1 ;
            owl:onClass <http://UNKNOWN.org/enum_CRDCH_Substance_substance_type> ;
            owl:onProperty linkml:substance_type ],
        <https://example.org/crdch_model/Entity> ;
    skos:definition "A type of material substance, or instance thereof,  as used in a particular application. May include information about the role the substance played in a particular application." ;
    skos:editorialNote "Derived from [Substance in sheet Substance](https://docs.google.com/spreadsheets/d/1oWS7cao-fgz2MKWtyr8h2dEL9unX__0bJrWKv6mQmM4/edit#gid=385534272)" .

<https://example.org/crdch_model/TobaccoExposureObservation> a owl:Class,
        linkml:ClassDefinition ;
    rdfs:label "TobaccoExposureObservation" ;
    rdfs:subClassOf [ a owl:Restriction ;
            owl:maxQualifiedCardinality 1 ;
            owl:onClass <http://UNKNOWN.org/enum_CRDCH_TobaccoExposureObservation_category> ;
            owl:onProperty linkml:category ],
        [ a owl:Restriction ;
            owl:maxQualifiedCardinality 1 ;
            owl:onClass <https://example.org/crdch_model/Organization> ;
            owl:onProperty linkml:performed_by ],
        [ a owl:Restriction ;
            owl:maxQualifiedCardinality 1 ;
            owl:onClass <https://example.org/crdch_model/Subject> ;
            owl:onProperty linkml:subject ],
        [ a owl:Restriction ;
            owl:maxQualifiedCardinality 1 ;
            owl:onClass <http://UNKNOWN.org/enum_CRDCH_TobaccoExposureObservation_method_type> ;
            owl:onProperty linkml:method_type ],
        [ a owl:Restriction ;
            owl:maxQualifiedCardinality 1 ;
            owl:onClass <https://example.org/crdch_model/Entity> ;
            owl:onProperty linkml:valueInteger ],
        [ a owl:Restriction ;
            owl:maxQualifiedCardinality 1 ;
            owl:onClass <https://example.org/crdch_model/Entity> ;
            owl:onProperty linkml:id ],
        [ a owl:Restriction ;
            owl:onClass <http://UNKNOWN.org/enum_CRDCH_TobaccoExposureObservation_observation_type> ;
            owl:onProperty linkml:observation_type ;
            owl:qualifiedCardinality 1 ],
        [ a owl:Restriction ;
            owl:maxQualifiedCardinality 1 ;
            owl:onClass <https://example.org/crdch_model/Entity> ;
            owl:onProperty linkml:focus ],
        [ a owl:Restriction ;
            owl:maxQualifiedCardinality 1 ;
            owl:onClass <http://UNKNOWN.org/enum_CRDCH_TobaccoExposureObservation_valueCodeableConcept> ;
            owl:onProperty linkml:valueCodeableConcept ],
        <https://example.org/crdch_model/Entity> ;
    skos:definition "A structured object that describes a single data item about an individual's exposure to tobacco, as generated through a point-in-time observation, measurement, or interpretation." ;
    skos:editorialNote "Derived from [TobaccoExposureObservation in sheet TobaccoExposureObservation](https://docs.google.com/spreadsheets/d/1oWS7cao-fgz2MKWtyr8h2dEL9unX__0bJrWKv6mQmM4/edit#gid=1464668175)" .

<https://example.org/crdch_model/ExecutionTimeObservation> a owl:Class,
        linkml:ClassDefinition ;
    rdfs:label "ExecutionTimeObservation" ;
    rdfs:subClassOf [ a owl:Restriction ;
            owl:maxQualifiedCardinality 1 ;
            owl:onClass <https://example.org/crdch_model/Organization> ;
            owl:onProperty linkml:performed_by ],
        [ a owl:Restriction ;
            owl:maxQualifiedCardinality 1 ;
            owl:onClass <http://UNKNOWN.org/enum_CRDCH_ExecutionTimeObservation_category> ;
            owl:onProperty linkml:category ],
        [ a owl:Restriction ;
            owl:maxQualifiedCardinality 1 ;
            owl:onClass <http://UNKNOWN.org/enum_CRDCH_ExecutionTimeObservation_method_type> ;
            owl:onProperty linkml:method_type ],
        [ a owl:Restriction ;
            owl:maxQualifiedCardinality 1 ;
            owl:onClass <https://example.org/crdch_model/Entity> ;
            owl:onProperty linkml:id ],
        [ a owl:Restriction ;
            owl:maxQualifiedCardinality 1 ;
            owl:onClass <https://example.org/crdch_model/Entity> ;
            owl:onProperty linkml:focus ],
        [ a owl:Restriction ;
            owl:maxQualifiedCardinality 1 ;
            owl:onClass <https://example.org/crdch_model/Subject> ;
            owl:onProperty linkml:subject ],
        [ a owl:Restriction ;
            owl:onClass <https://example.org/crdch_model/Quantity> ;
            owl:onProperty linkml:valueQuantity ;
            owl:qualifiedCardinality 1 ],
        [ a owl:Restriction ;
            owl:onClass <http://UNKNOWN.org/enum_CRDCH_ExecutionTimeObservation_observation_type> ;
            owl:onProperty linkml:observation_type ;
            owl:qualifiedCardinality 1 ],
        <https://example.org/crdch_model/Entity> ;
    skos:definition """A structured object that describes how long certain parts on an activity took to complete, as determined through a point-in-time observation or measurement.

Information describing the environmental conditions in which an activity, or a specific part of an activity, was performed.""" ;
    skos:editorialNote "Derived from [ExecutionTimeObservation in sheet ExecutionTimeObservation](https://docs.google.com/spreadsheets/d/1oWS7cao-fgz2MKWtyr8h2dEL9unX__0bJrWKv6mQmM4/edit#gid=638866265)" .

<https://example.org/crdch_model/ResearchSubject> a owl:Class,
        linkml:ClassDefinition ;
    rdfs:label "ResearchSubject" ;
    rdfs:subClassOf [ a owl:Restriction ;
            owl:maxQualifiedCardinality 1 ;
            owl:onClass <https://example.org/crdch_model/Quantity> ;
            owl:onProperty linkml:age_at_enrollment ],
        [ a owl:Restriction ;
            owl:maxQualifiedCardinality 1 ;
            owl:onClass <https://example.org/crdch_model/BodySite> ;
            owl:onProperty linkml:primary_diagnosis_site ],
        [ a owl:Restriction ;
            owl:maxQualifiedCardinality 1 ;
            owl:onClass <http://UNKNOWN.org/enum_CRDCH_ResearchSubject_index_timepoint> ;
            owl:onProperty linkml:index_timepoint ],
        [ a owl:Restriction ;
            owl:onClass <https://example.org/crdch_model/Subject> ;
            owl:onProperty linkml:associated_subject ;
            owl:qualifiedCardinality 1 ],
        [ a owl:Restriction ;
            owl:onClass <https://example.org/crdch_model/Entity> ;
            owl:onProperty linkml:id ;
            owl:qualifiedCardinality 1 ],
        [ a owl:Restriction ;
            owl:maxQualifiedCardinality 1 ;
            owl:onClass <https://example.org/crdch_model/ResearchProject> ;
            owl:onProperty linkml:member_of_research_project ],
        [ a owl:Restriction ;
            owl:maxQualifiedCardinality 1 ;
            owl:onClass <https://example.org/crdch_model/Organization> ;
            owl:onProperty linkml:originating_site ],
        [ a owl:Restriction ;
            owl:maxQualifiedCardinality 1 ;
            owl:onClass <http://UNKNOWN.org/enum_CRDCH_ResearchSubject_primary_diagnosis_condition> ;
            owl:onProperty linkml:primary_diagnosis_condition ],
        [ a owl:Restriction ;
            owl:allValuesFrom <https://example.org/crdch_model/Identifier> ;
            owl:onProperty linkml:identifier ],
        [ a owl:Restriction ;
            owl:maxQualifiedCardinality 1 ;
            owl:onClass <https://example.org/crdch_model/Entity> ;
            owl:onProperty linkml:description ],
        [ a owl:Restriction ;
            owl:allValuesFrom <https://example.org/crdch_model/Diagnosis> ;
            owl:onProperty linkml:comorbid_diagnosis ],
        [ a owl:Restriction ;
            owl:allValuesFrom <https://example.org/crdch_model/Diagnosis> ;
            owl:onProperty linkml:primary_diagnosis ],
        <https://example.org/crdch_model/Entity> ;
    skos:definition """A research subject is the entity of interest in a research study, typically a human being or an animal, but can also be a device, group of humans or animals, 
or a tissue sample. Human research subjects are usually not traceable to a particular person to protect the subject’s privacy.""" ;
    skos:editorialNote "Derived from [ResearchSubject in sheet ResearchSubject](https://docs.google.com/spreadsheets/d/1oWS7cao-fgz2MKWtyr8h2dEL9unX__0bJrWKv6mQmM4/edit#gid=665511119)" .

<https://example.org/crdch_model/SpecimenContainer> a owl:Class,
        linkml:ClassDefinition ;
    rdfs:label "SpecimenContainer" ;
    rdfs:subClassOf [ a owl:Restriction ;
            owl:allValuesFrom <https://example.org/crdch_model/Substance> ;
            owl:onProperty linkml:additive ],
        [ a owl:Restriction ;
            owl:maxQualifiedCardinality 1 ;
            owl:onClass <http://UNKNOWN.org/enum_CRDCH_SpecimenContainer_container_type> ;
            owl:onProperty linkml:container_type ],
        [ a owl:Restriction ;
            owl:allValuesFrom <https://example.org/crdch_model/Identifier> ;
            owl:onProperty linkml:identifier ],
        [ a owl:Restriction ;
            owl:maxQualifiedCardinality 1 ;
            owl:onClass <https://example.org/crdch_model/Entity> ;
            owl:onProperty linkml:container_number ],
        [ a owl:Restriction ;
            owl:maxQualifiedCardinality 1 ;
            owl:onClass <https://example.org/crdch_model/Entity> ;
            owl:onProperty linkml:id ],
        [ a owl:Restriction ;
            owl:maxQualifiedCardinality 1 ;
            owl:onClass <https://example.org/crdch_model/SpecimenContainer> ;
            owl:onProperty linkml:parent_container ],
        <https://example.org/crdch_model/Entity> ;
    skos:definition "A vessel in which a specimen is held or to which it is attached - for storage or as a substrate for growth (e.g. a cell culture dish) or analysis (e.g. a microscope slide or 96-well plate)" ;
    skos:editorialNote "Derived from [SpecimenContainer in sheet SpecimenContainer](https://docs.google.com/spreadsheets/d/1oWS7cao-fgz2MKWtyr8h2dEL9unX__0bJrWKv6mQmM4/edit#gid=729222697)" .

<https://example.org/crdch_model/BodySite> a owl:Class,
        linkml:ClassDefinition ;
    rdfs:label "BodySite" ;
    rdfs:subClassOf [ a owl:Restriction ;
            owl:onClass <http://UNKNOWN.org/enum_CRDCH_BodySite_site> ;
            owl:onProperty linkml:site ;
            owl:qualifiedCardinality 1 ],
        [ a owl:Restriction ;
            owl:allValuesFrom <http://UNKNOWN.org/enum_CRDCH_BodySite_qualifier> ;
            owl:onProperty linkml:qualifier ],
        <https://example.org/crdch_model/Entity> ;
    skos:definition "A site in the body of an organism, typically described in terms of an anatomical location and optional qualifiers (e.g. left/right, upper/lower). But body sites as defined here may include 'non-anatomic' sites, such as the location of an implanted medical device." ;
    skos:editorialNote "Derived from [BodySite in sheet BodySite](https://docs.google.com/spreadsheets/d/1oWS7cao-fgz2MKWtyr8h2dEL9unX__0bJrWKv6mQmM4/edit#gid=1097478901)" .

<https://example.org/crdch_model/ExecutionConditionObservation> a owl:Class,
        linkml:ClassDefinition ;
    rdfs:label "ExecutionConditionObservation" ;
    rdfs:subClassOf [ a owl:Restriction ;
            owl:maxQualifiedCardinality 1 ;
            owl:onClass <https://example.org/crdch_model/Entity> ;
            owl:onProperty linkml:id ],
        [ a owl:Restriction ;
            owl:maxQualifiedCardinality 1 ;
            owl:onClass <https://example.org/crdch_model/Subject> ;
            owl:onProperty linkml:subject ],
        [ a owl:Restriction ;
            owl:maxQualifiedCardinality 1 ;
            owl:onClass <https://example.org/crdch_model/Entity> ;
            owl:onProperty linkml:focus ],
        [ a owl:Restriction ;
            owl:onClass <http://UNKNOWN.org/enum_CRDCH_ExecutionConditionObservation_valueCodeableConcept> ;
            owl:onProperty linkml:valueCodeableConcept ;
            owl:qualifiedCardinality 1 ],
        [ a owl:Restriction ;
            owl:maxQualifiedCardinality 1 ;
            owl:onClass <https://example.org/crdch_model/Organization> ;
            owl:onProperty linkml:performed_by ],
        [ a owl:Restriction ;
            owl:maxQualifiedCardinality 1 ;
            owl:onClass <http://UNKNOWN.org/enum_CRDCH_ExecutionConditionObservation_category> ;
            owl:onProperty linkml:category ],
        [ a owl:Restriction ;
            owl:maxQualifiedCardinality 1 ;
            owl:onClass <http://UNKNOWN.org/enum_CRDCH_ExecutionConditionObservation_method_type> ;
            owl:onProperty linkml:method_type ],
        [ a owl:Restriction ;
            owl:onClass <http://UNKNOWN.org/enum_CRDCH_ExecutionConditionObservation_observation_type> ;
            owl:onProperty linkml:observation_type ;
            owl:qualifiedCardinality 1 ],
        <https://example.org/crdch_model/Entity> ;
    skos:definition """A structured object that describes how long certain parts on an activity took to complete, as determined through a point-in-time observation or measurement.

Information describing the environmental conditions in which an activity, or a specific part of an activity, was performed.""" ;
    skos:editorialNote "Derived from [ExecutionConditionObservation in sheet ExecutionConditionObservation](https://docs.google.com/spreadsheets/d/1oWS7cao-fgz2MKWtyr8h2dEL9unX__0bJrWKv6mQmM4/edit#gid=1598634433)" .

<https://example.org/crdch_model/SpecimenCreationActivity> a owl:Class,
        linkml:ClassDefinition ;
    rdfs:label "SpecimenCreationActivity" ;
    rdfs:subClassOf [ a owl:Restriction ;
            owl:maxQualifiedCardinality 1 ;
            owl:onClass <https://example.org/crdch_model/Organization> ;
            owl:onProperty linkml:performed_by ],
        [ a owl:Restriction ;
            owl:maxQualifiedCardinality 1 ;
            owl:onClass <http://UNKNOWN.org/enum_CRDCH_SpecimenCreationActivity_derivation_method_type> ;
            owl:onProperty linkml:derivation_method_type ],
        [ a owl:Restriction ;
            owl:maxQualifiedCardinality 1 ;
            owl:onClass <https://example.org/crdch_model/TimePoint> ;
            owl:onProperty linkml:date_started ],
        [ a owl:Restriction ;
            owl:maxQualifiedCardinality 1 ;
            owl:onClass <http://UNKNOWN.org/enum_CRDCH_SpecimenCreationActivity_collection_method_type> ;
            owl:onProperty linkml:collection_method_type ],
        [ a owl:Restriction ;
            owl:maxQualifiedCardinality 1 ;
            owl:onClass <https://example.org/crdch_model/Entity> ;
            owl:onProperty linkml:specimen_order ],
        [ a owl:Restriction ;
            owl:maxQualifiedCardinality 1 ;
            owl:onClass <https://example.org/crdch_model/TimePoint> ;
            owl:onProperty linkml:date_ended ],
        [ a owl:Restriction ;
            owl:maxQualifiedCardinality 1 ;
            owl:onClass <http://UNKNOWN.org/enum_CRDCH_SpecimenCreationActivity_activity_type> ;
            owl:onProperty linkml:activity_type ],
        [ a owl:Restriction ;
            owl:maxQualifiedCardinality 1 ;
            owl:onClass <https://example.org/crdch_model/Quantity> ;
            owl:onProperty linkml:quantity_collected ],
        [ a owl:Restriction ;
            owl:allValuesFrom <https://example.org/crdch_model/ExecutionConditionObservation> ;
            owl:onProperty linkml:execution_condition_observation ],
        [ a owl:Restriction ;
            owl:allValuesFrom <https://example.org/crdch_model/Substance> ;
            owl:onProperty linkml:additive ],
        [ a owl:Restriction ;
            owl:maxQualifiedCardinality 1 ;
            owl:onClass <https://example.org/crdch_model/BodySite> ;
            owl:onProperty linkml:collection_site ],
        [ a owl:Restriction ;
            owl:allValuesFrom <https://example.org/crdch_model/ExecutionTimeObservation> ;
            owl:onProperty linkml:execution_time_observation ],
        <https://example.org/crdch_model/Entity> ;
    skos:definition "The process of creating a specimen. This may occur through observing and/or collecting material from an biological source or natural setting, or through derivation from an existing specimen (e.g. via portioning or aliquoting)." ;
    skos:editorialNote "Derived from [SpecimenCreationActivity in sheet SpecimenCreationActivity](https://docs.google.com/spreadsheets/d/1oWS7cao-fgz2MKWtyr8h2dEL9unX__0bJrWKv6mQmM4/edit#gid=693792130)" ;
    skos:note "A creation' activity represents the entire process up to the point where the specimen is physically modified, stored, or transported." .

linkml:topValue a owl:DatatypeProperty ;
    rdfs:label "value" .

<https://example.org/crdch_model/Observation> a owl:Class,
        linkml:ClassDefinition ;
    rdfs:label "Observation" ;
    rdfs:subClassOf [ a owl:Restriction ;
            owl:maxQualifiedCardinality 1 ;
            owl:onClass <http://UNKNOWN.org/enum_CRDCH_Observation_valueCodeableConcept> ;
            owl:onProperty linkml:valueCodeableConcept ],
        [ a owl:Restriction ;
            owl:maxQualifiedCardinality 1 ;
            owl:onClass <https://example.org/crdch_model/Entity> ;
            owl:onProperty linkml:valueInteger ],
        [ a owl:Restriction ;
            owl:maxQualifiedCardinality 1 ;
            owl:onClass <https://example.org/crdch_model/Entity> ;
            owl:onProperty linkml:valueDecimal ],
        [ a owl:Restriction ;
            owl:maxQualifiedCardinality 1 ;
            owl:onClass <https://example.org/crdch_model/Entity> ;
            owl:onProperty linkml:valueString ],
        [ a owl:Restriction ;
            owl:maxQualifiedCardinality 1 ;
            owl:onClass <https://example.org/crdch_model/Entity> ;
            owl:onProperty linkml:valueEntity ],
        [ a owl:Restriction ;
            owl:maxQualifiedCardinality 1 ;
            owl:onClass <https://example.org/crdch_model/Organization> ;
            owl:onProperty linkml:performed_by ],
        [ a owl:Restriction ;
            owl:allValuesFrom <http://UNKNOWN.org/enum_CRDCH_Observation_method_type> ;
            owl:onProperty linkml:method_type ],
        [ a owl:Restriction ;
            owl:allValuesFrom <https://example.org/crdch_model/Entity> ;
            owl:onProperty linkml:focus ],
        [ a owl:Restriction ;
            owl:maxQualifiedCardinality 1 ;
            owl:onClass <https://example.org/crdch_model/Entity> ;
            owl:onProperty linkml:valueBoolean ],
        [ a owl:Restriction ;
            owl:maxQualifiedCardinality 1 ;
            owl:onClass <https://example.org/crdch_model/Entity> ;
            owl:onProperty linkml:valueDateTime ],
        [ a owl:Restriction ;
            owl:maxQualifiedCardinality 1 ;
            owl:onClass <http://UNKNOWN.org/enum_CRDCH_Observation_category> ;
            owl:onProperty linkml:category ],
        [ a owl:Restriction ;
            owl:maxQualifiedCardinality 1 ;
            owl:onClass <https://example.org/crdch_model/Quantity> ;
            owl:onProperty linkml:valueQuantity ],
        [ a owl:Restriction ;
            owl:onClass <http://UNKNOWN.org/enum_CRDCH_Observation_observation_type> ;
            owl:onProperty linkml:observation_type ;
            owl:qualifiedCardinality 1 ],
        [ a owl:Restriction ;
            owl:maxQualifiedCardinality 1 ;
            owl:onClass <https://example.org/crdch_model/Entity> ;
            owl:onProperty linkml:id ],
        [ a owl:Restriction ;
            owl:maxQualifiedCardinality 1 ;
            owl:onClass <https://example.org/crdch_model/Subject> ;
            owl:onProperty linkml:subject ],
        <https://example.org/crdch_model/Entity> ;
    skos:definition "A structured object that describes a single data item about an entity, as generated through a point-in-time observation, measurement, or interpretation." ;
    skos:editorialNote "Derived from [Observation in sheet Observation](https://docs.google.com/spreadsheets/d/1oWS7cao-fgz2MKWtyr8h2dEL9unX__0bJrWKv6mQmM4/edit#gid=550424063)" ;
    skos:note "At the core of an Observation is a flexible key-value pair (or a structured collection of key-value pairs), where a 'key' field defines the type of observation made, and the 'value' field describes the value or outcome of the observation. The fact that the type of observation captured is defined in the data allow Observation to convey a broad range of observation data." .

<https://example.org/crdch_model/Treatment> a owl:Class,
        linkml:ClassDefinition ;
    rdfs:label "Treatment" ;
    rdfs:subClassOf [ a owl:Restriction ;
            owl:maxQualifiedCardinality 1 ;
            owl:onClass <http://UNKNOWN.org/enum_CRDCH_Treatment_treatment_frequency> ;
            owl:onProperty linkml:treatment_frequency ],
        [ a owl:Restriction ;
            owl:maxQualifiedCardinality 1 ;
            owl:onClass <https://example.org/crdch_model/BodySite> ;
            owl:onProperty linkml:treatment_anatomic_site ],
        [ a owl:Restriction ;
            owl:allValuesFrom <https://example.org/crdch_model/Identifier> ;
            owl:onProperty linkml:identifier ],
        [ a owl:Restriction ;
            owl:maxQualifiedCardinality 1 ;
            owl:onClass <http://UNKNOWN.org/enum_CRDCH_Treatment_treatment_intent> ;
            owl:onProperty linkml:treatment_intent ],
        [ a owl:Restriction ;
            owl:allValuesFrom <https://example.org/crdch_model/Diagnosis> ;
            owl:onProperty linkml:treatment_for_diagnosis ],
        [ a owl:Restriction ;
            owl:maxQualifiedCardinality 1 ;
            owl:onClass <https://example.org/crdch_model/TimePoint> ;
            owl:onProperty linkml:date_started ],
        [ a owl:Restriction ;
            owl:maxQualifiedCardinality 1 ;
            owl:onClass <https://example.org/crdch_model/Subject> ;
            owl:onProperty linkml:subject ],
        [ a owl:Restriction ;
            owl:allValuesFrom <https://example.org/crdch_model/Treatment> ;
            owl:onProperty linkml:concurrent_treatment ],
        [ a owl:Restriction ;
            owl:maxQualifiedCardinality 1 ;
            owl:onClass <https://example.org/crdch_model/Entity> ;
            owl:onProperty linkml:number_of_cycles ],
        [ a owl:Restriction ;
            owl:maxQualifiedCardinality 1 ;
            owl:onClass <https://example.org/crdch_model/TimePoint> ;
            owl:onProperty linkml:date_ended ],
        [ a owl:Restriction ;
            owl:allValuesFrom <http://UNKNOWN.org/enum_CRDCH_Treatment_treatment_end_reason> ;
            owl:onProperty linkml:treatment_end_reason ],
        [ a owl:Restriction ;
            owl:maxQualifiedCardinality 1 ;
            owl:onClass <http://UNKNOWN.org/enum_CRDCH_Treatment_treatment_effect> ;
            owl:onProperty linkml:treatment_effect ],
        [ a owl:Restriction ;
            owl:maxQualifiedCardinality 1 ;
            owl:onClass <https://example.org/crdch_model/Substance> ;
            owl:onProperty linkml:therapeutic_agent ],
        [ a owl:Restriction ;
            owl:maxQualifiedCardinality 1 ;
            owl:onClass <http://UNKNOWN.org/enum_CRDCH_Treatment_regimen> ;
            owl:onProperty linkml:regimen ],
        [ a owl:Restriction ;
            owl:maxQualifiedCardinality 1 ;
            owl:onClass <http://UNKNOWN.org/enum_CRDCH_Treatment_treatment_type> ;
            owl:onProperty linkml:treatment_type ],
        [ a owl:Restriction ;
            owl:maxQualifiedCardinality 1 ;
            owl:onClass <http://UNKNOWN.org/enum_CRDCH_Treatment_treatment_outcome> ;
            owl:onProperty linkml:treatment_outcome ],
        [ a owl:Restriction ;
            owl:maxQualifiedCardinality 1 ;
            owl:onClass <https://example.org/crdch_model/Entity> ;
            owl:onProperty linkml:id ],
        <https://example.org/crdch_model/Entity> ;
    skos:definition "Represent medication administration or other treatment types." ;
    skos:editorialNote "Derived from [Treatment in sheet Treatment](https://docs.google.com/spreadsheets/d/1oWS7cao-fgz2MKWtyr8h2dEL9unX__0bJrWKv6mQmM4/edit#gid=2111784779)" ;
    skos:note "This entity is overloaded with the idea of medication/substance based treatments, and other more procedure-like interventions that are also considered to be a treatment. We should probably separate these concerns and it will be useful to have a \"Procedure\" entity long term. If that is done, this entity will be renamed to \"MedicationTreatment\" or something like that and the other concerns refactored out to other entities. Also, if we can consider a medication/substance based treatment as a procedure as well (which is commonly the case in other models), we can make this entity more about the individual doses for such treatments if that level of granularity is needed." .

<https://example.org/crdch_model/ResearchProject> a owl:Class,
        linkml:ClassDefinition ;
    rdfs:label "ResearchProject" ;
    rdfs:subClassOf [ a owl:Restriction ;
            owl:allValuesFrom <https://example.org/crdch_model/TimePoint> ;
            owl:onProperty linkml:associated_timepoint ],
        [ a owl:Restriction ;
            owl:allValuesFrom <https://example.org/crdch_model/Entity> ;
            owl:onProperty linkml:url ],
        [ a owl:Restriction ;
            owl:allValuesFrom <https://example.org/crdch_model/Identifier> ;
            owl:onProperty linkml:identifier ],
        [ a owl:Restriction ;
            owl:onClass <http://UNKNOWN.org/enum_CRDCH_ResearchProject_research_project_type> ;
            owl:onProperty linkml:research_project_type ;
            owl:qualifiedCardinality 1 ],
        [ a owl:Restriction ;
            owl:maxQualifiedCardinality 1 ;
            owl:onClass <https://example.org/crdch_model/Entity> ;
            owl:onProperty linkml:description_shortened ],
        [ a owl:Restriction ;
            owl:maxQualifiedCardinality 1 ;
            owl:onClass <https://example.org/crdch_model/TimePoint> ;
            owl:onProperty linkml:date_started ],
        [ a owl:Restriction ;
            owl:allValuesFrom <https://example.org/crdch_model/BodySite> ;
            owl:onProperty linkml:primary_anatomic_site ],
        [ a owl:Restriction ;
            owl:maxQualifiedCardinality 1 ;
            owl:onClass <https://example.org/crdch_model/Entity> ;
            owl:onProperty linkml:name_shortened ],
        [ a owl:Restriction ;
            owl:maxQualifiedCardinality 1 ;
            owl:onClass <https://example.org/crdch_model/Entity> ;
            owl:onProperty linkml:id ],
        [ a owl:Restriction ;
            owl:maxQualifiedCardinality 1 ;
            owl:onClass <https://example.org/crdch_model/Entity> ;
            owl:onProperty linkml:name ],
        [ a owl:Restriction ;
            owl:allValuesFrom <https://example.org/crdch_model/ResearchProject> ;
            owl:onProperty linkml:part_of ],
        [ a owl:Restriction ;
            owl:maxQualifiedCardinality 1 ;
            owl:onClass <https://example.org/crdch_model/Entity> ;
            owl:onProperty linkml:description ],
        [ a owl:Restriction ;
            owl:maxQualifiedCardinality 1 ;
            owl:onClass <https://example.org/crdch_model/TimePoint> ;
            owl:onProperty linkml:date_ended ],
        [ a owl:Restriction ;
            owl:allValuesFrom <https://example.org/crdch_model/Entity> ;
            owl:onProperty linkml:sponsor ],
        <https://example.org/crdch_model/Entity> ;
    skos:definition """A process where a researcher or organization plans and then executes a series of steps intended to increase the field of healthcare-related knowledge. 
This includes studies of safety, efficacy, comparative effectiveness and other information about medications, devices, therapies and other interventional 
and investigative techniques. A ResearchProject involves the gathering of information about human or animal subjects.""" ;
    skos:editorialNote "Derived from [ResearchProject in sheet ResearchProject](https://docs.google.com/spreadsheets/d/1oWS7cao-fgz2MKWtyr8h2dEL9unX__0bJrWKv6mQmM4/edit#gid=1123416579)" .

linkml:TypeDefinition a owl:Class ;
    rdfs:label "type_definition" ;
    skos:definition "A data type definition." .

<https://example.org/crdch_model/Diagnosis> a owl:Class,
        linkml:ClassDefinition ;
    rdfs:label "Diagnosis" ;
    rdfs:subClassOf [ a owl:Restriction ;
            owl:maxQualifiedCardinality 1 ;
            owl:onClass <https://example.org/crdch_model/Entity> ;
            owl:onProperty linkml:year_at_diagnosis ],
        [ a owl:Restriction ;
            owl:allValuesFrom <https://example.org/crdch_model/BodySite> ;
            owl:onProperty linkml:primary_site ],
        [ a owl:Restriction ;
            owl:maxQualifiedCardinality 1 ;
            owl:onClass <https://example.org/crdch_model/Diagnosis> ;
            owl:onProperty linkml:prior_diagnosis ],
        [ a owl:Restriction ;
            owl:allValuesFrom <https://example.org/crdch_model/CancerStageObservationSet> ;
            owl:onProperty linkml:stage ],
        [ a owl:Restriction ;
            owl:allValuesFrom <https://example.org/crdch_model/Observation> ;
            owl:onProperty linkml:supporting_observation ],
        [ a owl:Restriction ;
            owl:maxQualifiedCardinality 1 ;
            owl:onClass <https://example.org/crdch_model/Entity> ;
            owl:onProperty linkml:id ],
        [ a owl:Restriction ;
            owl:maxQualifiedCardinality 1 ;
            owl:onClass <https://example.org/crdch_model/Subject> ;
            owl:onProperty linkml:subject ],
        [ a owl:Restriction ;
            owl:allValuesFrom <https://example.org/crdch_model/CancerGradeObservationSet> ;
            owl:onProperty linkml:grade ],
        [ a owl:Restriction ;
            owl:maxQualifiedCardinality 1 ;
            owl:onClass <http://UNKNOWN.org/enum_CRDCH_Diagnosis_disease_status> ;
            owl:onProperty linkml:disease_status ],
        [ a owl:Restriction ;
            owl:allValuesFrom <https://example.org/crdch_model/BodySite> ;
            owl:onProperty linkml:metastatic_site ],
        [ a owl:Restriction ;
            owl:maxQualifiedCardinality 1 ;
            owl:onClass <https://example.org/crdch_model/Quantity> ;
            owl:onProperty linkml:age_at_diagnosis ],
        [ a owl:Restriction ;
            owl:allValuesFrom <https://example.org/crdch_model/Identifier> ;
            owl:onProperty linkml:identifier ],
        [ a owl:Restriction ;
            owl:maxQualifiedCardinality 1 ;
            owl:onClass <https://example.org/crdch_model/DimensionalObservationSet> ;
            owl:onProperty linkml:primary_tumor_dimensional_measures ],
        [ a owl:Restriction ;
            owl:maxQualifiedCardinality 1 ;
            owl:onClass <http://UNKNOWN.org/enum_CRDCH_Diagnosis_condition> ;
            owl:onProperty linkml:condition ],
        [ a owl:Restriction ;
            owl:maxQualifiedCardinality 1 ;
            owl:onClass <http://UNKNOWN.org/enum_CRDCH_Diagnosis_morphology> ;
            owl:onProperty linkml:morphology ],
        [ a owl:Restriction ;
            owl:allValuesFrom <https://example.org/crdch_model/Specimen> ;
            owl:onProperty linkml:related_specimen ],
        [ a owl:Restriction ;
            owl:maxQualifiedCardinality 1 ;
            owl:onClass <http://UNKNOWN.org/enum_CRDCH_Diagnosis_method_of_diagnosis> ;
            owl:onProperty linkml:method_of_diagnosis ],
        <https://example.org/crdch_model/Entity> ;
    skos:definition "A collection of characteristics that describe an abnormal condition of the body as assessed at a point in time. May be used to capture information about neoplastic and non-neoplastic conditions." ;
    skos:editorialNote "Derived from [Diagnosis in sheet Diagnosis](https://docs.google.com/spreadsheets/d/1oWS7cao-fgz2MKWtyr8h2dEL9unX__0bJrWKv6mQmM4/edit#gid=1015759209)" .

<https://example.org/crdch_model/Identifier> a owl:Class,
        linkml:ClassDefinition ;
    rdfs:label "Identifier" ;
    rdfs:subClassOf [ a owl:Restriction ;
            owl:maxQualifiedCardinality 1 ;
            owl:onClass <https://example.org/crdch_model/Entity> ;
            owl:onProperty linkml:system ],
        [ a owl:Restriction ;
            owl:maxQualifiedCardinality 1 ;
            owl:onClass <http://UNKNOWN.org/enum_CRDCH_Identifier_type> ;
            owl:onProperty linkml:type ],
        [ a owl:Restriction ;
            owl:onClass <https://example.org/crdch_model/Entity> ;
            owl:onProperty linkml:value ;
            owl:qualifiedCardinality 1 ],
        <https://example.org/crdch_model/Entity> ;
    skos:definition "An Identifier is associated with a unique object or entity within a given system." ;
    skos:editorialNote "Derived from [Identifier in sheet Identifier](https://docs.google.com/spreadsheets/d/1oWS7cao-fgz2MKWtyr8h2dEL9unX__0bJrWKv6mQmM4/edit#gid=1307792462)" ;
    skos:note "This data type is intended to be used to represent business identifiers that are shared between systems." .

<https://example.org/crdch_model/Quantity> a owl:Class,
        linkml:ClassDefinition ;
    rdfs:label "Quantity" ;
    rdfs:subClassOf [ a owl:Restriction ;
            owl:maxQualifiedCardinality 1 ;
            owl:onClass <https://example.org/crdch_model/Entity> ;
            owl:onProperty linkml:valueDecimal ],
        [ a owl:Restriction ;
            owl:maxQualifiedCardinality 1 ;
            owl:onClass <http://UNKNOWN.org/enum_CRDCH_Quantity_unit> ;
            owl:onProperty linkml:unit ],
        [ a owl:Restriction ;
            owl:maxQualifiedCardinality 1 ;
            owl:onClass <http://UNKNOWN.org/enum_CRDCH_Quantity_valueCodeableConcept> ;
            owl:onProperty linkml:valueCodeableConcept ],
        <https://example.org/crdch_model/Entity> ;
    skos:definition "A structured object to represent an amount of something (e.g., weight, mass, length, duration of time) - including a value and unit." ;
    skos:editorialNote "Derived from [Quantity in sheet Quantity](https://docs.google.com/spreadsheets/d/1oWS7cao-fgz2MKWtyr8h2dEL9unX__0bJrWKv6mQmM4/edit#gid=1941950611)" ;
    skos:note "QuantityMeasure' may be implemented as an Observation-like object that will let us capture any type of measure of the amount of some substance (e.g. weight, volume, maybe even concentration?), with distinct timestamps and methods associated.  It could be implemented as a \"simple\" observation (one measurement per instance, where the 'code' fields is bound to a value set describing the different types of quantity measures allowed -  e.g. 'weight', 'volume', 'concentration'),  or as \"composite\" observation (multiple measurements possible in a single instance, each captured as a component defined to hold a specific type of quantity measure - e.g.  'weight', 'volume', 'concentration').  The number of different quantity measures we anticipate needed to support, and the potential for data sparseness, are factors that determine whether a simple or composite Observation would be most appropriate." .

<https://example.org/crdch_model/Specimen> a owl:Class,
        linkml:ClassDefinition ;
    rdfs:label "Specimen" ;
    rdfs:subClassOf [ a owl:Restriction ;
            owl:allValuesFrom <https://example.org/crdch_model/SpecimenProcessingActivity> ;
            owl:onProperty linkml:processing_activity ],
        [ a owl:Restriction ;
            owl:maxQualifiedCardinality 1 ;
            owl:onClass <http://UNKNOWN.org/enum_CRDCH_Specimen_morphology_assessment_method> ;
            owl:onProperty linkml:morphology_assessment_method ],
        [ a owl:Restriction ;
            owl:maxQualifiedCardinality 1 ;
            owl:onClass <http://UNKNOWN.org/enum_CRDCH_Specimen_analyte_type> ;
            owl:onProperty linkml:analyte_type ],
        [ a owl:Restriction ;
            owl:allValuesFrom <https://example.org/crdch_model/HistologicalCompositionObservationSet> ;
            owl:onProperty linkml:histological_composition_measures ],
        [ a owl:Restriction ;
            owl:maxQualifiedCardinality 1 ;
            owl:onClass <https://example.org/crdch_model/Entity> ;
            owl:onProperty linkml:id ],
        [ a owl:Restriction ;
            owl:maxQualifiedCardinality 1 ;
            owl:onClass <http://UNKNOWN.org/enum_CRDCH_Specimen_source_material_type> ;
            owl:onProperty linkml:source_material_type ],
        [ a owl:Restriction ;
            owl:allValuesFrom <https://example.org/crdch_model/Identifier> ;
            owl:onProperty linkml:identifier ],
        [ a owl:Restriction ;
            owl:allValuesFrom <https://example.org/crdch_model/SpecimenTransportActivity> ;
            owl:onProperty linkml:transport_activity ],
        [ a owl:Restriction ;
            owl:maxQualifiedCardinality 1 ;
            owl:onClass <http://UNKNOWN.org/enum_CRDCH_Specimen_specific_tissue_morphology> ;
            owl:onProperty linkml:specific_tissue_morphology ],
        [ a owl:Restriction ;
            owl:maxQualifiedCardinality 1 ;
            owl:onClass <https://example.org/crdch_model/Organization> ;
            owl:onProperty linkml:data_provider ],
        [ a owl:Restriction ;
            owl:maxQualifiedCardinality 1 ;
            owl:onClass <https://example.org/crdch_model/Entity> ;
            owl:onProperty linkml:dysplasia_fraction ],
        [ a owl:Restriction ;
            owl:maxQualifiedCardinality 1 ;
            owl:onClass <http://UNKNOWN.org/enum_CRDCH_Specimen_general_tissue_morphology> ;
            owl:onProperty linkml:general_tissue_morphology ],
        [ a owl:Restriction ;
            owl:maxQualifiedCardinality 1 ;
            owl:onClass <http://UNKNOWN.org/enum_CRDCH_Specimen_degree_of_dysplasia> ;
            owl:onProperty linkml:degree_of_dysplasia ],
        [ a owl:Restriction ;
            owl:maxQualifiedCardinality 1 ;
            owl:onClass <https://example.org/crdch_model/DimensionalObservationSet> ;
            owl:onProperty linkml:dimensional_measures ],
        [ a owl:Restriction ;
            owl:allValuesFrom <https://example.org/crdch_model/SpecimenQualityObservation> ;
            owl:onProperty linkml:quality_measure ],
        [ a owl:Restriction ;
            owl:maxQualifiedCardinality 1 ;
            owl:onClass <http://UNKNOWN.org/enum_CRDCH_Specimen_section_location> ;
            owl:onProperty linkml:section_location ],
        [ a owl:Restriction ;
            owl:allValuesFrom <https://example.org/crdch_model/SpecimenStorageActivity> ;
            owl:onProperty linkml:storage_activity ],
        [ a owl:Restriction ;
            owl:maxQualifiedCardinality 1 ;
            owl:onClass <https://example.org/crdch_model/Subject> ;
            owl:onProperty linkml:source_subject ],
        [ a owl:Restriction ;
            owl:maxQualifiedCardinality 1 ;
            owl:onClass <https://example.org/crdch_model/SpecimenContainer> ;
            owl:onProperty linkml:contained_in ],
        [ a owl:Restriction ;
            owl:allValuesFrom <https://example.org/crdch_model/BiologicProduct> ;
            owl:onProperty linkml:derived_product ],
        [ a owl:Restriction ;
            owl:maxQualifiedCardinality 1 ;
            owl:onClass <https://example.org/crdch_model/Quantity> ;
            owl:onProperty linkml:distance_from_paired_specimen ],
        [ a owl:Restriction ;
            owl:maxQualifiedCardinality 1 ;
            owl:onClass <https://example.org/crdch_model/ResearchProject> ;
            owl:onProperty linkml:associated_project ],
        [ a owl:Restriction ;
            owl:maxQualifiedCardinality 1 ;
            owl:onClass <https://example.org/crdch_model/SpecimenCreationActivity> ;
            owl:onProperty linkml:creation_activity ],
        [ a owl:Restriction ;
            owl:maxQualifiedCardinality 1 ;
            owl:onClass <http://UNKNOWN.org/enum_CRDCH_Specimen_morphology_assessor_role> ;
            owl:onProperty linkml:morphology_assessor_role ],
        [ a owl:Restriction ;
            owl:allValuesFrom <https://example.org/crdch_model/SpecimenQuantityObservation> ;
            owl:onProperty linkml:quantity_measure ],
        [ a owl:Restriction ;
            owl:allValuesFrom <https://example.org/crdch_model/Specimen> ;
            owl:onProperty linkml:parent_specimen ],
        [ a owl:Restriction ;
            owl:allValuesFrom <https://example.org/crdch_model/Document> ;
            owl:onProperty linkml:related_document ],
        [ a owl:Restriction ;
            owl:maxQualifiedCardinality 1 ;
            owl:onClass <https://example.org/crdch_model/Entity> ;
            owl:onProperty linkml:morphology_pathologically_confirmed ],
        [ a owl:Restriction ;
            owl:maxQualifiedCardinality 1 ;
            owl:onClass <http://UNKNOWN.org/enum_CRDCH_Specimen_cellular_composition_type> ;
            owl:onProperty linkml:cellular_composition_type ],
        [ a owl:Restriction ;
            owl:maxQualifiedCardinality 1 ;
            owl:onClass <http://UNKNOWN.org/enum_CRDCH_Specimen_specimen_type> ;
            owl:onProperty linkml:specimen_type ],
        [ a owl:Restriction ;
            owl:maxQualifiedCardinality 1 ;
            owl:onClass <http://UNKNOWN.org/enum_CRDCH_Specimen_preinvasive_tissue_morphology> ;
            owl:onProperty linkml:preinvasive_tissue_morphology ],
        [ a owl:Restriction ;
            owl:maxQualifiedCardinality 1 ;
            owl:onClass <https://example.org/crdch_model/Entity> ;
            owl:onProperty linkml:description ],
        [ a owl:Restriction ;
            owl:maxQualifiedCardinality 1 ;
            owl:onClass <http://UNKNOWN.org/enum_CRDCH_Specimen_tumor_status_at_collection> ;
            owl:onProperty linkml:tumor_status_at_collection ],
        <https://example.org/crdch_model/Entity> ;
    skos:definition "Any material taken as a sample from a biological entity (living or dead), or from a physical object or the environment. Specimens are usually collected as an example of their kind, often for use in some investigation." ;
    skos:editorialNote "Derived from [Specimen in sheet Specimen](https://docs.google.com/spreadsheets/d/1oWS7cao-fgz2MKWtyr8h2dEL9unX__0bJrWKv6mQmM4/edit#gid=1439310281)" ;
    skos:note "Definition adapted from FHIR Specimen." .

<https://example.org/crdch_model/TimePoint> a owl:Class,
        linkml:ClassDefinition ;
    rdfs:label "TimePoint" ;
    rdfs:subClassOf [ a owl:Restriction ;
            owl:maxQualifiedCardinality 1 ;
            owl:onClass <https://example.org/crdch_model/TimePoint> ;
            owl:onProperty linkml:indexTimePoint ],
        [ a owl:Restriction ;
            owl:allValuesFrom <http://UNKNOWN.org/enum_CRDCH_TimePoint_eventType> ;
            owl:onProperty linkml:eventType ],
        [ a owl:Restriction ;
            owl:maxQualifiedCardinality 1 ;
            owl:onClass <https://example.org/crdch_model/Entity> ;
            owl:onProperty linkml:dateTime ],
        [ a owl:Restriction ;
            owl:maxQualifiedCardinality 1 ;
            owl:onClass <https://example.org/crdch_model/Quantity> ;
            owl:onProperty linkml:offsetFromIndex ],
        [ a owl:Restriction ;
            owl:maxQualifiedCardinality 1 ;
            owl:onClass <https://example.org/crdch_model/Entity> ;
            owl:onProperty linkml:id ],
        <https://example.org/crdch_model/Entity> ;
    skos:definition "A structured representation of a single point in time that allows direct/explicit declaration as a dateTime, or specification in terms of offset from a defined index." ;
    skos:editorialNote "Derived from [TimePoint in sheet TimePoint](https://docs.google.com/spreadsheets/d/1oWS7cao-fgz2MKWtyr8h2dEL9unX__0bJrWKv6mQmM4/edit#gid=300932847)" .

linkml:ClassDefinition a owl:Class ;
    rdfs:label "class_definition" ;
    skos:definition "the definition of a class or interface" .

<https://example.org/crdch_model/Organization> a owl:Class,
        linkml:ClassDefinition ;
    rdfs:label "Organization" ;
    rdfs:subClassOf [ a owl:Restriction ;
            owl:allValuesFrom <https://example.org/crdch_model/Identifier> ;
            owl:onProperty linkml:identifier ],
        [ a owl:Restriction ;
            owl:maxQualifiedCardinality 1 ;
            owl:onClass <https://example.org/crdch_model/Entity> ;
            owl:onProperty linkml:organization_type ],
        [ a owl:Restriction ;
            owl:maxQualifiedCardinality 1 ;
            owl:onClass <https://example.org/crdch_model/Entity> ;
            owl:onProperty linkml:name ],
        [ a owl:Restriction ;
            owl:onClass <https://example.org/crdch_model/Entity> ;
            owl:onProperty linkml:id ;
            owl:qualifiedCardinality 1 ],
        [ a owl:Restriction ;
            owl:maxQualifiedCardinality 1 ;
            owl:onClass <https://example.org/crdch_model/Entity> ;
            owl:onProperty linkml:alias ],
        <https://example.org/crdch_model/Entity> ;
    skos:definition "A grouping of people or organizations with a common purpose such as a data coordinating center, an university, or an institute within a university" ;
    skos:editorialNote "Derived from [Organization in sheet Organization](https://docs.google.com/spreadsheets/d/1oWS7cao-fgz2MKWtyr8h2dEL9unX__0bJrWKv6mQmM4/edit#gid=1477577710)" .

<https://example.org/crdch_model/Subject> a owl:Class,
        linkml:ClassDefinition ;
    rdfs:label "Subject" ;
    rdfs:subClassOf [ a owl:Restriction ;
            owl:maxQualifiedCardinality 1 ;
            owl:onClass <https://example.org/crdch_model/Entity> ;
            owl:onProperty linkml:year_of_birth ],
        [ a owl:Restriction ;
            owl:allValuesFrom <http://UNKNOWN.org/enum_CRDCH_Subject_race> ;
            owl:onProperty linkml:race ],
        [ a owl:Restriction ;
            owl:maxQualifiedCardinality 1 ;
            owl:onClass <http://UNKNOWN.org/enum_CRDCH_Subject_species> ;
            owl:onProperty linkml:species ],
        [ a owl:Restriction ;
            owl:maxQualifiedCardinality 1 ;
            owl:onClass <https://example.org/crdch_model/Entity> ;
            owl:onProperty linkml:year_of_death ],
        [ a owl:Restriction ;
            owl:maxQualifiedCardinality 1 ;
            owl:onClass <http://UNKNOWN.org/enum_CRDCH_Subject_ethnicity> ;
            owl:onProperty linkml:ethnicity ],
        [ a owl:Restriction ;
            owl:maxQualifiedCardinality 1 ;
            owl:onClass <http://UNKNOWN.org/enum_CRDCH_Subject_vital_status> ;
            owl:onProperty linkml:vital_status ],
        [ a owl:Restriction ;
            owl:allValuesFrom <https://example.org/crdch_model/Identifier> ;
            owl:onProperty linkml:identifier ],
        [ a owl:Restriction ;
            owl:onClass <https://example.org/crdch_model/Entity> ;
            owl:onProperty linkml:id ;
            owl:qualifiedCardinality 1 ],
        [ a owl:Restriction ;
            owl:maxQualifiedCardinality 1 ;
            owl:onClass <https://example.org/crdch_model/Quantity> ;
            owl:onProperty linkml:age_at_death ],
        [ a owl:Restriction ;
            owl:maxQualifiedCardinality 1 ;
            owl:onClass <http://UNKNOWN.org/enum_CRDCH_Subject_cause_of_death> ;
            owl:onProperty linkml:cause_of_death ],
        [ a owl:Restriction ;
            owl:maxQualifiedCardinality 1 ;
            owl:onClass <http://UNKNOWN.org/enum_CRDCH_Subject_sex> ;
            owl:onProperty linkml:sex ],
        [ a owl:Restriction ;
            owl:maxQualifiedCardinality 1 ;
            owl:onClass <http://UNKNOWN.org/enum_CRDCH_Subject_breed> ;
            owl:onProperty linkml:breed ],
        <https://example.org/crdch_model/Entity> ;
    skos:definition "Demographics and other administrative information about an individual or animal receiving care or other health-related services." ;
    skos:editorialNote "Derived from [Subject in sheet Subject](https://docs.google.com/spreadsheets/d/1oWS7cao-fgz2MKWtyr8h2dEL9unX__0bJrWKv6mQmM4/edit#gid=1651956379)" .

<https://example.org/crdch_model/Entity> a owl:Class,
        linkml:ClassDefinition ;
    rdfs:label "Entity" ;
    skos:definition "Any resource that has its own identifier" ;
    skos:editorialNote "Derived from [Entity in sheet Entity](https://docs.google.com/spreadsheets/d/1oWS7cao-fgz2MKWtyr8h2dEL9unX__0bJrWKv6mQmM4/edit#gid=65213867)" .

linkml:SlotDefinition a owl:Class ;
    rdfs:label "slot_definition" ;
    skos:definition "the definition of a property or a slot" .



